@prefix dcterms: <http://purl.org/dc/terms/> .
@prefix epa-frs: <http://w3id.org/fio/v1/epa-frs#> .
@prefix epa-frs-data: <http://w3id.org/fio/v1/epa-frs-data#> .
@prefix fio: <http://w3id.org/fio/v1/fio#> .
@prefix owl: <http://www.w3.org/2002/07/owl#> .
@prefix rdfs: <http://www.w3.org/2000/01/rdf-schema#> .
@prefix xsd: <http://www.w3.org/2001/XMLSchema#> .

epa-frs:401Certification a owl:Class ;
    rdfs:label "401 CERTIFICATION"^^xsd:string ;
    dcterms:description "UNDER SECTION 401 OF THE CLEAN WATER ACT (CWA), STATES AND TRIBES HAVE THE AUTHORITY TO REVIEW AND THEN DENY, CERTIFY, OR CONDITION FEDERAL PERMITS OR LICENSES THAT MIGHT RESULT IN A DISCHARGE TO STATE OR TRIBAL WATERS, INCLUDING WETLANDS, TO ENSURE COMPLIANCE WITH STATE WATER QUALITY STANDARDS.  THE MAJOR FEDERAL LICENSES AND PERMITS SUBJECT TO SECTION 401 ARE SECTION 402 AND 404 PERMITS (IN NONDELEGATED STATES), FEDERAL ENERGY REGULATORY COMMISSION (FERC) HYDROPOWER LICENSES, AND RIVERS AND HARBORS ACT SECTION 9 AND 10 PERMITS."^^xsd:string ;
    rdfs:subClassOf epa-frs:WasteWaterPrograms .

epa-frs:AFO a owl:Class ;
    rdfs:label "AFO"^^xsd:string ;
    dcterms:description "ANIMAL FEEDING OPERATION- MEANS A LOT, YARD, CORRAL, BUILDING, OR OTHER AREA IN WHICH ANIMALS ARE CONFINED AND FED AND MAINTAINED FOR 45 DAYS OR MORE IN ANY 12-MONTH PERIOD, AND ALL STRUCTURES USED FOR THE STORAGE OF MANURE FROM ANIMALS IN THE OPERATION"^^xsd:string ;
    rdfs:subClassOf epa-frs:AnimalOperations .

epa-frs:Air-NotApplicable a owl:Class ;
    rdfs:label "AIR - NOT APPLICABLE"^^xsd:string ;
    dcterms:description "FACILITY WIDE AIR REPORTING REQUIREMENTS EXIST, BUT THEY ARE NOT SPECIFIC TO ANY ONE POLLUTANT."^^xsd:string ;
    rdfs:subClassOf epa-frs:EnvironmentalInterest .

epa-frs:Air-Other a owl:Class ;
    rdfs:label "AIR - OTHER"^^xsd:string ;
    dcterms:description "THE AIR EMISSIONS CLASSIFICATION STATUS FOR THE FACILITY IS NOT KNOWN."^^xsd:string ;
    rdfs:subClassOf epa-frs:EnvironmentalInterest .

epa-frs:AirEmissionInventory a owl:Class ;
    rdfs:label "AIR EMISSION INVENTORY"^^xsd:string ;
    dcterms:description "AN ENVIRONMENTAL PROGRAM THAT MAINTAINS A NATIONAL EMISSION INVENTORY WHICH CHARACTERIZES EMISSIONS OF CRITERIA AIR POLLUTANTS.  CRITERIA AIR POLLUTANTS ARE THOSE WHICH AN AMBIENT STANDARD, OBJECTIVE, OR GUIDELINE HAS BEEN ESTABLISHED TO PROTECT HUMAN HEALTH AND WELFARE.  NATIONAL AMBIENT STANDARDS ARE IN PLACE FOR OZONE, CARBON MONOXIDE, NITROGEN OXIDES, SULFUR OXIDES, LEAD, AND FINE PARTICULATE MATTER."^^xsd:string ;
    rdfs:subClassOf epa-frs:AirPrograms .

epa-frs:AirEmissionsClassificationUnknown a owl:Class ;
    rdfs:label "AIR EMISSIONS CLASSIFICATION UNKNOWN"^^xsd:string ;
    dcterms:description "THE AIR EMISSIONS CLASSIFICATION STATUS FOR THE FACILITY IS NOT KNOWN."^^xsd:string ;
    rdfs:subClassOf epa-frs:EnvironmentalInterest .

epa-frs:AirMajor a owl:Class ;
    rdfs:label "AIR MAJOR"^^xsd:string ;
    dcterms:description "A CLEAN AIR ACT STATIONARY SOURCE MAJOR DISCHARGER OF AIR POLLUTANTS ACCORDING TO THE ALABAMA POWER DECISION'S DEFINITION OF A MAJOR SOURCE OR THE 1993 EPA COMPLIANCE MONITORING BRANCH CLASSIFICATION GUIDANCE.  A FACILITY IS CLASSIFIED AS A MAJOR DISCHARGER IF:  (A) ACTUAL OR POTENTIAL EMISSIONS ARE ABOVE THE APPLICABLE MAJOR SOURCE THRESHOLDS; OR (B) ACTUAL OR POTENTIAL CONTROLLED EMISSIONS > 100 TONS/YEAR AS PER ALABAMA POWER DECISION; OR (C) UNREGULATED POLLUTANT ACTUAL OR POTENTIAL CONTROLLED EMISSIONS > 100 TONS/YEAR AS PER ALABAMA POWER DECISION."^^xsd:string ;
    rdfs:subClassOf epa-frs:AirPrograms .

epa-frs:AirMinor a owl:Class ;
    rdfs:label "AIR MINOR"^^xsd:string ;
    dcterms:description "A FACILITY IS CLASSIFIED AS A CLEAN AIR ACT STATIONARY SOURCE MINOR DISCHARGER OF AIR POLLUTANTS IF:  (A) POTENTIAL UNCONTROLLED EMISSIONS < 100 TONS/YEAR; OR (B) MAJOR SOURCE THRESHOLDS ARE NOT DEFINED, OR CLASSIFICATION IS UNKNOWN."^^xsd:string ;
    rdfs:subClassOf epa-frs:AirPrograms .

epa-frs:AirMonitoringSite a owl:Class ;
    rdfs:label "AIR MONITORING SITE"^^xsd:string ;
    dcterms:description "A SITE ESTABLISHED TO MEASURE CONCENTRATIONS OF AIR POLLUTANTS."^^xsd:string ;
    rdfs:subClassOf epa-frs:AirPrograms .

epa-frs:AirO3NAMajor a owl:Class ;
    rdfs:label "AIR O3 N/A MAJOR"^^xsd:string ;
    dcterms:description "FACILITY IS MAJOR BASED UPON ONLY 40 CFR 70 MAJOR SOURCE DEFINITION PARAGRAPH 3 (OZONE N/A AREA LESSER TONS FOR NOX OR VOC)"^^xsd:string ;
    rdfs:subClassOf epa-frs:AirPrograms .

epa-frs:AirProgram a owl:Class ;
    rdfs:label "AIR PROGRAM"^^xsd:string ;
    dcterms:description "AN ENVIRONMENTAL PROGRAM THAT REGULATES OR MONITORS AIR EMISSIONS FROM AREA, STATIONARY, AND MOBILE SOURCES, AS REQUIRED BY THE CLEAN AIR ACT."^^xsd:string ;
    rdfs:subClassOf epa-frs:AirPrograms .

epa-frs:AirProgram-Reservation a owl:Class ;
    rdfs:label "AIR PROGRAM - RESERVATION"^^xsd:string ;
    dcterms:description "THE FEDERAL AIR RULES FOR RESERVATIONS (FARR) APPLIES TO 39 INDIAN RESERVATIONS IN IDAHO, OREGON, AND WASHINGTON. THEY COMPRISE A SET OF RULES THAT ADDRESS AIR QUALITY ISSUES INCLUDING EMISSIONS, PARTICULATE MATTER, WOOD WASTE, SULFUR DIOXIDE, FUELS, OPEN BURNING, AGRICULTURAL BURNING, FORESTRY AND SILVICULTURAL BURNING, AIR POLLUTION EPISODES, REGISTRATION OF AIR POLLUTION SOURCES, REPORTING OF EMISSIONS, AND RULES FOR NON-TITLE V OPERATING PERMITS."^^xsd:string ;
    rdfs:subClassOf epa-frs:AirPrograms .

epa-frs:AirStationaryPointSource a owl:Class ;
    rdfs:label "AIR STATIONARY POINT SOURCE"^^xsd:string ;
    dcterms:description "STATIONARY POINT SOURCES OF EMISSIONS OF CRITERIA AIR POLLUTANTS OR PRECURSORS TO CRITERIA AIR POLLUTANTS.  THESE ARE TYPICALLY COMMERCIAL, INDUSTRIAL, INSTITUTIONAL, GOVERNMENT, OR LARGE MULTI UNIT RESIDENTIAL SOURCES OF EMISSIONS.  THEY ARE NOT MOBILE (VEHICLE) OR AREA SOURCES SUCH AS SINGLE UNIT OR SMALL RESIDENTIAL, CONSTRUCTION, CONSUMER USE EMISSIONS.  CRITERIA AIR POLLUTANTS ARE OZONE, CARBON MONOXIDE NITROGEN OXIDES, SULFUR DIOXIDE, LEAD AND PARTICULATE MATTER."^^xsd:string ;
    rdfs:subClassOf epa-frs:AirPrograms .

epa-frs:AirSyntheticMinor a owl:Class ;
    rdfs:label "AIR SYNTHETIC MINOR"^^xsd:string ;
    dcterms:description "A FACILITY IS CLASSIFIED AS A CLEAN AIR ACT STATIONARY SOURCE SYNTHETIC MINOR DISCHARGER OF AIR POLLUTANTS IF:  (A) POTENTIAL EMISSIONS ARE BELOW ALL APPLICABLE MAJOR SOURCE THRESHOLDS IF AND ONLY IF THE SOURCE COMPLIES WITH FEDERALLY ENFORCEABLE REGULATIONS OR LIMITATIONS; OR (B) ACTUAL EMISSIONS < 100 TONS/YEAR, BUT POTENTIAL UNCONTROLLED EMISSIONS > 100 TONS/YEAR; OR (C) UNREGULATED POLLUTANT ACTUAL EMISSIONS < 100 TONS/YEAR."^^xsd:string ;
    rdfs:subClassOf epa-frs:AirPrograms .

epa-frs:AnimalFeedingOperation a owl:Class ;
    rdfs:label "ANIMAL FEEDING OPERATION"^^xsd:string ;
    dcterms:description "ANIMAL FEEDING OPERATIONS (AFOS) ARE AGRICULTURAL OPERATIONS WHERE ANIMALS ARE KEPT AND RAISED IN CONFINED SITUATIONS. AFOS CONGREGATE ANIMALS, FEED, MANURE, DEAD ANIMALS, AND PRODUCTION OPERATIONS ON A SMALL LAND AREA. FEED IS BROUGHT TO THE ANIMALS RATHER THAN THE ANIMALS GRAZING OR OTHERWISE SEEKING FEED IN PASTURES. AN OPERATION IS AN AFO IF (1) ANIMALS ARE CONFINED FOR AT LEAST 45 DAYS IN A 12-MONTH PERIOD, AND (2) THERE'S NO GRASS OR OTHER VEGETATION IN THE CONFINEMENT AREA DURING THE NORMAL GROWING SEASON."^^xsd:string ;
    rdfs:subClassOf epa-frs:AnimalOperations .

epa-frs:AquiferProtectionProgram a owl:Class ;
    rdfs:label "AQUIFER PROTECTION PROGRAM"^^xsd:string ;
    dcterms:description "THE AQUIFER PROTECTION PROGRAM REQUIRES A WATER POLLUTION ABATEMENT PLAN (WPAP) FOR ANY REGULATED ACTIVITY PROPOSED ON DESIGNATED AQUIFER RECHARGE ZONES (I.E., THE TEXAS EDWARDS AQUIFER). THE PLAN INCLUDES ANY CONSTRUCTION-RELATED ACTIVITY ON THE RECHARGE ZONE, SUCH AS THE CONSTRUCTION OF BUILDINGS, UTILITY STATIONS, ROADS, HIGHWAYS, RAILROADS; CLEARING, EXCAVATION, OR ANY OTHER ACTIVITIES THAT ALTER OR DISTURB THE TOPOGRAPHIC, GEOLOGIC, OR EXISTING RECHARGE CHARACTERISTICS OF A SITE; OR ANY OTHER ACTIVITIES WHICH MAY POSE A POTENTIAL FOR CONTAMINATING THE AQUIFER AND HYDROLOGICALLY CONNECTED SURFACE STREAMS. "^^xsd:string ;
    rdfs:subClassOf epa-frs:GroundWaterPrograms .

epa-frs:AsbestosAbatementProgram a owl:Class ;
    rdfs:label "ASBESTOS ABATEMENT PROGRAM"^^xsd:string ;
    dcterms:description "AN ENVIRONMENTAL PROGRAM CONCERNED WITH ASBESTOS REMOVAL AND DISPOSAL."^^xsd:string ;
    rdfs:subClassOf epa-frs:AirPrograms .

epa-frs:BRAC a owl:Class ;
    rdfs:label "BRAC"^^xsd:string ;
    dcterms:description "BASE REALIGNMENT AND CLOSURE"^^xsd:string ;
    rdfs:subClassOf epa-frs:RemediationAndRedevelopmentPrograms .

epa-frs:Biosolids a owl:Class ;
    rdfs:label "BIOSOLIDS"^^xsd:string ;
    dcterms:description "BIOSOLIDS ARE A PRIMARILY ORGANIC, SEMISOLID PRODUCT RESULTING FROM THE WASTEWATER TREATMENT PROCESS AND CAN BE BENEFICIALLY RECYCLED. BECAUSE BIOSOLIDS CONTAIN ESSENTIAL PLANT NUTRIENTS AND ORGANIC MATTER, THEY CAN BE TREATED, PROCESSED AND USED AS A SOIL AMENDMENT AND NUTRIENT SOURCE TO IMPROVE AND MAINTAIN PRODUCTIVE SOILS AND STIMULATE PLANT GROWTH. HOWEVER, THE TREATMENT PROCESS MUST MEET ALL APPLICABLE REQUIREMENTS AND REGULATORY STANDARDS UNDER STATE AND FEDERAL LAW BEFORE THE BIOSOLIDS CAN BE APPLIED TO THE LAND. AT THE NATIONAL LEVEL, BIOSOLIDS FALL UNDER THE FEDERAL CLEAN WATER ACT (CWA); STATES MAY ISSUE PERMITS THAT IMPOSE ADDITIONAL OR MORE STRINGENT REQUIREMENTS."^^xsd:string ;
    rdfs:subClassOf epa-frs:WasteWaterPrograms .

epa-frs:BrownfieldsProperty a owl:Class ;
    rdfs:label "BROWNFIELDS PROPERTY"^^xsd:string ;
    dcterms:description "A LOCATION IDENTIFIED BY A BROWNFIELDS PILOT/GRANT."^^xsd:string ;
    rdfs:subClassOf epa-frs:RemediationAndRedevelopmentPrograms .

epa-frs:BrownfieldsSite a owl:Class ;
    rdfs:label "BROWNFIELDS SITE"^^xsd:string ;
    dcterms:description "WITH CERTAIN LEGAL EXCLUSIONS AND ADDITIONS/ THE TERM 'BROWNFIELD SITE' MEANS REAL PROPERTY/ THE EXPANSION/ REDEVELOPMENT/ OR REUSE OF WHICH MAY BE COMPLICATED BY THE PRESENCE OR POTENTIAL PRESENCE OF A HAZARDOUS SUBSTANCE/ POLLUTANT"^^xsd:string ;
    rdfs:subClassOf epa-frs:RemediationAndRedevelopmentPrograms .

epa-frs:CESQG a owl:Class ;
    rdfs:label "CESQG"^^xsd:string ;
    dcterms:description "HAZARDOUS WASTE CONDITIONALLY EXEMPT SMALL QUANTITY GENERATORS GENERATE:  A) 100 KILOGRAMS OR LESS OF HAZARDOUS WASTE PER CALENDAR MONTH, AND ACCUMULATE 1000 KG OR LESS OF HAZARDOUS WASTE AT ANY TIME; OR (B) ONE KILOGRAM OR LESS OF ACUTELY HAZARDOUS WASTE PER CALENDAR MONTH, AND ACCUMULATE AT ANY TIME: 1 KG OR LESS OF ACUTELY HAZARDOUS WASTE; OR 100 KG OR LESS OF ANY RESIDUE OR CONTAMINATED SOIL, WASTE OR OTHER DEBRIS RESULTING FROM THE CLEANUP OF A SPILL, INTO OR ON ANY LAND OR WATER, OF ACUTELY HAZARDOUS WASTE; OR (C) 100 KG OR LESS OF ANY RESIDUE OR CONTAMINATED SOIL, WASTE OR OTHER DEBRIS RESULTING FROM THE CLEANUP OF A SPILL, INTO OR ON ANY LAND OR WATER, OF ACUTELY HAZARDOUS WASTE DURING ANY CALENDAR MONTH, AND ACCUMULATE AT ANY TIME:  1 KG OR LESS OF ACUTELY HAZARDOUS WASTE; OR 100 KG OR LESS OF ANY RESIDUE OR CONTAMINATED SOIL, WASTE OR OTHER DEBRIS RESULTING FROM THE CLEANUP OF A SPILL, INTO OR ON ANY LAND OR WATER, OF ACUTELY HAZARDOUS WASTE."^^xsd:string ;
    rdfs:subClassOf epa-frs:HazardousWastePrograms .

epa-frs:CathodeRayTubePermit a owl:Class ;
    rdfs:label "CATHODE RAY TUBE PERMIT"^^xsd:string ;
    dcterms:description "PERMIT FOR THE COLLECTION AND/OR RECYCLING OF DISCARDED CATHODE RAY TUBE (CRT) DEVICES AND THE DISASSEMBLY AND REMOVAL OF TOXIC PARTS IN A MANNER THAT IS SAFE FOR HUMAN HEALTH AND THE ENVIRONMENT. ELECTRONIC WASTE, ALSO KNOWN AS E-WASTE, REFERS TO ELECTRONIC EQUIPMENT THAT IS NO LONGER USABLE OR WANTED. IT ENCOMPASSES A BROAD AND GROWING RANGE OF ELECTRONIC DEVICES, INCLUDING COMPUTERS, TVS, CELLULAR PHONES AND PERSONAL STEREOS, DIGITAL CAMERAS, MP3 PLAYERS, DVD PLAYERS AND ELECTRONIC GAMES. DISCARDED ELECTRONICS CONTAIN HAZARDOUS MATERIALS. IF DISPOSED IMPROPERLY, THEY POSE A POTENTIAL THREAT TO HUMAN HEALTH AND THE ENVIRONMENT. THE ACIDIC CONDITIONS OF A LANDFILL PROVIDE AN ENVIRONMENT IN WHICH LEAD AND OTHER HEAVY METALS MAY LEAK OUT AND CONTAMINATE GROUNDWATER. E-WASTE ACCOUNTS FOR 40 PERCENT OF THE LEAD AND 75 PERCENT OF THE HEAVY METALS FOUND IN LANDFILLS. MUCH OF THE FOCUS ON MANAGING E-WASTE REVOLVES AROUND CRTS, OFTEN CALLED \"PICTURE TUBES,\" WHICH CONVERT AN ELECTRONIC SIGNAL INTO A VISUAL IMAGE. COMPUTER MONITORS, TELEVISIONS, SOME CAMCORDERS, AND OTHER ELECTRONIC DEVICES CONTAIN CRTS. A TYPICAL CRT CONTAINS BETWEEN TWO AND FIVE POUNDS OF LEAD"^^xsd:string ;
    rdfs:subClassOf epa-frs:HazardousWasteProgram .

epa-frs:CleanWatershedsNeedsSurvey2008 a owl:Class ;
    rdfs:label "CLEAN WATERSHEDS NEEDS SURVEY 2008"^^xsd:string ;
    dcterms:description "THE FACILITY WAS INCLUDED IN THE 2008 CLEAN WATERSHEDS NEEDS SURVEY (CWNS), WHICH IS A COMPREHENSIVE ASSESSMENT OF THE CAPITAL NEEDS REQUIRED TO MEET WATER QUALITY GOALS SET IN THE CLEAN WATER ACT. EVERY FOUR YEARS, THE STATES AND EPA COLLECT INFORMATION ABOUT PUBLICLY OWNED WASTEWATER COLLECTION AND TREATMENT FACILITIES, STORMWATER AND COMBINED SEWER OVERFLOWS CONTROL FACILITIES, NONPOINT SOURCE (NPS) POLLUTION CONTROL PROJECTS, DECENTRALIZED WASTEWATER MANAGEMENT, AND ESTUARY MANAGEMENT PROJECTS. INFORMATION COLLECTED INCLUDES ESTIMATED NEEDS, INCLUDING COSTS AND TECHNICAL INFORMATION, TO ADDRESS WATER QUALITY OR WATER-RELATED PUBLIC HEALTH PROBLEMS, LOCATION AND CONTACT INFORMATION, POPULATIONS SERVED, FLOW, EFFLUENT, AND UNIT PROCESS INFORMATION, AND NPS BEST MANAGEMENT PRACTICES. THIS INFORMATION IS USED BY EPA TO DOCUMENT NATIONAL NEEDS IN A REPORT TO CONGRESS, WHICH ASSISTS IN BUDGETING EFFORTS. THE DATA ARE ALSO USED TO HELP MEASURE ENVIRONMENTAL PROGRESS, CONTRIBUTE TO ACADEMIC RESEARCH, PROVIDE INFORMATION TO THE PUBLIC, AND HELP LOCAL AND STATE GOVERNMENTS IMPLEMENT WATER QUALITY PROGRAMS."^^xsd:string ;
    rdfs:subClassOf epa-frs:WasteWaterPrograms .

epa-frs:ClosedCriminalEnforcementCase a owl:Class ;
    rdfs:label "CLOSED CRIMINAL ENFORCEMENT CASE"^^xsd:string ;
    dcterms:description "CLOSED CRIMINAL CASES THAT RESULTED FROM CRIMINAL INVESTIGATIONS OF ALLEGED VIOLATIONS OF ENVIRONMENTAL STATUES."^^xsd:string ;
    rdfs:subClassOf epa-frs:LegalEnforcementActivities .

epa-frs:CoastalErosion a owl:Class ;
    rdfs:label "COASTAL EROSION"^^xsd:string ;
    dcterms:description "STATE PROGRAMS TO PREVENT AND REDUCE COASTAL EROSION INCLUDING PRESERVING NATURAL PROTECTIVE FEATURES SUCH AS DUNES AND BLUFFS; RESTRICTING OR PROHIBITING ACTIVITIES, DEVELOPMENT OR ACTIONS IN NATURAL PROTECTIVE FEATURE AREAS TO PREVENT OR REDUCE EROSION; PLACING NEW CONSTRUCTION OR STRUCTURES A SAFE DISTANCE FROM AREAS OF ACTIVE EROSION AND IMPACTS OF COASTAL STORMS; REGULATING THE PLACEMENT AND CONSTRUCTION OF EROSION PROTECTION STRUCTURES; AND ESTABLISHING STANDARDS FOR THE ISSUANCE OF COASTAL EROSION MANAGEMENT PERMITS."^^xsd:string ;
    rdfs:subClassOf epa-frs:CoastalAndOceanPrograms .

epa-frs:CoastalZoneManagement-CZM a owl:Class ;
    rdfs:label "COASTAL ZONE MANAGEMENT (CZM)"^^xsd:string ;
    dcterms:description "THE NATION-WIDE COASTAL ZONE MANAGEMENT (CZM) PROGRAM IS A VOLUNTARY STATE-FEDERAL PARTNERSHIP WHICH ENCOURAGES STATES TO ADOPT THEIR OWN MANAGEMENT PROGRAMS IN ORDER TO MEET THE FEDERAL GOALS OF PROTECTION, RESTORATION, AND APPROPRIATE DEVELOPMENT OF COASTAL ZONE RESOURCES. THE NATIONAL CZM PROGRAM IS BASED ON THE FEDERAL COASTAL ZONE MANAGEMENT ACT OF 1972, WHICH IS IMPLEMENTED BY THE NATIONAL OCEANIC AND ATMOSPHERIC ADMINISTRATION (NOAA) THROUGH THE OFFICE OF OCEAN AND COASTAL RESOURCE MANAGEMENT. COASTAL AREAS AND WETLANDS ARE ALSO PROTECTED BY SECTION 401 OF THE CLEAN WATER ACT, WHICH REQUIRES PERMITS FOR ACTIVITIES SUCH AS: DEVELOPMENT INVOLVING FILLING OF WETLANDS; DREDGING AND OTHER IN-WATER ACTIVITIES; BRIDGE CROSSINGS; CONSTRUCTION OF DRIVES AND PARKING LOTS; ETC."^^xsd:string ;
    rdfs:subClassOf epa-frs:CoastalAndOceanPrograms .

epa-frs:CombinedSewerOverflow a owl:Class ;
    rdfs:label "COMBINED SEWER OVERFLOW"^^xsd:string ;
    dcterms:description "EPA''S COMBINED SEWER OVERFLOW (CSO) CONTROL POLICY IS A NATIONAL FRAMEWORK FOR CONTROL OF CSOS THROUGH THE NATIONAL POLLUTANT DISCHARGE ELIMINATION SYSTEM (NPDES) PERMITTING PROGRAM. THE POLICY RESULTED FROM NEGOTIATIONS AMONG MUNICIPAL ORGANIZATIONS, ENVIRONMENTAL GROUPS, AND STATE AGENCIES. IT PROVIDES GUIDANCE TO MUNICIPALITIES AND STATE AND FEDERAL PERMITTING AUTHORITIES ON HOW TO MEET THE CLEAN WATER ACT''S POLLUTION CONTROL GOALS AS FLEXIBLY AND COST-EFFECTIVELY AS POSSIBLE."^^xsd:string ;
    rdfs:subClassOf epa-frs:WasteWaterPrograms .

epa-frs:CommunityWaterSystem a owl:Class ;
    rdfs:label "COMMUNITY WATER SYSTEM"^^xsd:string ;
    dcterms:description "A PUBLIC WATER SYSTEM THAT PIPES WATER FOR HUMAN CONSUMPTION AT LEAST 15 SERVICE CONNECTIONS USED BY YEAR-ROUND RESIDENTS OR REGULARLY SERVES AT LEAST 25 YEAR-ROUND RESIDENTS."^^xsd:string ;
    rdfs:subClassOf epa-frs:DrinkingWaterPrograms .

epa-frs:ComplianceActivity a owl:Class ;
    rdfs:label "COMPLIANCE ACTIVITY"^^xsd:string ;
    dcterms:description "A COMPLIANCE MONITORING OR ENFORCEMENT ACTIVITY, FROM THE TIME AN INSPECTOR CONDUCTS AN INSPECTION UNTIL THE TIME THE INSPECTOR CLOSES OR THE CASE SETTLES THE ENFORCEMENT ACTION."^^xsd:string ;
    rdfs:subClassOf epa-frs:LegalEnforcementActivities .

epa-frs:ComplianceAndEmissionsReporting a owl:Class ;
    rdfs:label "COMPLIANCE AND EMISSIONS REPORTING"^^xsd:string ;
    dcterms:description "EPA REGULATIONS CODIFIED IN 40 CFR PART 60 AND 63 REQUIRE AFFECTED SOURCES TO PERFORM EMISSIONS SOURCE TESTS, CONDUCT CONTINUOUS EMISSIONS MONITORING, AND SUBMIT COMPLIANCE AND EMISSIONS REPORTS. THESE REPORTS ARE ELECTRONICALLY SUBMITTED VIA THE COMPLIANCE AND EMISSIONS DATA REPORTING INTERFACE (CEDRI) WHICH IS LOCATED ON EPA'S CENTRAL DATA EXCHANGE (CDX)."^^xsd:string ;
    rdfs:subClassOf epa-frs:AirPrograms .

epa-frs:ComplianceAssistance a owl:Class ;
    rdfs:label "COMPLIANCE ASSISTANCE"^^xsd:string ;
    dcterms:description "COMPLIANCE ASSISTANCE HELPS THE REGULATED COMMUNITY UNDERSTAND AND MEET THEIR ENVIRONMENTAL OBLIGATIONS."^^xsd:string ;
    rdfs:subClassOf epa-frs:AssistanceAndSupportPrograms .

epa-frs:ConcentratedAnimalFeedingOperation a owl:Class ;
    rdfs:label "CONCENTRATED ANIMAL FEEDING OPERATION"^^xsd:string ;
    dcterms:description "CONCENTRATED ANIMAL FEEDING OPERATIONS (CAFOS) ARE ANIMAL FEEDING OPERATIONS (AFOS) THAT MEET CERTAIN EPA CRITERIA. PREVIOUS EPA REGULATIONS BASED THE DEFINITION OF CAFOS ON THE NUMBER OF \"ANIMAL UNITS\" CONFINED. EPA NO LONGER USES THE TERM \"ANIMAL UNIT,\" BUT INSTEAD REFERS TO THE ACTUAL NUMBER OF ANIMALS AT THE OPERATION. CAFOS MAKE UP APPROXIMATELY 15 PERCENT OF TOTAL AFOS. AN OPERATION IS A CAFO IF (1) IT MEETS THE DEFINITION OF AN AFO, AND (2) THE OPERATION MEETS ONE OF THE REGULATORY DEFINITIONS OF LARGE CAFOS, MEDIUM CAFO, AND SMALL CAFOS."^^xsd:string ;
    rdfs:subClassOf epa-frs:AnimalOperations .

epa-frs:ConstructionDemolitionLandfill a owl:Class ;
    rdfs:label "CONSTRUCTION & DEMOLITION LANDFILL"^^xsd:string ;
    dcterms:description "LANDFILL THAT IS PERMITTED TO ACCEPT CONSTRUCTION AND DEMOLITION WASTE."^^xsd:string ;
    rdfs:subClassOf epa-frs:SolidWastePrograms .

epa-frs:CorrectiveAction a owl:Class ;
    rdfs:label "CORRECTIVE ACTION"^^xsd:string ;
    dcterms:description "SITES SUBJECT TO ENFORCEABLE RCRA CORRECTIVE ACTION (CA) OBLIGATIONS. SITES INCLUDED ARE THOSE WITH ONGOING CA, AND ALSO THOSE WHERE CA IS STATUTORILY REQUIRED TO BE ADDRESSED (I.E., TSD FACILITIES), BUT HAS NOT YET BEEN IMPOSED."^^xsd:string ;
    rdfs:subClassOf epa-frs:HazardousWastePrograms .

epa-frs:CriteriaAirPollutantMajor a owl:Class ;
    rdfs:label "CRITERIA AIR POLLUTANT MAJOR"^^xsd:string ;
    dcterms:description "FACILITY IS MAJOR BASED UPON 40 CFR 70 MAJOR SOURCE DEFINITION PARAGRAPH 2 (100 TPY ANY CAP.  ALSO MEETS PARAGRAPH 3 DEFINITION, BUT NOT PARAGRAPH 1 DEFINITION)."^^xsd:string ;
    rdfs:subClassOf epa-frs:AirPrograms .

epa-frs:CriteriaAndHazardousAirPollutantInventory a owl:Class ;
    rdfs:label "CRITERIA AND HAZARDOUS AIR POLLUTANT INVENTORY"^^xsd:string ;
    dcterms:description "A NATIONAL INVENTORY OF EMISSIONS DATA OF BOTH HAZARDOUS AIR POLLUTANTS (HAPS) AND CRITERIA AIR POLLUTANTS. CRITERIA AIR POLLUTANTS INCLUDE OZONE, CARBON MONOXIDE, NITROGEN OXIDES, SULFUR OXIDES, LEAD, AND FINE PARTICULATE MATTER AND HAPS, OR AIR TOXICS, ARE DEFINED IN SECTION 112(B) OF THE 1990 CLEAN AIR ACT AMENDMENTS."^^xsd:string ;
    rdfs:subClassOf epa-frs:AirPrograms .

epa-frs:DamSite a owl:Class ;
    rdfs:label "DAM SITE"^^xsd:string ;
    dcterms:description "UNDER STATE LAW, THE DEPARTMENT OF ECOLOGY IS RESPONSIBLE FOR REGULATING DAMS THAT CAPTURE AND STORE AT LEAST 10 ACRE-FEET OF WATER OR WATERY MATERIALS SUCH AS MINE TAILINGS, SEWAGE AND MANURE WASTE. ECOLOGYS DAM SAFETY OFFICE CURRENTLY OVERSEES ABOUT 870 DAMS ACROSS THE STATE THROUGH PLAN REVIEWS AND CONSTRUCTION INSPECTIONS OF NEW DAMS AS WELL AS CONDUCTING INSPECTIONS OF EXISTING DAMS TO ENSURE PROPER OPERATION AND MAINTENANCE"^^xsd:string ;
    rdfs:subClassOf epa-frs:WaterResourcesPrograms .

epa-frs:DischargePreventionProgram a owl:Class ;
    rdfs:label "DISCHARGE PREVENTION PROGRAM"^^xsd:string ;
    dcterms:description "DISCHARGE PREVENTION, CONTAINMENT AND COUNTERMEASURES (DPCC) IS A STATE PROGRAM THAT  WORKS TO FORESTALL THE RELEASE OF HAZARDOUS SUBSTANCES AND PETROLEUM PRODUCTS TO THE ENVIRONMENT, THEREBY PROTECTING NATURAL RESOURCES AND PUBLIC HEALTH BEFORE PROBLEMS OCCUR. THE PROGRAM CENTERS ON SOUND MANAGEMENT PRACTICES THAT ARE CONSIDERED ESSENTIAL WHEN WORKING WITH HAZARDOUS SUBSTANCES.  THESE PRACTICES INCLUDE TRAINING EMPLOYEES WHO HANDLE SUCH MATERIALS, PERIODICALLY INSPECTING STORAGE TANKS, AND ASSURING THAT ADEQUATE SECONDARY CONTAINMENT IS IN PLACE, AS WELL AS DEVELOPING STANDARD OPERATING PROCEDURES FOR ROUTINE OPERATIONS AND MAINTENANCE. THE PROGRAM ALSO WORKS TO ENSURE THAT RESPONSE PLANS, TRAINED PERSONNEL AND EMERGENCY EQUIPMENT ARE AT HAND SHOULD AN INCIDENT OCCUR. ALL FACILITIES AND INDIVIDUALS IN THE STATE, EVEN HOMEOWNERS, ARE SUBJECT TO THE REPORTING REQUIREMENTS SHOULD A DISCHARGE OF A HAZARDOUS SUBSTANCE OCCUR. HOWEVER, THE MAJORITY OF THE REGULATORY REQUIREMENTS APPLY ONLY TO FACILITIES THAT STORE 20,000 GALLONS OR MORE OF STATE-REGULATED HAZARDOUS SUBSTANCES, EXCLUDING PETROLEUM PRODUCTS, OR 200,000 GALLONS OF REGULATED HAZARDOUS SUBSTANCES INCLUDING PETROLEUM PRODUCTS. "^^xsd:string ;
    rdfs:subClassOf epa-frs:ChemicalStoragePrograms .

epa-frs:DrinkingWaterProgram a owl:Class ;
    rdfs:label "DRINKING WATER PROGRAM"^^xsd:string ;
    dcterms:description "AN ENVIRONMENTAL PROGRAM THAT PROTECTS THE QUALITY OF DRINKING WATER IN THE UNITED STATES, AS REQUIRED BY THE SAFE DRINKING WATER ACT."^^xsd:string ;
    rdfs:subClassOf epa-frs:DrinkingWaterPrograms .

epa-frs:DrinkingWaterSystem a owl:Class ;
    rdfs:label "DRINKING WATER SYSTEM"^^xsd:string ;
    dcterms:description "A PUBLIC DRINKING WATER SYSTEM HAS AT LEAST 15 SERVICE CONNECTIONS OR REGULARLY SERVES AN AVERAGE OR AT LEAST 25 INDIVIDUALS DAILY AT LEAST 60 DAYS OUT OF THE YEAR."^^xsd:string ;
    rdfs:subClassOf epa-frs:DrinkingWaterPrograms .

epa-frs:DryCleanerRemediationProgram a owl:Class ;
    rdfs:label "DRY CLEANER REMEDIATION PROGRAM"^^xsd:string ;
    dcterms:description "THE DRY CLEANER REMEDIATION PROGRAM (DCRP) WAS ESTABLISHED AT THE STATE LEVEL TO CLEAN UP LEAD AT DRY CLEANER RELATED CONTAMINATED SITES. IT ALSO ESTABLISHED DRY CLEANER FACILITY REGISTRATION REQUIREMENTS, FEES, PERFORMANCE STANDARDS, DISTRIBUTOR REGISTRATION, AND REVENUE DISBURSEMENT."^^xsd:string ;
    rdfs:subClassOf epa-frs:RemediationAndRedevelopmentPrograms .

epa-frs:E-Waste a owl:Class ;
    rdfs:label "E-WASTE"^^xsd:string ;
    dcterms:description "FACILITIES THAT COLLECTS, BROKERS, STORES, RESELLS, DISMANTLES OR DEMANUFACTURES E-WASTE. "^^xsd:string ;
    rdfs:subClassOf epa-frs:SolidWastePrograms .

epa-frs:EPCRA a owl:Class ;
    rdfs:label "EPCRA"^^xsd:string ;
    dcterms:description "THE EMERGENCY PLANNING & COMMUNITY RIGHT-TO-KNOW ACT (EPCRA) IS INCLUDED AS TITLE III OF THE SUPERFUND AMENDMENTS AND REAUTHORIZATION ACT (SARA) OF 1986 AND IS SOMETIMES REFERRED TO AS SARA TITLE III.  THE EPCRA PROGRAM PROVIDES THE PUBLIC WITH KNOWLEDGE OF AND ACCESS TO INFORMATION REGARDING THE USE, STORAGE, PRODUCTION, AND RELEASE OF HAZARDOUS CHEMICALS TO THE ENVIRONMENT, AND ENCOURAGES AND SUPPORTS RESPONSE PLANNING FOR ENVIRONMENTAL EMERGENCIES."^^xsd:string ;
    rdfs:subClassOf epa-frs:ChemicalStoragePrograms .

epa-frs:ElectricGenerator a owl:Class ;
    rdfs:label "ELECTRIC GENERATOR"^^xsd:string ;
    dcterms:description "A FACILITY THAT PRODUCES ELECTRICITY, COMMONLY EXPRESSED IN KILOWATT-HOURS (KWH) OR MEGAWATT HOURS (MWH), INCLUDING ELECTRIC UTILITIES AND INDEPENDENT POWER PRODUCERS."^^xsd:string ;
    rdfs:subClassOf epa-frs:AirPrograms .

epa-frs:ElectricPowerGeneration a owl:Class ;
    rdfs:label "ELECTRIC POWER GENERATION"^^xsd:string ;
    dcterms:description "AN ELECTRICITY GENERATING PLANT THAT PROVIDES POWER TO THE ELECTRIC GRID. "^^xsd:string ;
    rdfs:subClassOf epa-frs:AirPrograms .

epa-frs:ElectricPowerGenerator-BiomassBased a owl:Class ;
    rdfs:label "ELECTRIC POWER GENERATOR (BIOMASS BASED)"^^xsd:string ;
    dcterms:description "AN ELECTRICITY GENERATING PLANT THAT PROVIDES POWER TO THE ELECTRIC GRID, USING BIOMASS AS THE PLANT¿S PRIMARY FUEL, BASED ON MAXIMUM HEAT INPUT. BIOMASS IS A FUEL DERIVED FROM ORGANIC MATTER SUCH AS WOOD AND PAPER PRODUCTS, AGRICULTURAL WASTE, OR METHANE (E.G., FROM LANDFILLS). "^^xsd:string ;
    rdfs:subClassOf epa-frs:AirPrograms .

epa-frs:ElectricPowerGenerator-CoalBased a owl:Class ;
    rdfs:label "ELECTRIC POWER GENERATOR (COAL BASED)"^^xsd:string ;
    dcterms:description "AN ELECTRICITY GENERATING PLANT THAT PROVIDES POWER TO THE ELECTRIC GRID, USING COAL AS THE PLANT¿S PRIMARY FUEL, BASED ON MAXIMUM HEAT INPUT."^^xsd:string ;
    rdfs:subClassOf epa-frs:AirPrograms .

epa-frs:ElectricPowerGenerator-GasBased a owl:Class ;
    rdfs:label "ELECTRIC POWER GENERATOR (GAS BASED)"^^xsd:string ;
    dcterms:description "AN ELECTRICITY GENERATING PLANT THAT PROVIDES POWER TO THE ELECTRIC GRID, USING GAS THE PLANT¿S PRIMARY FUEL, BASED ON MAXIMUM HEAT INPUT."^^xsd:string ;
    rdfs:subClassOf epa-frs:AirPrograms .

epa-frs:ElectricPowerGenerator-GeothermalBased a owl:Class ;
    rdfs:label "ELECTRIC POWER GENERATOR (GEOTHERMAL BASED)"^^xsd:string ;
    dcterms:description "AN ELECTRICITY GENERATING PLANT THAT PROVIDES POWER TO THE ELECTRIC GRID, WITH THE MAXIMUM GENERATION BASED ON GEOTHERMAL POWER. "^^xsd:string ;
    rdfs:subClassOf epa-frs:AirPrograms .

epa-frs:ElectricPowerGenerator-NuclearBased a owl:Class ;
    rdfs:label "ELECTRIC POWER GENERATOR (NUCLEAR BASED)"^^xsd:string ;
    dcterms:description "AN ELECTRICITY GENERATING PLANT THAT PROVIDES POWER TO THE ELECTRIC GRID, WITH THE MAXIMUM GENERATION BASED ON NUCLEAR POWER."^^xsd:string ;
    rdfs:subClassOf epa-frs:AirPrograms .

epa-frs:ElectricPowerGenerator-OilBased a owl:Class ;
    rdfs:label "ELECTRIC POWER GENERATOR (OIL BASED)"^^xsd:string ;
    dcterms:description "AN ELECTRICITY GENERATING PLANT THAT PROVIDES POWER TO THE ELECTRIC GRID, USING OIL AS THE PLANT¿S PRIMARY FUEL, BASED ON MAXIMUM HEAT INPUT."^^xsd:string ;
    rdfs:subClassOf epa-frs:AirPrograms .

epa-frs:ElectricPowerGenerator-OtherFossilFuelBased a owl:Class ;
    rdfs:label "ELECTRIC POWER GENERATOR (OTHER FOSSIL FUEL BASED)"^^xsd:string ;
    dcterms:description "AN ELECTRICITY GENERATING PLANT THAT PROVIDES POWER TO THE ELECTRIC GRID, USING FOSSIL FUEL AS THE PLANT¿S PRIMARY FUEL, BASED ON MAXIMUM HEAT INPUT. FOSSIL FUEL IS ANY NATURALLY OCCURRING ORGANIC FUEL, SUCH AS PETROLEUM, COAL, AND NATURAL GAS."^^xsd:string ;
    rdfs:subClassOf epa-frs:AirPrograms .

epa-frs:ElectricPowerGenerator-SolarBased a owl:Class ;
    rdfs:label "ELECTRIC POWER GENERATOR (SOLAR BASED)"^^xsd:string ;
    dcterms:description "AN ELECTRICITY GENERATING PLANT THAT PROVIDES POWER TO THE ELECTRIC GRID, WITH THE MAXIMUM GENERATION BASED ON SOLAR POWER."^^xsd:string ;
    rdfs:subClassOf epa-frs:AirPrograms .

epa-frs:ElectricPowerGenerator-UnknownOtherSource a owl:Class ;
    rdfs:label "ELECTRIC POWER GENERATOR (UNKNOWN/OTHER SOURCE)"^^xsd:string ;
    dcterms:description "None"^^xsd:string ;
    rdfs:subClassOf epa-frs:EnvironmentalInterest .

epa-frs:ElectricPowerGenerator-UnknownSource a owl:Class ;
    rdfs:label "ELECTRIC POWER GENERATOR (UNKNOWN SOURCE)"^^xsd:string ;
    dcterms:description "AN ELECTRICITY GENERATING PLANT THAT PROVIDES POWER TO THE ELECTRIC GRID, WITH THE MAXIMUM GENERATION BASED ON AN UNKNOWN SOURCE."^^xsd:string ;
    rdfs:subClassOf epa-frs:AirPrograms .

epa-frs:ElectricPowerGenerator-WaterBased a owl:Class ;
    rdfs:label "ELECTRIC POWER GENERATOR (WATER BASED)"^^xsd:string ;
    dcterms:description "AN ELECTRICITY GENERATING PLANT THAT PROVIDES POWER TO THE ELECTRIC GRID, WITH THE MAXIMUM GENERATION BASED ON WATER POWER."^^xsd:string ;
    rdfs:subClassOf epa-frs:AirPrograms .

epa-frs:ElectricPowerGenerator-WindBased a owl:Class ;
    rdfs:label "ELECTRIC POWER GENERATOR (WIND BASED)"^^xsd:string ;
    dcterms:description "AN ELECTRICITY GENERATING PLANT THAT PROVIDES POWER TO THE ELECTRIC GRID, WITH THE MAXIMUM GENERATION BASED ON WIND POWER."^^xsd:string ;
    rdfs:subClassOf epa-frs:AirPrograms .

epa-frs:EnforcementComplianceActivity a owl:Class ;
    rdfs:label "ENFORCEMENT/COMPLIANCE ACTIVITY"^^xsd:string ;
    dcterms:description "ENFORCEMENT/COMPLIANCE ACTIVITY"^^xsd:string ;
    rdfs:subClassOf epa-frs:LegalEnforcementActivities .

epa-frs:EnvironmentalAssistance a owl:Class ;
    rdfs:label "ENVIRONMENTAL ASSISTANCE"^^xsd:string ;
    dcterms:description "ASSISTANCE AND OUTREACH ACTIVITIES RELATED TO ENVIRONMENTAL ISSUES."^^xsd:string ;
    rdfs:subClassOf epa-frs:AssistanceAndSupportPrograms .

epa-frs:EnvironmentalCleanupStudyArea a owl:Class ;
    rdfs:label "ENVIRONMENTAL CLEANUP STUDY AREA"^^xsd:string ;
    dcterms:description "A GROUP OF INDIVIDUAL SITES THAT MAY BE CONTRIBUTING TO A LARGER, AREA-WIDE PROBLEM, WHICH IS STUDIED TO DETERMINE POTENTIAL SOURCES OF CONTAMINATION."^^xsd:string ;
    rdfs:subClassOf epa-frs:RemediationAndRedevelopmentPrograms .

epa-frs:ErosionControl a owl:Class ;
    rdfs:label "EROSION CONTROL"^^xsd:string ;
    dcterms:description "A STATE REGULATORY PROGRAM ENACTED TO REDUCE THE ADVERSE EFFECTS OF STORMWATER RUNOFF AND SEDIMENT.  UNDER THIS PROGRAM, NO PERSON, UNLESS EXEMPTED, MAY ENGAGE IN A LAND DISTURBING ACTIVITY WITHOUT FIRST SUBMITTING A STORMWATER MANAGEMENT AND SEDIMENT CONTROL PLAN TO THE APPROPRIATE IMPLEMENTING AGENCY AND OBTAINING A PERMIT.  A LAND DISTURBING ACTIVITY IS DEFINED AS ANY USE OF THE LAND THAT RESULTS IN A CHANGE IN THE NATURAL COVER OR TOPOGRAPHY THAT MAY CAUSE EROSION AND CONTRIBUTE TO SEDIMENTATION AND ALTER THE QUALITY AND QUANTITY OF STORMWATER RUNOFF."^^xsd:string ;
    rdfs:subClassOf epa-frs:WaterResourcesPrograms .

epa-frs:EthanolFacility a owl:Class ;
    rdfs:label "ETHANOL FACILITY"^^xsd:string ;
    dcterms:description "AN ETHANOL PRODUCER REGISTERED WITH THE RENEWABLE FUEL STANDARD (RFS) PROGRAM, INCLUDING REFINERS, IMPORTERS, AND BLENDERS. THE ENERGY POLICY ACT OF 2005 AMENDED THE CLEAN AIR ACT TO ESTABLISH THE RFS PROGRAM, WHICH IS DESIGNED TO ENCOURAGE BLENDING RENEWABLE FUELS INTO OUR NATION'S MOTOR VEHICLE FUEL. A RENEWABLE FUEL IS DEFINED IN THE ENERGY POLICY ACT AS A MOTOR VEHICLE FUEL THAT IS PRODUCED FROM PLANT OR ANIMAL PRODUCTS OR WASTES AND INCLUDES ETHANOL, BIODIESEL, AND OTHER MOTOR VEHICLE FUELS MADE FROM RENEWABLE SOURCES. "^^xsd:string ;
    rdfs:subClassOf epa-frs:AirPrograms .

epa-frs:EthanolFacilityGasolineAndDieselProducers a owl:Class ;
    rdfs:label "ETHANOL FACILITY/GASOLINE AND DIESEL PRODUCERS"^^xsd:string ;
    dcterms:description "EPA REGULATIONS REQUIRE THAT EACH MANUFACTURER OR IMPORTER OF GASOLINE DIESEL FUEL OR A FUEL ADDITIVE HAVE ITS PRODUCT REGISTERED PRIOR TO ITS INTRODUCTION INTO COMMERCE AND IN SOME CASES TESTED FOR POSSIBLE HEALTH EFFECTS. EPA ESTABLISHES FUEL QUALITY STANDARDS TO HELP PROTECT PUBLIC HEALTH AND THE ENVIRONMENT FROM HARMFUL GAS AND PARTICULATE MATTER EMISSIONS FROM MOTOR VEHICLES AND ENGINES IN ACCORDANCE WITH THE FEDERAL CLEAN AIR ACT (CAA). OVER THE YEARS THESE REGULATIONS HAVE INCLUDED THE REQUIREMENT FOR GASOLINE TO CONTAIN A CERTIFIED DETERGENT TO REDUCE EMISSIONS THE REMOVAL OF LEAD IN MOTOR VEHICLE GASOLINE VOLATILITY STANDARDS THE REFORMULATED GASOLINE (RFG) PROGRAM TO REDUCE EMISSIONS OF SMOG-FORMING AND TOXIC POLLUTANTS AND STANDARDS FOR TOXICS AND FOR LOW SULFUR GASOLINE."^^xsd:string ;
    rdfs:subClassOf epa-frs:AirPrograms .

epa-frs:FRP a owl:Class ;
    rdfs:label "FRP"^^xsd:string ;
    dcterms:description "THE OIL POLLUTION ACT AMENDED THE CLEAN WATER ACT TO REQUIRE A ¿SUBSTANTIAL HARM¿ FACILITY TO DEVELOP AND IMPLEMENT A FACILITY RESPONSE PLAN (FRP). A ¿SUBSTANTIAL HARM¿ FACILITY IS A FACILITY THAT, BECAUSE OF ITS LOCATION, COULD REASONABLY BE EXPECTED TO CAUSE SUBSTANTIAL HARM TO THE ENVIRONMENT BY DISCHARGING OIL INTO OR ON NAVIGABLE WATERS OR ADJOINING SHORELINES. A FRP DEMONSTRATES A FACILITY'S PREPAREDNESS TO RESPOND TO A WORST CASE OIL DISCHARGE."^^xsd:string ;
    rdfs:subClassOf epa-frs:ChemicalStoragePrograms .

epa-frs:Facility a owl:Class ;
    rdfs:label "FACILITY"^^xsd:string ;
    dcterms:description "A FEDERAL REGISTRY SYSTEM THAT MAINTAINS BASIC IDENTIFICATION INFORMATION FOR A FACILITY SITE, INCLUDING THE FACILITY REGISTRY IDENTIFIER, GEOGRAPHIC ADDRESS, AFFILIATED ORGANIZATIONS AND CONTACTS, INDUSTRIAL CLASSIFICATIONS, AND LINKAGES TO ENVIRONMENTAL PERMITS AND PROGRAMS."^^xsd:string ;
    rdfs:subClassOf epa-frs:FacilitySiteIdentification .

epa-frs:FederalFacilityHazardousWasteDocket a owl:Class ;
    rdfs:label "FEDERAL FACILITY HAZARDOUS WASTE DOCKET"^^xsd:string ;
    dcterms:description "THE FACILITY IS ON THE FEDERAL FACILITY HAZARDOUS WASTE COMPLIANCE DOCKET, WHICH IS A LISTING OF FEDERAL FACILITIES THAT ARE MANAGING OR HAVE MANAGED HAZARDOUS WASTE; OR HAVE HAD A RELEASE OF HAZARDOUS WASTE."^^xsd:string ;
    rdfs:subClassOf epa-frs:HazardousWastePrograms .

epa-frs:FloodplainManagement a owl:Class ;
    rdfs:label "FLOODPLAIN MANAGEMENT"^^xsd:string ;
    dcterms:description "FLOODPLAIN MANAGEMENT IS THE CORRECTIVE AND PREVENTATIVE MEASURES FOR REDUCING FLOOD DAMAGE. THESE MEASURES ARE ADOPTED BY STATE AND LOCAL GOVERNMENTS SO THAT THE CITIZENS IN THE COMMUNITY WILL BE ELIGIBLE TO PURCHASE FLOOD INSURANCE."^^xsd:string ;
    rdfs:subClassOf epa-frs:WaterResourcesPrograms .

epa-frs:FormalEnforcementAction a owl:Class ;
    rdfs:label "FORMAL ENFORCEMENT ACTION"^^xsd:string ;
    dcterms:description "A CIVIL JUDICIAL OR ADMINISTRATIVE ENFORCEMENT CASE UNDER AN ENVIRONMENTAL STATUTE."^^xsd:string ;
    rdfs:subClassOf epa-frs:LegalEnforcementActivities .

epa-frs:FormerlyUsedDefenseSite a owl:Class ;
    rdfs:label "FORMERLY USED DEFENSE SITE"^^xsd:string ;
    dcterms:description "THE DEPARTMENT OF DEFENSE (DOD) IS RESPONSIBLE FOR CLEANING UP PROPERTIES THAT WERE FORMERLY OWNED, LEASED POSSESSED, OR OPERATED BY DOD. THESE PROPERTIES ARE KNOWN AS FORMERLY USED DEFENSE SITES (FUDS). THE ARMY IS THE EXECUTIVE AGENT FOR THE PROGRAM AND THE U.S. ARMY CORPS OF ENGINEERS IS THE ORGANIZATION THAT MANAGES AND EXECUTES THE PROGRAM. INFORMATION ABOUT THE ORIGIN AND EXTENT OF CONTAMINATION, LAND TRANSFER ISSUES, PAST AND PRESENT PROPERTY OWNERSHIP, AND PROGRAM POLICIES MUST BE EVALUATED BEFORE DOD CONSIDERS A PROPERTY ELIGIBLE FOR DEFENSE ENVIRONMENT RESTORATION ACCOUNT (DERA) FUNDING UNDER THE FUDS PROGRAM.  "^^xsd:string ;
    rdfs:subClassOf epa-frs:RemediationAndRedevelopmentPrograms .

epa-frs:GasolineAndDieselProducers a owl:Class ;
    rdfs:label "GASOLINE AND DIESEL PRODUCERS"^^xsd:string ;
    dcterms:description "EPA REGULATIONS REQUIRE THAT EACH MANUFACTURER OR IMPORTER OF GASOLINE DIESEL FUEL OR A FUEL ADDITIVE HAVE ITS PRODUCT REGISTERED PRIOR TO ITS INTRODUCTION INTO COMMERCE AND IN SOME CASES TESTED FOR POSSIBLE HEALTH EFFECTS. EPA ESTABLISHES FUEL QUALITY STANDARDS TO HELP PROTECT PUBLIC HEALTH AND THE ENVIRONMENT FROM HARMFUL GAS AND PARTICULATE MATTER EMISSIONS FROM MOTOR VEHICLES AND ENGINES IN ACCORDANCE WITH THE FEDERAL CLEAN AIR ACT (CAA). OVER THE YEARS THESE REGULATIONS HAVE INCLUDED THE REQUIREMENT FOR GASOLINE TO CONTAIN A CERTIFIED DETERGENT TO REDUCE EMISSIONS THE REMOVAL OF LEAD IN MOTOR VEHICLE GASOLINE VOLATILITY STANDARDS THE REFORMULATED GASOLINE (RFG) PROGRAM TO REDUCE EMISSIONS OF SMOG-FORMING AND TOXIC POLLUTANTS AND STANDARDS FOR TOXICS AND FOR LOW SULFUR GASOLINE."^^xsd:string ;
    rdfs:subClassOf epa-frs:AirPrograms .

epa-frs:GrantsAndPlanning a owl:Class ;
    rdfs:label "GRANTS AND PLANNING"^^xsd:string ;
    dcterms:description "GRANTS FOR ENVIRONMENTAL PROGRAMS."^^xsd:string ;
    rdfs:subClassOf epa-frs:AssistanceAndSupportPrograms .

epa-frs:GreenhouseGasReporter a owl:Class ;
    rdfs:label "GREENHOUSE GAS REPORTER"^^xsd:string ;
    dcterms:description "GREENHOUSE GAS REPORTERS ARE REQUIRED TO ANNUALLY REPORT GREENHOUSE GASES (GHGS) FROM LARGE GHG EMISSION SOURCES IN THE UNITED STATES. IMPLEMENTATION OF 40 CFR PART 98 IS REFERRED TO AS THE GREENHOUSE GAS REPORTING PROGRAM (GHGRP) AND APPLIES TO DIRECT GHG EMITTERS, FOSSIL FUEL SUPPLIERS, INDUSTRIAL GAS SUPPLIERS, AND FACILITIES THAT INJECT CO2 UNDERGROUND FOR SEQUESTRATION OR OTHER REASONS. IN GENERAL, THE THRESHOLD FOR REPORTING IS 25,000 METRIC TONS OR MORE OF CARBON DIOXIDE (CO2) EQUIVALENT PER YEAR. REPORTING IS AT THE FACILITY LEVEL, EXCEPT FOR CERTAIN SUPPLIERS OF FOSSIL FUELS AND INDUSTRIAL GREENHOUSE GASES."^^xsd:string ;
    rdfs:subClassOf epa-frs:AirPrograms .

epa-frs:GroundWaterProgram a owl:Class ;
    rdfs:label "GROUND WATER PROGRAM"^^xsd:string ;
    dcterms:description "AN ENVIRONMENTAL PROGRAM/PERMIT DESIGNED TO PROTECT GROUND WATER.  A GROUND WATER DISCHARGE PERMIT CONTAINS THE LIMITATIONS AND REQUIREMENTS DEEMED NECESSARY TO PROTECT PUBLIC HEALTH AND MINIMIZE GROUND WATER POLLUTION.  GROUND WATER PERMITS MAY APPLY TO VARIOUS ACTIVITIES, SUCH AS:(A) THE DISPOSAL OF TREATED MUNICIPAL OR INDUSTRIAL WASTEWATER INTO GROUNDWATER VIA SPRAY IRRIGATION OR OTHER LAND-TREATMENT APPLICATIONS. (B) THE DISCHARGE OF POLLUTANTS GENERATED AS A RESULT OF RAIN WATER OR GROUND WATER PASSING THROUGH THE RUBBLE WASTE IN AN UNLINED DISPOSAL CELL AND SEEPING INTO GROUND WATER BENEATH THE LANDFILL. (C) THE DISPOSAL OF TREATED INDUSTRIAL WASTEWATER FROM OIL TERMINALS INTO GROUND WATER VIA INFILTRATION/PERCOLATION OR OTHER LAND-TREATMENT APPLICATIONS. (D) THE REMEDIATION OF GROUNDWATER FROM PETROLEUM CONTAMINATED GROUNDWATER SOURCES."^^xsd:string ;
    rdfs:subClassOf epa-frs:GroundWaterPrograms .

epa-frs:GroundwaterUse a owl:Class ;
    rdfs:label "GROUNDWATER USE"^^xsd:string ;
    dcterms:description "A STATE ENVIRONMENTAL PERMIT FOR GROUNDWATER WITHDRAWALS OR PROPOSED GROUNDWATER WITHDRAWALS IN EXCESS OF THREE (3) MILLION GALLONS IN ANY MONTH WITHIN DESIGNATED CAPACITY USE AREAS."^^xsd:string ;
    rdfs:subClassOf epa-frs:GroundWaterPrograms .

epa-frs:HapAreaSource a owl:Class ;
    rdfs:label "HAP AREA SOURCE"^^xsd:string ;
    dcterms:description "EPS"^^xsd:string ;
    rdfs:subClassOf epa-frs:ElectronicPermitSystem .

epa-frs:HapMajorSource a owl:Class ;
    rdfs:label "HAP MAJOR SOURCE"^^xsd:string ;
    dcterms:description "EPS"^^xsd:string ;
    rdfs:subClassOf epa-frs:ElectronicPermitSystem .

epa-frs:HazardousAirPollutantMajor a owl:Class ;
    rdfs:label "HAZARDOUS AIR POLLUTANT MAJOR"^^xsd:string ;
    dcterms:description "FACILITY IS MAJOR BASED UPON ONLY 40 CFR 70 MAJOR SOURCE DEFINITION PARAGRAPH 1 (10/25 TPY HAPS)."^^xsd:string ;
    rdfs:subClassOf epa-frs:AirPrograms .

epa-frs:HazardousAndCriteriaAirPollutantMajor a owl:Class ;
    rdfs:label "HAZARDOUS AND CRITERIA AIR POLLUTANT MAJOR"^^xsd:string ;
    dcterms:description "FACILITY MEETS BOTH PARAGRAPH 1 AND 2 OF 40 CFR 70 MAJOR SOURCE DEFINITIONS (10/25 TPY HAPS AND 100 TPY ANY CAP)"^^xsd:string ;
    rdfs:subClassOf epa-frs:AirPrograms .

epa-frs:HazardousAndO3NAAirMajor a owl:Class ;
    rdfs:label "HAZARDOUS AND O3 N/A AIR MAJOR"^^xsd:string ;
    dcterms:description "FACILITY MEETS BOTH PARAGRAPH 1 AND 3 OF 40 CFR 70 MAJOR SOURCE DEFINITIONS (10/25 TPY HAPS AND OZONE N/A AREA LESSER TONS FOR NOX OR VOC)."^^xsd:string ;
    rdfs:subClassOf epa-frs:AirPrograms .

epa-frs:HazardousSolidCdWasteLandfill a owl:Class ;
    rdfs:label "HAZARDOUS, SOLID & C&D WASTE LANDFILL"^^xsd:string ;
    dcterms:description "LANDFILL THAT IS PERMITTED TO ACCEPT ALL THREE TYPES OF WASTE: HAZARDOUS, SOLID & C&D WASTE."^^xsd:string ;
    rdfs:subClassOf epa-frs:SolidWastePrograms .

epa-frs:HazardousWasteBiennialReporter a owl:Class ;
    rdfs:label "HAZARDOUS WASTE BIENNIAL REPORTER"^^xsd:string ;
    dcterms:description "UNDER THE AUTHORITY OF SECTIONS 3002 AND 3004 OF THE RESOURCE CONSERVATION AND RECOVERY ACT OF 1976 (RCRA), AS AMENDED BY THE HAZARDOUS AND SOLID WASTE AMENDMENTS OF 1984 (HSWA), HAZARDOUS WASTE GENERATORS AND TREATMENT, STORAGE, AND DISPOSAL FACILITIES ARE REQUIRED TO REPORT TO THE EPA OR THE AUTHORIZED STATES, AT LEAST EVERY TWO YEARS, THE QUANTITIES, NATURE, AND DISPOSITION OF HAZARDOUS WASTE."^^xsd:string ;
    rdfs:subClassOf epa-frs:HazardousWastePrograms .

epa-frs:HazardousWasteLandfill a owl:Class ;
    rdfs:label "HAZARDOUS WASTE LANDFILL"^^xsd:string ;
    dcterms:description "LANDFILL THAT IS PERMITTED TO ACCEPT HAZARDOUS WASTE (RCRA SUBTITLE C)."^^xsd:string ;
    rdfs:subClassOf epa-frs:SolidWastePrograms .

epa-frs:HistoricPreservation a owl:Class ;
    rdfs:label "HISTORIC PRESERVATION"^^xsd:string ;
    dcterms:description "PROGRAMS THAT SUPPORT IDENTIFYING, PRESERVING, PROTECTING AND SUSTAINING HISTORIC AND ARCHAEOLOGICAL RESOURCES."^^xsd:string ;
    rdfs:subClassOf epa-frs:EcologyOperations .

epa-frs:ICIS-NPDESMajor a owl:Class ;
    rdfs:label "ICIS-NPDES MAJOR"^^xsd:string ;
    dcterms:description "FOR PUBLICLY OWNED TREATMENT WORKS (POTWS), MAJOR DISCHARGERS INCLUDE ALL FACILITIES WITH DESIGN FLOWS EQUAL TO OR GREATER THAN ONE MILLION GALLONS PER DAY, OR SERVE A POPULATION OF 10,000 OR MORE, OR CAUSE SIGNIFICANT WATER QUALITY IMPACTS. NON-POTW DISCHARGES ARE CLASSIFIED AS MAJOR FACILITIES ON THE BASIS OF THE NUMBER OF POINTS ACCUMULATED USING A RATING WORKSHEET, WHICH EVALUATES THE SIGNIFICANCE OF A FACILITY USING SEVERAL CRITERIA, INCLUDING TOXIC POLLUTANT POTENTIAL, FLOW VOLUME, AND WATER QUALITY FACTORS SUCH AS IMPAIRMENT OF THE RECEIVING WATER OR PROXIMITY OF THE DISCHARGE TO COASTAL WATERS. "^^xsd:string ;
    rdfs:subClassOf epa-frs:WasteWaterPrograms .

epa-frs:ICIS-NPDESMinor a owl:Class ;
    rdfs:label "ICIS-NPDES MINOR"^^xsd:string ;
    dcterms:description "A CLEAN WATER ACT (CWA) NATIONAL POLLUTANT DISCHARGE ELIMINATION SYSTEM (NPDES) MINOR DISCHARGER OF POLLUTANTS WITH A ¿PENDING¿ PERMIT."^^xsd:string ;
    rdfs:subClassOf epa-frs:WasteWaterPrograms .

epa-frs:ICIS-NPDESNon-Major a owl:Class ;
    rdfs:label "ICIS-NPDES NON-MAJOR"^^xsd:string ;
    dcterms:description "A CLEAN WATER ACT (CWA) NATIONAL POLLUTANT DISCHARGE ELIMINATION SYSTEM (NPDES) DISCHARGER OF POLLUTANTS INTO WATERS OF THE UNITED STATES THAT IS NOT DESIGNATED AS A MAJOR IS CONSIDERED A NON-MAJOR.  "^^xsd:string ;
    rdfs:subClassOf epa-frs:WasteWaterPrograms .

epa-frs:ICIS-NPDESUnpermitted a owl:Class ;
    rdfs:label "ICIS-NPDES UNPERMITTED"^^xsd:string ;
    dcterms:description "A FACILITY THAT IS UNPERMITTED, BUT DISCHARGING POLLUTANTS INTO WATERS OF THE UNITED STATES AND REGULATED UNDER THE CLEAN WATER ACT (CWA) NATIONAL POLLUTANT DISCHARGE ELIMINATION SYSTEM (NPDES). "^^xsd:string ;
    rdfs:subClassOf epa-frs:WasteWaterPrograms .

epa-frs:IhwCorrectiveAction a owl:Class ;
    rdfs:label "IHW CORRECTIVE ACTION"^^xsd:string ;
    dcterms:description "SITES SUBJECT TO ENFORCEABLE RCRA CORRECTIVE ACTION (CA) OBLIGATIONS. SITES INCLUDED ARE THOSE WITH ONGOING CA, AND ALSO THOSE WHERE CA IS STATUTORILY REQUIRED TO BE ADDRESSED (I.E., TSD FACILITIES), BUT HAS NOT YET BEEN IMPOSED."^^xsd:string ;
    rdfs:subClassOf epa-frs:HazardousWastePrograms .

epa-frs:Incinerator a owl:Class ;
    rdfs:label "INCINERATOR"^^xsd:string ;
    dcterms:description "A FURNACE FOR BURNING WASTE UNDER CONTROLLED CONDITIONS."^^xsd:string ;
    rdfs:subClassOf epa-frs:HazardousWastePrograms .

epa-frs:IndependentCleanup a owl:Class ;
    rdfs:label "INDEPENDENT CLEANUP"^^xsd:string ;
    dcterms:description "ANY REMEDIAL ACTION WITHOUT DEPARTMENT OVERSIGHT OR APPROVAL AND NOT UNDER AN ORDER OR DECREE. "^^xsd:string ;
    rdfs:subClassOf epa-frs:RemediationAndRedevelopmentPrograms .

epa-frs:IndustrialSites a owl:Class ;
    rdfs:label "INDUSTRIAL SITES"^^xsd:string ;
    dcterms:description "STATE ENVIRONMENTAL PROGRAMS RESPONSIBLE FOR PERMITTING, SITE INSPECTIONS, AND COMPLIANCE ISSUES THAT FOCUS ON THE COMPLEXITIES OF INDUSTRIAL SITES, WHICH COVER MULTI-MEDIA INTERESTS REGULATING AIR, WATER, HAZARDOUS WASTE, AND CLEANUP MANAGEMENT ACTIVITIES. INDUSTRIAL SITES INCLUDE ALUMINUM SMELTERS, OIL REFINERIES AND PULP AND PAPER MILLS."^^xsd:string ;
    rdfs:subClassOf epa-frs:SolidWastePrograms .

epa-frs:InfectiousWaste a owl:Class ;
    rdfs:label "INFECTIOUS WASTE"^^xsd:string ;
    dcterms:description "A COMPREHENSIVE STATE PROGRAM THAT MONITORS COMPLIANCE WITH INFECTIOUS WASTE MANAGEMENT REGULATIONS.  THE PROGRAM IS ACTIVELY INVOLVED IN THE REGISTRATION OF GENERATORS AND TRANSPORTERS OF INFECTIOUS WASTE.  INFECTIOUS WASTE GENERATORS ARE RESPONSIBLE FOR THE STORAGE, COLLECTION AND DISPOSAL OF THEIR INFECTIOUS WASTE, AND FOR ENSURING THAT THE WASTE IS TRANSPORTED OFF SITE FOR TREATMENT BY A REGISTERED TRANSPORTER AND DISPOSED OF AT A SITE OR FACILITY WHICH HAS ALL APPLICABLE PERMITS REQUIRED TO RECEIVE WASTE.  INFECTIOUS WASTE INCLUDES ANY WASTE ITEM FROM RESEARCH OR THE HEALTH CARE COMMUNITY IN THESE CATEGORIES:  SHARPS, MICROBIOLOGICALS, BLOOD AND BLOOD PRODUCTS, PATHOLOGICAL WASTE, ISOLATION WASTE AND CONTAMINATED ANIMAL WASTE."^^xsd:string ;
    rdfs:subClassOf epa-frs:HazardousWastePrograms .

epa-frs:InnocentOwnerOperatorProgram a owl:Class ;
    rdfs:label "INNOCENT OWNER/OPERATOR PROGRAM"^^xsd:string ;
    dcterms:description "THE INNOCENT OWNER/OPERATOR PROGRAM (IOP) IS A STATE PROGRAM WHICH PROVIDES A CERTIFICATE TO AN INNOCENT OWNER OR OPERATOR IF THEIR PROPERTY IS CONTAMINATED AS A RESULT OF A RELEASE OR MIGRATION OF CONTAMINANTS FROM A SOURCE OR SOURCES NOT LOCATED ON THE PROPERTY, AND THEY DID NOT CAUSE OR CONTRIBUTE TO THE SOURCE OR SOURCES OF CONTAMINATION. SIMILAR TO A VOLUNTARY CLEANUP PROGRAM, THE IOP CAN BE USED AS A REDEVELOPMENT TOOL OR AS A TOOL TO ADD VALUE TO A CONTAMINATED PROPERTY."^^xsd:string ;
    rdfs:subClassOf epa-frs:RemediationAndRedevelopmentPrograms .

epa-frs:LQG a owl:Class ;
    rdfs:label "LQG"^^xsd:string ;
    dcterms:description "HAZARDOUS WASTE LARGE QUANTITY GENERATORS GENERATE:  (A) 1,000 KG OR MORE OF HAZARDOUS WASTE DURING ANY CALENDAR MONTH; OR (B) MORE THAN 1 KG OF ACUTELY HAZARDOUS WASTE DURING ANY CALENDAR MONTH; OR (C) MORE THAN 100 KG OF ANY RESIDUE OR CONTAMINATED SOIL, WASTE OR OTHER DEBRIS RESULTING FROM THE CLEANUP OF A SPILL, INTO OR ON ANY LAND OR WATER, OF ACUTELY HAZARDOUS WASTE DURING ANY CALENDAR MONTH; OR (D) 1 KG OR LESS OF ACUTELY HAZARDOUS WASTE DURING ANY CALENDAR MONTH, AND ACCUMULATE MORE THAN 1 KG OF ACUTELY HAZARDOUS WASTE AT ANY TIME; OR (E) 100 KG OR LESS OF ANY RESIDUE OR CONTAMINATED SOIL, WASTE OR OTHER DEBRIS RESULTING FROM THE CLEANUP OF A SPILL, INTO OR ON ANY LAND OR WATER, OF ACUTELY HAZARDOUS WASTE DURING ANY CALENDAR MONTH, AND ACCUMULATED MORE THAN 100 KG OF THAT MATERIAL AT ANY TIME."^^xsd:string ;
    rdfs:subClassOf epa-frs:HazardousWastePrograms .

epa-frs:Laboratory a owl:Class ;
    rdfs:label "LABORATORY"^^xsd:string ;
    dcterms:description "A CERTIFICATION OFFERED TO LABORATORIES WISHING TO ANALYZE ENVIRONMENTAL SAMPLES.  THE SCOPE OF ACCREDITATION MAY COVER THE SAFE DRINKING WATER ACT, CLEAN WATER ACT, AND SOLID AND HAZARDOUS WASTES INCLUDING RCRA AND CERCLA REQUIREMENTS."^^xsd:string ;
    rdfs:subClassOf epa-frs:AssistanceAndSupportPrograms .

epa-frs:LaboratoryCertification a owl:Class ;
    rdfs:label "LABORATORY CERTIFICATION"^^xsd:string ;
    dcterms:description "A CERTIFICATION OFFERED TO LABORATORIES WISHING TO ANALYZE ENVIRONMENTAL SAMPLES.  THE SCOPE OF ACCREDITATION MAY COVER THE SAFE DRINKING WATER ACT, CLEAN WATER ACT, AND SOLID AND HAZARDOUS WASTES INCLUDING RCRA AND CERCLA REQUIREMENTS."^^xsd:string ;
    rdfs:subClassOf epa-frs:AssistanceAndSupportPrograms .

epa-frs:LandfillGas-LfgRecovery a owl:Class ;
    rdfs:label "LANDFILL GAS (LFG) RECOVERY"^^xsd:string ;
    dcterms:description "BECAUSE MUNICIPAL SOLID WASTE (MSW) LANDFILLS ARE THE THIRD-LARGEST SOURCE OF METHANE EMISSIONS IN THE UNITED STATES GENERATED BY HUMAN ACTIVITY AND BECAUSE THESE METHANE EMISSIONS REPRESENT A LOST OPPORTUNITY TO CAPTURE AND USE A SIGNIFICANT ENERGY RESOURCE, EPA LAUNCHED THE LANDFILL METHANE OUTREACH PROGRAM (LMOP) TO ENCOURAGE PRODUCTIVE REUSE. CREATIVE USE OF LANDFILL GAS (LFG) INCLUDES HEATING GREENHOUSES, PRODUCING ELECTRICITY AND HEAT IN COGENERATION APPLICATIONS, FIRING BRICK KILNS, SUPPLYING HIGH–BTU PIPELINE–QUALITY GAS, FUELING GARBAGE TRUCKS, AND PROVIDING FUEL TO CHEMICAL AND AUTOMOBILE MANUFACTURING. PROJECTS RANGE FROM SMALL–SCALE COMMUNITY–DRIVEN INITIATIVES TO MULTI–MILLION–DOLLAR PRIVATE INVESTMENTS. FOR MORE DETAILS ON SPECIFIC PROJECTS, SEE THE LMOP WEBSITE."^^xsd:string ;
    rdfs:subClassOf epa-frs:AirPrograms .

epa-frs:LeakingStorageTank a owl:Class ;
    rdfs:label "LEAKING STORAGE TANK"^^xsd:string ;
    dcterms:description "AN ENVIRONMENTAL PROGRAM THAT ADDRESSES LEAKING STORAGE TANKS OF PETROLEUM SUBSTANCES."^^xsd:string ;
    rdfs:subClassOf epa-frs:UndergroundStorageTankPrograms .

epa-frs:LeakingUndergroundStorageTank-Arra a owl:Class ;
    rdfs:label "LEAKING UNDERGROUND STORAGE TANK - ARRA"^^xsd:string ;
    dcterms:description "LEAKING UNDERGROUND STORAGE TANK RELEASES THAT ARE BEING TRACKED BY THE PERFORMANCE MEASURES ASSOCIATED WITH THE AMERICAN RECOVERY AND REINVESTMENT ACT (ARRA) OR FOR WHICH ARRA FUNDS ARE BEING SPENT"^^xsd:string ;
    rdfs:subClassOf epa-frs:UndergroundStorageTankPrograms .

epa-frs:LegalServices a owl:Class ;
    rdfs:label "LEGAL SERVICES"^^xsd:string ;
    dcterms:description "LEGAL SERVICES IN SUPPORT OF AN ENVIRONMENTAL PROGRAM. "^^xsd:string ;
    rdfs:subClassOf epa-frs:LegalEnforcementActivities .

epa-frs:LivestockWasteControl a owl:Class ;
    rdfs:label "LIVESTOCK WASTE CONTROL"^^xsd:string ;
    dcterms:description "A COMBINATION OF BMPS DESIGNED TO ADDRESS WATER QUALITY OR PUBLIC HEALTH PROBLEMS CAUSED BY AGRICULTURAL ACTIVITIES RELATED TO GRAZING AND ANIMAL PRODUCTION SUCH AS ANIMAL FEEDING OPERATIONS THAT ARE NOT SUBJECT TO THE CONCENTRATED ANIMAL FEEDING OPERATION (CAFO) REGULATIONS. ANIMAL WASTE INCLUDES THE FECAL AND URINARY WASTES OF LIVESTOCK AND POULTRY; PROCESS WATER (SUCH AS THAT FROM A MILKING PARLOR); AND THE FEED, BEDDING, LITTER, AND SOIL WITH WHICH THEY BECOME INTERMIXED. POLLUTANTS SUCH AS ORGANIC SOLIDS, SALTS, BACTERIA, VIRUSES, AND OTHER MICROORGANISMS, AND SEDIMENTS MIGHT BE CONTAINED IN ANIMAL WASTE TRANSPORTED BY RUNOFF WATER AND PROCESS WASTEWATER."^^xsd:string ;
    rdfs:subClassOf epa-frs:AnimalOperations .

epa-frs:LowLevelRadioactiveWaste a owl:Class ;
    rdfs:label "LOW LEVEL RADIOACTIVE WASTE"^^xsd:string ;
    dcterms:description "A FACILITY THAT ACCEPTS LOW-LEVEL RADIOACTIVE WASTE FOR DISPOSAL."^^xsd:string ;
    rdfs:subClassOf epa-frs:RadiationProtectionPrograms .

epa-frs:MaterialRecycling a owl:Class ;
    rdfs:label "MATERIAL RECYCLING"^^xsd:string ;
    dcterms:description "A FACILITY THAT RECOVERS MATERIALS FOR RECYCLING OR OTHER USE."^^xsd:string ;
    rdfs:subClassOf epa-frs:SolidWastePrograms .

epa-frs:MineGeneralPermit a owl:Class ;
    rdfs:label "MINE GENERAL PERMIT"^^xsd:string ;
    dcterms:description "A GENERAL MINE OPERATING PERMIT ISSUED FOR A SITE FIVE ACRES OR LESS AND LIMITED TO THE REMOVAL OF SAND/CLAY OR TOPSOIL."^^xsd:string ;
    rdfs:subClassOf epa-frs:SolidWastePrograms .

epa-frs:MineOperatingPermit a owl:Class ;
    rdfs:label "MINE OPERATING PERMIT"^^xsd:string ;
    dcterms:description "AN INDIVIDUAL MINE OPERATING PERMIT USED FOR OPERATIONS OF ANY SIZE OR MINERAL RESOURCE.  MINING IS DEFINED AS THE REMOVAL OF ORES FROM THE GROUND FOR SALE (I.E. GRANITE QUARRIES) OR FOR USE IN A BUSINESS (I.E. BRICK MANUFACTURING)."^^xsd:string ;
    rdfs:subClassOf epa-frs:SolidWastePrograms .

epa-frs:MineralExploration a owl:Class ;
    rdfs:label "MINERAL EXPLORATION"^^xsd:string ;
    dcterms:description "PERMITS TO CONDUCT DRILLING, DRIVING, BORING OR DIGGING OF ANY MINERAL EXPLORATION HOLE(S)."^^xsd:string ;
    rdfs:subClassOf epa-frs:GroundWaterPrograms .

epa-frs:MiningProgram a owl:Class ;
    rdfs:label "MINING PROGRAM"^^xsd:string ;
    dcterms:description "A PROGRAM THAT REGULATES THE MINING OF ORE, ROCK, OR OTHER SUBSTANCES AND ENSURES THE RECLAMATION OF LAND AFFECTED BY SURFACE AND UNDERGROUND MINING ACTIVITY AND REGULATION OF THE DEVELOPMENT OF THE MINES IN ORDER TO MAINTAIN THE INTEGRITY OF THE STATE¿S NATURAL RESOURCES."^^xsd:string ;
    rdfs:subClassOf epa-frs:SolidWastePrograms .

epa-frs:Multi-PermittedSite a owl:Class ;
    rdfs:label "MULTI-PERMITTED SITE"^^xsd:string ;
    dcterms:description "A SITE THAT HAS BEEN ISSUED PERMITS BY MORE THAN ONE STATE ENVIRONMENTAL PROGRAM."^^xsd:string ;
    rdfs:subClassOf epa-frs:EnvironmentalInterest .

epa-frs:NPDESGeneralPermit a owl:Class ;
    rdfs:label "NPDES GENERAL PERMIT"^^xsd:string ;
    dcterms:description "A NPDES GENERAL PERMIT COVERS MULTIPLE FACILITIES WITHIN A SPECIFIC CATEGORY AND WITHIN A SPECIFIC GEOGRAPHICAL OR GEOPOLITICAL AREA SUCH AS A CITY, COUNTY, DESIGNATED PLANNING AREA, SEWER DISTRICT, STATE HIGHWAY SYSTEM, STANDARD METROPOLITAN STATISTICAL AREA, OR URBANIZED AREA.  GENERAL PERMITS MAY BE WRITTEN TO COVER CATEGORIES OF POINT SOURCES HAVING COMMON ELEMENTS, SUCH AS STORM WATER POINT SOURCES, FACILITIES THAT DISCHARGE THE SAME TYPES OF WASTES OR ENGAGE IN THE SAME TYPES OF SLUDGE USE OR DISPOSAL PRACTICES, FACILITIES THAT INVOLVE THE SAME OR SUBSTANTIALLY SIMILAR TYPES OF OPERATIONS, FACILITIES THAT REQUIRE THE SAME EFFLUENT LIMITS, OPERATING CONDITIONS, OR STANDARDS FOR SEWAGE SLUDGE USE OR DISPOSAL, AND FACILITIES THAT REQUIRE THE SAME OR SIMILAR MONITORING."^^xsd:string ;
    rdfs:subClassOf epa-frs:WasteWaterPrograms .

epa-frs:NPDESMajor a owl:Class ;
    rdfs:label "NPDES MAJOR"^^xsd:string ;
    dcterms:description "A CLEAN WATER ACT (CWA) NATIONAL POLLUTANT DISCHARGE ELIMINATION SYSTEM (NPDES) MAJOR DISCHARGER OF POLLUTANTS INTO WATERS OF THE UNITED STATES."^^xsd:string ;
    rdfs:subClassOf epa-frs:WasteWaterPrograms .

epa-frs:NPDESNoExposureCertification a owl:Class ;
    rdfs:label "NPDES NO EXPOSURE CERTIFICATION"^^xsd:string ;
    dcterms:description "PROVIDES LIGHT INDUSTRIAL FACILITIES CONDITIONAL EXCLUSIONS FROM OBTAINING STORM WATER PERMITS BASED ON NO EXPOSURE OF INDUSTRIAL ACTIVITIES TO STORM WATER.  NO EXPOSURE MEANS ALL INDUSTRIAL MATERIALS AND ACTIVITIES ARE PROTECTED BY A STORM RESISTANT SHELTER TO PREVENT EXPOSURE TO RAIN, SNOW, SNOWMELT AND/OR RUNOFF."^^xsd:string ;
    rdfs:subClassOf epa-frs:WasteWaterPrograms .

epa-frs:NPDESNon-Major a owl:Class ;
    rdfs:label "NPDES NON-MAJOR"^^xsd:string ;
    dcterms:description "A CLEAN WATER ACT (CWA) NATIONAL POLLUTANT DISCHARGE ELIMINATION SYSTEM (NPDES) NON-MAJOR DISCHARGER OF POLLUTANTS INTO WATERS OF THE UNITED STATES."^^xsd:string ;
    rdfs:subClassOf epa-frs:WasteWaterPrograms .

epa-frs:NPDESPermit a owl:Class ;
    rdfs:label "NPDES PERMIT"^^xsd:string ;
    dcterms:description "A CLEAN WATER ACT (CWA) NATIONAL POLLUTANT DISCHARGE ELIMINATION SYSTEM (NPDES) PERMIT, WHICH ESTABLISHES POLLUTION LIMITS, AND SPECIFIES MONITORING AND REPORTING REQUIREMENTS FOR DISCHARGERS OF POLLUTANTS INTO WATERS OF THE UNITED STATES."^^xsd:string ;
    rdfs:subClassOf epa-frs:WasteWaterPrograms .

epa-frs:NPDESPretreatmentProgram a owl:Class ;
    rdfs:label "NPDES PRETREATMENT PROGRAM"^^xsd:string ;
    dcterms:description "THE PRETREATMENT PROGRAM, A COMPONENT OF THE CLEAN WATER ACT (CWA) NATIONAL POLLUTANT DISCHARGE ELIMINATION SYSTEM (NPDES), REQUIRES INDUSTRIAL AND COMMERCIAL DISCHARGERS TO TREAT OR CONTROL POLLUTANTS IN THEIR WASTEWATER PRIOR TO DISCHARGE TO PUBLICLY OWNED TREATMENT WORKS (POTWS)."^^xsd:string ;
    rdfs:subClassOf epa-frs:WasteWaterPrograms .

epa-frs:NPDESStormwaterPermit a owl:Class ;
    rdfs:label "NPDES STORMWATER PERMIT"^^xsd:string ;
    dcterms:description "THE STORM WATER PROGRAM, A COMPONENT OF THE CLEAN WATER ACT (CWA) NATIONAL POLLUTANT DISCHARGE ELIMINATION SYSTEM (NPDES), REQUIRES NPDES PERMITS FOR STORM WATER DISCHARGES FROM MUNICIPAL SEPARATE STORM SEWER SYSTEMS (MS4S), INDUSTRIES, AND CONSTRUCTIONS SITES."^^xsd:string ;
    rdfs:subClassOf epa-frs:WasteWaterPrograms .

epa-frs:NPDESUnpermitted a owl:Class ;
    rdfs:label "NPDES UNPERMITTED"^^xsd:string ;
    dcterms:description "A FACILITY THAT IS UNPERMITTED, BUT DISCHARGING POLLUTANTS INTO WATERS OF THE UNITED STATES AND REGULATED UNDER THE CLEAN WATER ACT (CWA) NATIONAL POLLUTANT DISCHARGE ELIMINATION SYSTEM (NPDES). "^^xsd:string ;
    rdfs:subClassOf epa-frs:WasteWaterPrograms .

epa-frs:NSRMajorSource a owl:Class ;
    rdfs:label "NSR MAJOR SOURCE"^^xsd:string ;
    dcterms:description "EPS"^^xsd:string ;
    rdfs:subClassOf epa-frs:ElectronicPermitSystem .

epa-frs:NSRSyntheticMinorSource a owl:Class ;
    rdfs:label "NSR SYNTHETIC MINOR SOURCE"^^xsd:string ;
    dcterms:description "EPS"^^xsd:string ;
    rdfs:subClassOf epa-frs:ElectronicPermitSystem .

epa-frs:NSRTrueMinorSource a owl:Class ;
    rdfs:label "NSR TRUE MINOR SOURCE"^^xsd:string ;
    dcterms:description "EPS"^^xsd:string ;
    rdfs:subClassOf epa-frs:ElectronicPermitSystem .

epa-frs:NavigableWaters a owl:Class ;
    rdfs:label "NAVIGABLE WATERS"^^xsd:string ;
    dcterms:description "A STATE PERMIT, ACONSTRUCTION IN NAVIGABLE WATERS@, MUST BE OBTAINED BEFORE COMMENCING ANY ACTIVITY, SUCH AS CONSTRUCTION, DREDGING, FILLING OR OTHER ALTERATIONS, BELOW THE MEAN HIGH WATER LINE (TIDAL WATERS) OR THE ORDINARY HIGH WATER MARK (NON-TIDAL WATERS) WITHIN A NAVIGABLE WATERWAY."^^xsd:string ;
    rdfs:subClassOf epa-frs:WaterResourcesPrograms .

epa-frs:Non-CommunityWaterSystem a owl:Class ;
    rdfs:label "NON-COMMUNITY WATER SYSTEM"^^xsd:string ;
    dcterms:description "A PUBLIC WATER SYSTEM THAT PIPES WATER FOR HUMAN CONSUMPTION TO AT LEAST 15 SERVICE CONNECTIONS USED BY INDIVIDUALS OTHER THAN YEAR-ROUND RESIDENTS OR AT LEAST 60 DAYS A YEAR, OR THAT SERVE 25 OR MORE PEOPLE AT LEAST 60 DAYS A YEAR (E.G., SCHOOLS, FACTORIES, REST AREAS)."^^xsd:string ;
    rdfs:subClassOf epa-frs:DrinkingWaterPrograms .

epa-frs:Non-TitleVSource a owl:Class ;
    rdfs:label "NON-TITLE V SOURCE"^^xsd:string ;
    dcterms:description "EPS"^^xsd:string ;
    rdfs:subClassOf epa-frs:ElectronicPermitSystem .

epa-frs:NotInAUniverse a owl:Class ;
    rdfs:label "NOT IN A UNIVERSE"^^xsd:string ;
    dcterms:description "THE HANDLER IS NOT CURRENTLY IN ANY HAZARDOUS WASTE UNIVERSE."^^xsd:string ;
    rdfs:subClassOf epa-frs:HazardousWastePrograms .

epa-frs:OSHAEstablishment a owl:Class ;
    rdfs:label "OSHA ESTABLISHMENT"^^xsd:string ;
    dcterms:description "THE ESTABLISHMENT HAS UNDERGONE AN INSPECTION BY A COMPLIANCE SAFETY AND HEALTH OFFICER WHOSE GOAL IS TO ASSURE COMPLIANCE WITH OCCUPATIONAL SAFETY AND HEALTH ADMINISTRATION (OSHA) REQUIREMENTS AND HELP EMPLOYERS AND WORKERS REDUCE ON-THE-JOB HAZARDS AND PREVENT INJURIES, ILLNESSES AND DEATHS IN THE WORKPLACE."^^xsd:string ;
    rdfs:subClassOf epa-frs:HealthAndSafetyPrograms .

epa-frs:OilAndGas a owl:Class ;
    rdfs:label "OIL AND GAS"^^xsd:string ;
    dcterms:description "AN ENVIRONMENTAL PROGRAM THAT ADDRESSES GAS AND OIL DRILLING MUDS, OIL PRODUCTION BRINES, AND OTHER WASTE ASSOCIATED WITH EXPLORATION FOR, DEVELOPMENT AND PRODUCTION OF CRUDE OIL OR NATURAL GAS."^^xsd:string ;
    rdfs:subClassOf epa-frs:WasteWaterPrograms .

epa-frs:OilControl a owl:Class ;
    rdfs:label "OIL CONTROL"^^xsd:string ;
    dcterms:description "AN ENVIRONMENTAL PROGRAM/PERMIT WHICH REGULATES THE STORAGE AND TRANSPORTATION OF OIL AND THE STORAGE AND TREATMENT OF OIL CONTAMINATED SOIL.  "^^xsd:string ;
    rdfs:subClassOf epa-frs:SolidWastePrograms .

epa-frs:OnsiteWastewaterTreatment a owl:Class ;
    rdfs:label "ONSITE WASTEWATER TREATMENT"^^xsd:string ;
    dcterms:description "AN ENVIRONMENTAL PROGRAM CONCERNED WITH THE DESIGN, OPERATION, AND MAINTENANCE OF SEPTIC TANK SYSTEMS."^^xsd:string ;
    rdfs:subClassOf epa-frs:WasteWaterPrograms .

epa-frs:OperatorCertification a owl:Class ;
    rdfs:label "OPERATOR CERTIFICATION"^^xsd:string ;
    dcterms:description "REGULATIONS RELATED TO THE CERTIFICATION OF WASTEWATER TREATMENT FACILITY OPERATORS. "^^xsd:string ;
    rdfs:subClassOf epa-frs:WasteWaterPrograms .

epa-frs:OtherHazardousWasteActivities a owl:Class ;
    rdfs:label "OTHER HAZARDOUS WASTE ACTIVITIES"^^xsd:string ;
    dcterms:description "THE HANDLER IS IN A HAZARDOUS WASTE UNIVERSE OTHER THAN TSD, GENERATOR (LQG, SQG, CESQG), TRANSPORTER, OR TRANSFER FACILITY. OTHER HAZARDOUS WASTE ACTIVITIES INCLUDE IMPORTERS OF HAZARDOUS WASTE, MIXED HAZARDOUS/ RADIOACTIVE WASTE GENERATORS, SMALL QUANTITY ON-SITE BURNER EXEMPTION SITES, SMELTING, MELTING, AND REFINING FURNACE EXEMPTION SITES, SHORT-TERM GENERATORS, UNDERGROUND INJECTION CONTROL SITES, OFF-SITE RECEIVER OF HAZARDOUS WASTE, RECYCLER, OR UNIVERSAL WASTE HANDLER."^^xsd:string ;
    rdfs:subClassOf epa-frs:HazardousWastePrograms .

epa-frs:ParksAndForestry a owl:Class ;
    rdfs:label "PARKS AND FORESTRY"^^xsd:string ;
    dcterms:description "PROGRAMS THAT MONITOR INDIVIDUALS LICENSED IN THE FIELDS OF PARKS AND FORESTRY"^^xsd:string ;
    rdfs:subClassOf epa-frs:EcologyOperations .

epa-frs:PesticideProducer a owl:Class ;
    rdfs:label "PESTICIDE PRODUCER"^^xsd:string ;
    dcterms:description "AN ESTABLISHMENT THAT PRODUCES PESTICIDES, ACTIVE INGREDIENTS OR DEVICES, INCLUDING IMPORTERS, MUST REGISTER AND FILE PRODUCTION REPORTS WITH EPA, AS REQUIRED UNDER SECTION 7 OF THE FEDERAL INSECTICIDE, FUNGICIDE, AND RODENTICIDE ACT (FIFRA)."^^xsd:string ;
    rdfs:subClassOf epa-frs:PesticidesPrograms .

epa-frs:Pesticides-Application a owl:Class ;
    rdfs:label "PESTICIDES - APPLICATION"^^xsd:string ;
    dcterms:description "ANY PERSON OR ENTITY WHO APPLIES PESTICIDES FOR ANY PURPOSE. ANY PERSON WHO USES, OR SUPERVISES THE USE, OF PESTICIDES ON A \"FOR HIRE\" BASIS*, NO MATTER WHAT FOR. ALSO, ANY PERSON WHO APPLIES PESTICIDES AS PART OF HIS JOB WITH ANY GOVERNMENTAL AGENCY. EXAMPLES OF COMMERCIAL APPLICATORS ARE THOSE WHO WORK FOR EXTERMINATORS; LANDSCAPERS; TREE SERVICES; AERIAL APPLICATORS; WEED CONTROL FIRMS; PET GROOMERS, APARTMENTS, MOTELS, NURSING HOMES, RESTAURANTS, ETC. WHO DO THEIR OWN PEST CONTROL WORK; AND GOVERNMENTAL AGENCIES SUCH AS MOSQUITO EXTERMINATION COMMISSIONS, PUBLIC SCHOOLS, DEPARTMENTS OF PUBLIC WORKS, DEPARTMENTS OF HEALTH, THE DOT, ETC."^^xsd:string ;
    rdfs:subClassOf epa-frs:PesticidesPrograms .

epa-frs:Pesticides-Distribution a owl:Class ;
    rdfs:label "PESTICIDES - DISTRIBUTION"^^xsd:string ;
    dcterms:description "A PESTICIDE DEALER BUSINESS IS DEFINED AS ANY PERSON OR ORGANIZATION WHICH ULTIMATELY CONTROLS THE TRANSACTIONS CONDUCTED AT, AND THE OPERATIONS OF, APESTICIDE DEALER OUTLET."^^xsd:string ;
    rdfs:subClassOf epa-frs:PesticidesPrograms .

epa-frs:Pesticides-General a owl:Class ;
    rdfs:label "PESTICIDES - GENERAL"^^xsd:string ;
    dcterms:description "A PROGRAM THAT MONITORS AN ASPECT OF PESITICIDES."^^xsd:string ;
    rdfs:subClassOf epa-frs:PesticidesPrograms .

epa-frs:Pesticides-Manufacture a owl:Class ;
    rdfs:label "PESTICIDES - MANUFACTURE"^^xsd:string ;
    dcterms:description "A PESTICIDE PRODUCER IS A BUSINESS THAT CREATES OR PROCESSES PESTICIDES TO BE SOLD TO PESTICIDE APPLICATION ENTITIES."^^xsd:string ;
    rdfs:subClassOf epa-frs:PesticidesPrograms .

epa-frs:PhaseIIMs4 a owl:Class ;
    rdfs:label "PHASE II MS4"^^xsd:string ;
    dcterms:description "A COMBINATION OF UNIT PROCESSES OR BMPS DESIGNED TO COLLECT, TREAT, AND TRANSPORT STORMWATER FOR ENTITIES REGULATED UNDER THE NPDES PHASE II PERMIT PROCESS. PHASE II PERMITS WERE REQUIRED FOR SMALL MS4S (POPULATION 99,999 OR LESS) LOCATED IN \"URBANIZED AREAS\" (UAS) AS DEFINED BY THE BUREAU OF THE CENSUS, AND THOSE SMALL MS4S LOCATED OUTSIDE OF A UA THAT ARE DESIGNATED BY NPDES PERMITTING AUTHORITIES."^^xsd:string ;
    rdfs:subClassOf epa-frs:EnvironmentalInterest .

epa-frs:PostClosureCareSite a owl:Class ;
    rdfs:label "POST CLOSURE CARE SITE"^^xsd:string ;
    dcterms:description "THE TIME PERIOD FOLLOWING THE SHUTDOWN OF A WASTE MANAGEMENT OR MANUFACTURING FACILITY; FOR MONITORING PURPOSES, OFTEN CONSIDERED TO BE 30 YEARS."^^xsd:string ;
    rdfs:subClassOf epa-frs:HazardousWastePrograms .

epa-frs:RadNESHAPS a owl:Class ;
    rdfs:label "RAD NESHAPS"^^xsd:string ;
    dcterms:description "AN ENVIRONMENTAL PROGRAM, THE NATIONAL EMISSIONS STANDARDS FOR HAZARDOUS AIR POLLUTANTS (NESHAPS) THAT INCLUDES STANDARDS FOR LIMITING THE RADIONUCLIDE EMISSIONS TO AIR. THESE STANDARDS ARE PUBLISHED IN THE CODE OF FEDERAL REGULATIONS (CFR) AT 40 CFR PART 61. STANDARDS FOR SPECIFIC SOURCES OF RADIONUCLIDE EMISSIONS ARE CONTAINED IN THE FOLLOWING SUBPARTS OF PART 61:  SUBPART B UNDERGROUND URANIUM MINES; SUBPART H DEPARTMENT OF ENERGY FACILITIES; SUBPART I CERTAIN NON-DOE FEDERAL FACILITIES; SUBPART K ELEMENTAL PHOSPHATE PLANTS; SUBPART Q DOE FACILITIES RADON EMISSIONS; SUBPART R RADON FROM PHOSPHOGYPSUM STACKS; SUBPART T NON-OPERATIONAL URANIUM MILL TAILING PILES; SUBPART W OPERATING URANIUM MILL TAILING PILES."^^xsd:string ;
    rdfs:subClassOf epa-frs:RadiationProtectionPrograms .

epa-frs:RadNPL a owl:Class ;
    rdfs:label "RAD NPL"^^xsd:string ;
    dcterms:description "A CERCLA NATIONAL PRIORITY LIST (NPL) SITE WITH RADIOACTIVE CONTAMINATION.  THE REGULATIONS ARE PUBLISHED IN THE CODE OF FEDERAL REGULATIONS (CFR) AT 40 CFR PART 300. "^^xsd:string ;
    rdfs:subClassOf epa-frs:RadiationProtectionPrograms .

epa-frs:RadWIPP a owl:Class ;
    rdfs:label "RAD WIPP"^^xsd:string ;
    dcterms:description "AN EPA PROGRAM THAT OVERSEES THE U.S. DEPARTMENT OF ENERGY¿S (DOE) ACTIVITIES AT THE WASTE ISOLATION PILOT PLANT (WIPP). THE REGULATIONS FOR RADIOACTIVE WASTE DISPOSAL ARE PUBLISHED IN THE CODE OF FEDERAL REGULATIONS (CFR) AT 40 CFR PART 191. THE CRITERIA DEVELOPED BY THE EPA THAT DESCRIBE THE INFORMATION DOE MUST SUBMIT IN A CERTIFICATION APPLICATION ARE PUBLISHED AT 40 CFR 194. "^^xsd:string ;
    rdfs:subClassOf epa-frs:RadiationProtectionPrograms .

epa-frs:RadioactiveMaterials a owl:Class ;
    rdfs:label "RADIOACTIVE MATERIALS"^^xsd:string ;
    dcterms:description "A STATE DELEGATED PROGRAM, IN PARTNERSHIP WITH THE U.S. NUCLEAR REGULATORY COMMISSION, RESPONSIBLE FOR LICENSING AND INSPECTING FACILITIES THAT POSSESS AND USE RADIOACTIVE MATERIAL, FROM MEDICAL INSTITUTIONS WHERE HEALTH PROFESSIONS USE RADIOACTIVE MATERIALS FOR BOTH DIAGNOSTIC AND THERAPEUTIC PURPOSES TO INDUSTRIAL GAUGES WHERE USES RANGE FROM PRODUCT STERILIZATION TO THE LEVEL AND DENSITY MEASUREMENTS OF VARIOUS CONSTRUCTION MATERIALS."^^xsd:string ;
    rdfs:subClassOf epa-frs:RadiationProtectionPrograms .

epa-frs:RadioactiveWaste a owl:Class ;
    rdfs:label "RADIOACTIVE WASTE"^^xsd:string ;
    dcterms:description "A STATE DELEGATED RADIOACTIVE WASTE MANAGEMENT PROGRAM.  STATES RECEIVE DELEGATED RESPONSIBILITIES FROM THE U.S. NUCLEAR REGULATORY COMMISSION FOR THE REGULATORY OVERSIGHT AND LICENSING OF THE PROCESSING, TRANSPORTATION, MANAGEMENT, AND DISPOSAL OF LOW LEVEL RADIOACTIVE WASTE AND RADIOACTIVE MATERIAL PRODUCTION; THE INSPECTION OF HIGH LEVEL, TRANSURANIC, AND SPENT FUEL SHIPMENTS; RELATED ENFORCEMENT ACTIVITIES; AND RADIOLOGICAL TECHNICAL ASSISTANCE."^^xsd:string ;
    rdfs:subClassOf epa-frs:RadiationProtectionPrograms .

epa-frs:RefuseDisposal a owl:Class ;
    rdfs:label "REFUSE DISPOSAL"^^xsd:string ;
    dcterms:description "A PERMIT/PROGRAM TO ENSURE THE PROPER DISPOSAL OF SOLID WASTE IN AN ENVIRONMENTALLY ACCEPTABLE MANNER WHILE PROTECTING PUBLIC HEALTH AND THE ENVIRONMENT. REFUSE DISPOSAL SYSTEMS INCLUDE:MUNICIPAL LANDFILLS, LAND CLEARING LANDFILLS, INDUSTRIAL LANDFILLS, RUBBLE LANDFILLS, MUNICIPAL AND SPECIAL MEDICAL WASTES INCINERATORS, WASTE TRANSFER STATIONS, AND WASTE PROCESSING FACILITIES.  "^^xsd:string ;
    rdfs:subClassOf epa-frs:SolidWastePrograms .

epa-frs:ReleaseAssessment a owl:Class ;
    rdfs:label "RELEASE ASSESSMENT"^^xsd:string ;
    dcterms:description "AN ENVIRONMENTAL PROGRAM THAT RECEIVES NOTIFICATION OF SPILLS, LEAKS, AND OTHER ENVIRONMENTAL EMERGENCIES, AND PROVIDES TECHNICAL ASSISTANCE AND REGULATORY OVERSIGHT TO THOSE THAT POSE AN IMMEDIATE HAZARD TO EITHER THE ENVIRONMENT OR PUBLIC HEALTH."^^xsd:string ;
    rdfs:subClassOf epa-frs:ChemicalReleasePrograms .

epa-frs:RemedialActionPlanMonitoring a owl:Class ;
    rdfs:label "REMEDIAL ACTION PLAN MONITORING"^^xsd:string ;
    dcterms:description "THE REMEDIAL ACTION PLAN MONITORING ACT (RAPMA) PROVIDES BUSINESSES (I.E., PROPERTY OWNERS OR OTHER PARTIES RESPONSIBLE FOR CONTAMINATION) WITH A MECHANISM FOR DEVELOPING VOLUNTARY ENVIRONMENTAL CLEANUP PLANS WHICH ARE REVIEWED/APPROVED BY THE STATE."^^xsd:string ;
    rdfs:subClassOf epa-frs:RemediationAndRedevelopmentPrograms .

epa-frs:RemediationAndRedevelopmentPrograms-SuperfundNPL a owl:Class ;
    rdfs:label "REMEDIATION AND REDEVELOPMENT PROGRAMS: SUPERFUND NPL"^^xsd:string ;
    dcterms:description "A SUPERFUND SITE WHICH IS LISTED, PROPOSED, OR PREVIOUSLY LISTED ON THE NATIONAL PRIORITIES LIST (NPL).  THE NPL LISTS NATIONAL PRIORITIES AMONG THE KNOWN RELEASES OR THREATENED RELEASES OF HAZARDOUS SUBSTANCES, POLLUTANTS, OR CONTAMINANTS THROUGHOUT THE UNITED STATES."^^xsd:string ;
    rdfs:subClassOf epa-frs:RemediationAndRedevelopmentPrograms .

epa-frs:RemediationFundingSource a owl:Class ;
    rdfs:label "REMEDIATION FUNDING SOURCE"^^xsd:string ;
    dcterms:description "REGULATIONS WHICH REQUIRE THE ESTABLISHMENT OF A REMEDIATION FUNDING SOURCE (RFS) BY CERTAIN OBLIGATED PARTIES REMEDIATING SITES UNDER A STATE SITE REMEDIATION PROGRAM TO ENSURE THE AVAILABILITY OF FUNDS AND TO ENSURE PUBLIC FUNDS ARE NOT SPENT IN REMEDIATING THESE SITES."^^xsd:string ;
    rdfs:subClassOf epa-frs:RemediationAndRedevelopmentPrograms .

epa-frs:ResidualWaste a owl:Class ;
    rdfs:label "RESIDUAL WASTE"^^xsd:string ;
    dcterms:description "THE AMOUNT OF A POLLUTANT REMAINING IN THE ENVIRONMENT AFTER A NATURAL OR TECHNOLOGICAL PROCESS HAS TAKEN PLACE (E.G., THE SLUDGE REMAINING AFTER INITIAL WASTEWATER TREATMENT)."^^xsd:string ;
    rdfs:subClassOf epa-frs:HazardousWastePrograms .

epa-frs:RmpReporter a owl:Class ;
    rdfs:label "RMP REPORTER"^^xsd:string ;
    dcterms:description "UNDER SECTION 112(R) OF THE CLEAN AIR ACT, A FACILITY THAT USES CERTAIN FLAMMABLE AND TOXIC SUBSTANCES MUST DEVELOP A RISK MANAGEMENT PLAN, WHICH INCLUDES INFORMATION ABOUT THE RISK MANAGEMENT PROGRAMS THAT MUST BE IMPLEMENTED TO PREVENT AND PREPARE FOR CHEMICAL ACCIDENTS."^^xsd:string ;
    rdfs:subClassOf epa-frs:ChemicalStoragePrograms .

epa-frs:SPCC a owl:Class ;
    rdfs:label "SPCC"^^xsd:string ;
    dcterms:description "ORIGINALLY PUBLISHED IN 1973 UNDER THE AUTHORITY OF THE CLEAN WATER ACT, THE OIL POLLUTION PREVENTION REGULATION SETS FORTH REQUIREMENTS FOR PREVENTION OF, PREPAREDNESS FOR, AND RESPONSE TO OIL DISCHARGES AT SPECIFIC NON-TRANSPORTATION-RELATED FACILITIES. TO PREVENT OIL FROM REACHING NAVIGABLE WATERS AND ADJOINING SHORELINES, AND TO CONTAIN DISCHARGES OF OIL, THE REGULATION REQUIRES THESE FACILITIES TO DEVELOP AND IMPLEMENT SPILL PREVENTION, CONTROL, AND COUNTERMEASURE (SPCC) PLANS AND ESTABLISHES PROCEDURES, METHODS, AND EQUIPMENT REQUIREMENTS."^^xsd:string ;
    rdfs:subClassOf epa-frs:ChemicalStoragePrograms .

epa-frs:SQG a owl:Class ;
    rdfs:label "SQG"^^xsd:string ;
    dcterms:description "HAZARDOUS WASTE SMALL QUANTITY GENERATORS GENERATE:  (A)  MORE THAN 100 AND LESS THAN 1000 KILOGRAMS OF HAZARDOUS WASTE DURING ANY CALENDAR MONTH AND ACCUMULATE LESS THAN 6000 KG OF HAZARDOUS WASTE AT ANY TIME; OR (B)  100 KG OR LESS OF HAZARDOUS WASTE DURING ANY CALENDAR MONTH, AND ACCUMULATE MORE THAN 1000 KG OF HAZARDOUS WASTE AT ANY TIME."^^xsd:string ;
    rdfs:subClassOf epa-frs:HazardousWastePrograms .

epa-frs:SW a owl:Class ;
    rdfs:label "SW"^^xsd:string ;
    dcterms:description "None"^^xsd:string ;
    rdfs:subClassOf epa-frs:EnvironmentalInterest .

epa-frs:SanitaryLandfills a owl:Class ;
    rdfs:label "SANITARY LANDFILLS"^^xsd:string ;
    dcterms:description "A COMBINATION OF BEST MANAGEMENT PRACTICES (BMPS) DESIGNED TO ADDRESS WATER QUALITY OR PUBLIC HEALTH PROBLEMS AT SANITARY LANDFILLS. SANITARY LANDFILLS ARE LANDFILLS DESIGNED AS DISPOSAL SITES FOR NONHAZARDOUS SOLID WASTES RATHER THAN HAZARDOUS SOLID WASTE OR BIOSOLIDS."^^xsd:string ;
    rdfs:subClassOf epa-frs:WasteWaterPrograms .

epa-frs:ScrapTireManagement a owl:Class ;
    rdfs:label "SCRAP TIRE MANAGEMENT"^^xsd:string ;
    dcterms:description "A SCRAP TIRE MANAGEMENT PROGRAM RELATED TO THE TRANSPORTATION, COLLECTION, PROCESSING, RECYCLING, DISPOSAL, INCINERATION OR UTILIZATION OF SCRAP TIRES AS TIRE DERIVED FUEL (TDF).  LICENSES OR APPROVALS MAY BE REQUIRED FOR:(A) SCRAP TIRE HAULERS -  COMMERCIAL BUSINESSES WHICH TRANSPORT SCRAP TIRES. (B) SCRAP TIRE COLLECTION FACILITIES - FACILITIES WHICH COLLECT OR ACCUMULATE SCRAP TIRES TEMPORARILY AND TRANSFER THE TIRES TO OTHER LICENSED OR APPROVED SCRAP TIRE FACILITIES. (C) SCRAP TIRE RECYCLERS -  FACILITIES THAT RECYCLE OR PROCESS SCRAP TIRES INTO RAW MATERIALS OR MARKETABLE PRODUCTS. (D) TIRE DERIVED FUEL OR SUBSTITUTE FUEL FACILITIES - FACILITIES WHICH UTILIZE SCRAP TIRES (WHOLE OR CHIPPED) AS A FUEL OR SUPPLEMENTAL FUEL. (E) SOLID WASTE ACCEPTANCE FACILITIES - PERMITTED SOLID WASTE ACCEPTANCE FACILITIES THAT ACCEPT, STORE, USE IN A PROCESS, OR TRANSFER SCRAP TIRES TO OTHER LICENSED APPROVED TIRE FACILITIES."^^xsd:string ;
    rdfs:subClassOf epa-frs:SolidWastePrograms .

epa-frs:Section404Permitting a owl:Class ;
    rdfs:label "SECTION 404 PERMITTING"^^xsd:string ;
    dcterms:description "SECTION 404 OF THE CLEAN WATER ACT (CWA) ESTABLISHES A PROGRAM TO REGULATE THE DISCHARGE OF DREDGED OR FILL MATERIAL INTO WATERS OF THE UNITED STATES, INCLUDING WETLANDS. ACTIVITIES IN WATERS OF THE UNITED STATES REGULATED UNDER THIS PROGRAM INCLUDE FILL FOR DEVELOPMENT, WATER RESOURCE PROJECTS (SUCH AS DAMS AND LEVEES), INFRASTRUCTURE DEVELOPMENT (SUCH AS HIGHWAYS AND AIRPORTS) AND MINING PROJECTS. SECTION 404 REQUIRES A PERMIT BEFORE DREDGED OR FILL MATERIAL MAY BE DISCHARGED INTO WATERS OF THE UNITED STATES, UNLESS THE ACTIVITY IS EXEMPT FROM SECTION 404 REGULATION (E.G. CERTAIN FARMING AND FORESTRY ACTIVITIES)."^^xsd:string ;
    rdfs:subClassOf epa-frs:WasteWaterPrograms .

epa-frs:Sediments a owl:Class ;
    rdfs:label "SEDIMENTS"^^xsd:string ;
    dcterms:description "A SEDIMENT SITE IS A LOCATION OF INTEREST AT WHICH SEDIMENT CHEMICAL AND/OR BIOLOGICAL DATA HAS BEEN OBTAINED AND EVALUATED FOR POTENTIAL IMPACTS TO HUMAN HEALTH OR THE ENVIRONMENT.   SEDIMENT SITES MAY EXIST BENEATH OR BE ASSOCIATED WITH FRESHWATER, MARINE AND ESTUARINE BODIES OF WATER.   SEDIMENT SITES MAY OR MAY NOT BE LINKED TO A KNOWN LAND-BASED FACILITY."^^xsd:string ;
    rdfs:subClassOf epa-frs:RemediationAndRedevelopmentPrograms .

epa-frs:SewageSludgeUtilization a owl:Class ;
    rdfs:label "SEWAGE SLUDGE UTILIZATION"^^xsd:string ;
    dcterms:description "A SEWAGE SLUDGE UTILIZATION PERMIT IS REQUIRED FOR THE COLLECTION, INCINERATION, STORAGE, TREATMENT, APPLICATION TO LAND, TRANSPORTATION OR DISPOSAL OF SEWAGE SLUDGE.  SEWAGE SLUDGE IS ONE OF THE FINAL PRODUCTS OF THE TREATMENT OF SEWAGE AT A SEWAGE (WASTEWATER) TREATMENT PLANT. AFTER TREATMENT TO BREAK DOWN THE ORGANIC MATTER AND DESTROY DISEASE ORGANISMS, THE REMAINING FINE PARTICLES ULTIMATELY BECOME SLUDGE. THE APPLICATION OF SEWAGE SLUDGE TO LAND RETURNS ESSENTIAL NUTRIENTS TO THE SOIL, ADDS ORGANIC MATTER, AND CAN IMPROVE THE TILLABILTY AND MOISTURE RETENTION CAPABILITY OF THE SOIL."^^xsd:string ;
    rdfs:subClassOf epa-frs:SolidWastePrograms .

epa-frs:Silviculture a owl:Class ;
    rdfs:label "SILVICULTURE"^^xsd:string ;
    dcterms:description "A COMBINATION OF BEST MANAGEMENT PRACTICES (BMPS) DESIGNED TO ADDRESS WATER QUALITY OR PUBLIC HEALTH PROBLEMS CAUSED BY FORESTRY ACTIVITIES SUCH AS REMOVAL OF STREAMSIDE VEGETATION, ROAD CONSTRUCTION AND USE, TIMBER HARVESTING, AND SITE PREPARATION FOR THE PLANTING OF TREES. SEDIMENT FROM EROSION DUE TO TREE HARVESTING ACTIVITIES AND ACCESS ROAD CONSTRUCTION, TEMPERATURE INCREASES DUE TO RIPARIAN SHADE REMOVAL, AND PESTICIDES AND FERTILIZER USED DURING TIMBER OPERATIONS ARE SOME OF THE MAJOR POLLUTANTS FROM TIMBER HARVESTING SITES. SILVICULTURE BMPS INCLUDE MEASURES THAT CONTROL EROSION FROM ACCESS ROADS, MAINTAIN THE STABILITY OF STREAM BANKS, ENSURE THE REVEGETATION OF HARVESTED AREAS, AND CONTROL THE INTRODUCTION OF PESTICIDES AND FERTILIZERS INTO WATERWAYS."^^xsd:string ;
    rdfs:subClassOf epa-frs:WasteWaterPrograms .

epa-frs:SolidCdWasteLandfill a owl:Class ;
    rdfs:label "SOLID & C&D WASTE LANDFILL"^^xsd:string ;
    dcterms:description "LANDFILL THAT ACCEPTS BOTH SOLID WASTE AND C&D WASTE (NOT EVERY STATE PERMITS SEPARATELY FOR C&D)."^^xsd:string ;
    rdfs:subClassOf epa-frs:SolidWastePrograms .

epa-frs:SolidWasteLandfill a owl:Class ;
    rdfs:label "SOLID WASTE LANDFILL"^^xsd:string ;
    dcterms:description "LANDFILL THAT IS PERMITTED TO ACCEPT SOLID WASTE (RCRA SUBTITLE D)."^^xsd:string ;
    rdfs:subClassOf epa-frs:SolidWastePrograms .

epa-frs:SolidWasteProgram a owl:Class ;
    rdfs:label "SOLID WASTE PROGRAM"^^xsd:string ;
    dcterms:description "ENVIRONMENTAL PROGRAMS THAT REGULATE SOLID WASTES (E.G., COMPOST SITES, LANDFILLS, TRANSFER STATIONS)"^^xsd:string ;
    rdfs:subClassOf epa-frs:SolidWastePrograms .

epa-frs:StateCleanupSite a owl:Class ;
    rdfs:label "STATE CLEANUP SITE"^^xsd:string ;
    dcterms:description "A CONTAMINATED SITE THAT IS BEING CLEANED UP UNDER STATE REGULATIONS. LAND-BASED CONTAMINATION IS THE PRIMARY BUT NOT EXCLUSIVE FOCUS. CONTAMINATED SITES RANGE FROM COMPLEX, HIGHLY INDUSTRIALIZED AREAS SUCH AS SMELTER PLUMES COVERING HUNDREDS OF SQUARE MILES, SEA PORTS, AND ABANDONED MINES, TO CORNER GAS STATIONS WHERE A LEAK FROM AN UNDERGROUND STORAGE TANK HAS OCCURRED. THE CONTAMINATION MAY BE IN THE SOIL, SEDIMENTS, UNDERGROUND WATER, AIR, DRINKING WATER, AND/OR SURFACE WATER. CLEANUP SITES ARE IDENTIFIED, EVALUATED, AND PRIORITIZED WITH THE GOAL OF HABITAT RESTORATION, REPLACEMENT, OR ENHANCEMENT BASED ON COMMUNITY SUSTAINABILITY PRINCIPALS. "^^xsd:string ;
    rdfs:subClassOf epa-frs:RemediationAndRedevelopmentPrograms .

epa-frs:StateMaster a owl:Class ;
    rdfs:label "STATE MASTER"^^xsd:string ;
    dcterms:description "A STATE REGISTRY SYSTEM THAT MAINTAINS BASIC IDENTIFICATION INFORMATION FOR A FACILITY SITE, INCLUDING THE STATE MASTER IDENTIFIER, GEOGRAPHIC ADDRESS, AFFILIATED ORGANIZATIONS AND CONTACTS, INDUSTRIAL CLASSIFICATIONS, AND LINKAGES TO ENVIRONMENTAL PERMITS AND PROGRAMS. "^^xsd:string ;
    rdfs:subClassOf epa-frs:FacilitySiteIdentification .

epa-frs:StateRegulatedTSD a owl:Class ;
    rdfs:label "STATE REGULATED TSD"^^xsd:string ;
    dcterms:description "STATE REGULATED TREATMENT, STORAGE, OR DISPOSAL ACTIVITIES (TSDS) ARE STATE-PERMITTED TSD ACTIVITIES NOT SUBJECT TO FEDERAL RCRA PERMIT REQUIREMENTS. SUCH ACTIVITIES ARE REGULATED UNDER STATE STANDARDS (I.E., STATE REQUIREMENTS THAT ARE NOT CONSIDERED PART OF THE STATE AUTHORIZED HAZARDOUS PROGRAM)."^^xsd:string ;
    rdfs:subClassOf epa-frs:HazardousWastePrograms .

epa-frs:StormWaterConstruction a owl:Class ;
    rdfs:label "STORM WATER CONSTRUCTION"^^xsd:string ;
    dcterms:description "THE STORM WATER PROGRAM, A COMPONENT OF THE CLEAN WATER ACT (CWA) NATIONAL POLLUTANT DISCHARGE ELIMINATION SYSTEM (NPDES), REQUIRES NPDES PERMITS FOR STORM WATER DISCHARGES FROM CONSTRUCTIONS SITES."^^xsd:string ;
    rdfs:subClassOf epa-frs:WasteWaterPrograms .

epa-frs:StormWaterIndustrial a owl:Class ;
    rdfs:label "STORM WATER INDUSTRIAL"^^xsd:string ;
    dcterms:description "THE STORM WATER PROGRAM, A COMPONENT OF THE CLEAN WATER ACT (CWA) NATIONAL POLLUTANT DISCHARGE ELIMINATION SYSTEM (NPDES), REQUIRES NPDES PERMITS FOR STORM WATER DISCHARGES FROM INDUSTRIES."^^xsd:string ;
    rdfs:subClassOf epa-frs:WasteWaterPrograms .

epa-frs:Superfund a owl:Class ;
    rdfs:label "SUPERFUND"^^xsd:string ;
    dcterms:description "AN UNCONTROLLED OR ABANDONED PLACE WHERE HAZARDOUS WASTE IS LOCATED, POSSIBLY AFFECTING LOCAL ECOSYSTEMS OR PEOPLE."^^xsd:string ;
    rdfs:subClassOf epa-frs:RemediationAndRedevelopmentPrograms .

epa-frs:Superfund-Non-NPL a owl:Class ;
    rdfs:label "SUPERFUND (NON-NPL)"^^xsd:string ;
    dcterms:description "AN UNCONTROLLED OR ABANDONED PLACE WHERE HAZARDOUS WASTE IS LOCATED, POSSIBLY AFFECTING LOCAL ECOSYSTEMS OR PEOPLE."^^xsd:string ;
    rdfs:subClassOf epa-frs:RemediationAndRedevelopmentPrograms .

epa-frs:SuperfundNPL a owl:Class ;
    rdfs:label "SUPERFUND NPL"^^xsd:string ;
    dcterms:description "A SUPERFUND SITE WHICH IS LISTED, PROPOSED, OR PREVIOUSLY LISTED ON THE NATIONAL PRIORITIES LIST (NPL).  THE NPL LISTS NATIONAL PRIORITIES AMONG THE KNOWN RELEASES OR THREATENED RELEASES OF HAZARDOUS SUBSTANCES, POLLUTANTS, OR CONTAMINANTS THROUGHOUT THE UNITED STATES."^^xsd:string ;
    rdfs:subClassOf epa-frs:RemediationAndRedevelopmentPrograms .

epa-frs:SurfaceWaterSite a owl:Class ;
    rdfs:label "SURFACE WATER SITE"^^xsd:string ;
    dcterms:description "AN ENVIRONMENTAL PROGRAM THAT IMPROVES THE QUALITY OF AND PROTECTS NON-COASTAL AND AQUATIC ECOSYSTEMS FROM POLLUTION."^^xsd:string ;
    rdfs:subClassOf epa-frs:WasteWaterPrograms .

epa-frs:TRIReporter a owl:Class ;
    rdfs:label "TRI REPORTER"^^xsd:string ;
    dcterms:description "A TOXIC RELEASE INVENTORY REPORTER IS A FACILITY WHICH:  EMPLOYS THE EQUIVALENT OF 10 OR MORE FULL-TIME EMPLOYEES; AND IS INCLUDED IN STANDARD INDUSTRIAL CLASSIFICATION (SIC) CODES 10XX, 12XX, 20XX-39XX, 4911, 4931, 4939, 4953, 5169, 5171, OR 7389; AND MANUFACTURES (DEFINED TO INCLUDE IMPORTING), PROCESSES, OR OTHERWISE USES ANY EMERGENCY PLANNING AND COMMUNITY RIGHT-TO-KNOW ACT (EPCRA) SECTION 313 CHEMICAL IN QUANTITIES GREATER THAN THE ESTABLISHED THRESHOLD IN THE COURSE OF A CALENDAR YEAR  (I.E., MANUFACTURES OR PROCESSES OVER 25,000 POUNDS OF THE APPROXIMATELY 600 DESIGNATED CHEMICALS OR 28 CHEMICAL CATEGORIES SPECIFIED IN THE REGULATIONS, OR USES MORE THAN 10,000 POUNDS OF ANY DESIGNATED CHEMICAL OR CATEGORY)."^^xsd:string ;
    rdfs:subClassOf epa-frs:ChemicalReleasePrograms .

epa-frs:TSCASubmitter a owl:Class ;
    rdfs:label "TSCA SUBMITTER"^^xsd:string ;
    dcterms:description "THE TOXIC SUBSTANCES CONTROL ACT (TSCA) OF 1976 PROVIDES EPA WITH AUTHORITY TO REQUIRE REPORTING, RECORD-KEEPING AND TESTING REQUIREMENTS, AND RESTRICTIONS RELATING TO CHEMICAL SUBSTANCES AND/OR MIXTURES. CERTAIN SUBSTANCES ARE GENERALLY EXCLUDED FROM TSCA, INCLUDING, AMONG OTHERS, FOOD, DRUGS, COSMETICS AND PESTICIDES. TSCA ADDRESSES THE PRODUCTION, IMPORTATION, USE, AND DISPOSAL OF SPECIFIC CHEMICALS INCLUDING POLYCHLORINATED BIPHENYLS (PCBS), ASBESTOS, RADON AND LEAD-BASED PAINT."^^xsd:string ;
    rdfs:subClassOf epa-frs:ChemicalReleasePrograms .

epa-frs:TSD a owl:Class ;
    rdfs:label "TSD"^^xsd:string ;
    dcterms:description "A HAZARDOUS WASTE TREATMENT, STORAGE, AND DISPOSAL (TSD) FACILITY PERFORMS ONE OR MORE OF THE FOLLOWING FUNCTIONS:  (1) TREATMENT: ANY METHOD, TECHNIQUE, OR PROCESS, INCLUDING NEUTRALIZATION, DESIGNED TO CHANGE THE PHYSICAL, CHEMICAL OR BIOLOGICAL CHARACTER OR COMPOSITION OF ANY HAZARDOUS WASTE SO AS TO NEUTRALIZE SUCH WASTE, OR SO AS TO RECOVER ENERGY OR MATERIAL RESOURCES FROM THE WASTE, OR SO AS TO RENDER SUCH WASTE NON-HAZARDOUS, OR LESS HAZARDOUS; SAFER TO TRANSPORT, STORE OR DISPOSE OF; OR AMENABLE FOR RECOVERY, AMENABLE FOR STORAGE, OR REDUCED IN VOLUME.  (2) STORAGE: THE HOLDING OF HAZARDOUS WASTE FOR A TEMPORARY PERIOD, AT THE END OF WHICH THE HAZARDOUS WASTE IS TREATED, DISPOSED OF, OR STORED ELSEWHERE.  (3) DISPOSAL: THE DISCHARGE, DEPOSIT, INJECTION, DUMPING, SPILLING, LEAKING, OR PLACING OF ANY SOLID WASTE OR HAZARDOUS WASTE INTO OR ON ANY LAND OR WATER SO THAT SUCH SOLID WASTE OR HAZARDOUS WASTE OR ANY CONSTITUENT THEREOF MAY ENTER THE ENVIRONMENT OR BE EMITTED INTO THE AIR OR DISCHARGED INTO ANY WATERS, INCLUDING GROUNDWATERS."^^xsd:string ;
    rdfs:subClassOf epa-frs:HazardousWastePrograms .

epa-frs:Title200ReimbursementFund a owl:Class ;
    rdfs:label "TITLE 200 REIMBURSEMENT FUND"^^xsd:string ;
    dcterms:description "THE TITLE 200 PETROLEUM RELEASE REMEDIAL ACTION REIMBURSEMENT FUND REIMBURSES CERTAIN COSTS FOR THE CLEANUP OF LEAKING PETROLEUM TANKS."^^xsd:string ;
    rdfs:subClassOf epa-frs:AssistanceAndSupportPrograms .

epa-frs:TitleVAreaSource a owl:Class ;
    rdfs:label "TITLE V AREA SOURCE"^^xsd:string ;
    dcterms:description "EPS"^^xsd:string ;
    rdfs:subClassOf epa-frs:ElectronicPermitSystem .

epa-frs:TitleVMajorSource a owl:Class ;
    rdfs:label "TITLE V MAJOR SOURCE"^^xsd:string ;
    dcterms:description "EPS"^^xsd:string ;
    rdfs:subClassOf epa-frs:ElectronicPermitSystem .

epa-frs:TransferFacility a owl:Class ;
    rdfs:label "TRANSFER FACILITY"^^xsd:string ;
    dcterms:description "A HAZARDOUS WASTE TRANSFER FACILITY HOLDS MANIFESTED HAZARDOUS WASTE(S) FOR A PERIOD OF TEN DAYS OR LESS WHILE THE WASTE IS IN TRANSIT."^^xsd:string ;
    rdfs:subClassOf epa-frs:HazardousWastePrograms .

epa-frs:Transporter a owl:Class ;
    rdfs:label "TRANSPORTER"^^xsd:string ;
    dcterms:description "HAZARDOUS WASTE HANDLERS ENGAGED IN THE TRANSPORTATION OF HAZARDOUS WASTE."^^xsd:string ;
    rdfs:subClassOf epa-frs:HazardousWastePrograms .

epa-frs:TribalMaster a owl:Class ;
    rdfs:label "TRIBAL MASTER"^^xsd:string ;
    dcterms:description "A TRIBAL REGISTRY SYSTEM THAT MAINTAINS BASIC IDENTIFICATION INFORMATION FOR A FACILITY SITE ON TRIBAL LAND, INCLUDING THE TRIBAL MASTER IDENTIFIER, GEOGRAPHIC ADDRESS, AFFILIATED ORGANIZATIONS AND CONTACTS, INDUSTRIAL CLASSIFICATIONS, AND LINKAGES TO ENVIRONMENTAL PERMITS AND PROGRAMS."^^xsd:string ;
    rdfs:subClassOf epa-frs:FacilitySiteIdentification .

epa-frs:UIC a owl:Class ;
    rdfs:label "UIC"^^xsd:string ;
    dcterms:description "UNDERGROUND INJECTION CONTROL (UIC) IS THE SUBSURFACE EMPLACEMENT OF FLUIDS THROUGH A BORED, DRILLED OR DRIVEN WELL; OR THROUGH A DUG WELL, WHERE THE DEPTH OF THE DUG WELL IS GREATER THAN THE LARGEST SURFACE DIMENSION. UNDERGROUND INJECTION WELLS ARE REGULATED UNDER BOTH THE SAFE DRINKING WATER ACT AND THE RESOURCE CONSERVATION AND RECOVERY ACT (SEE 40 CFR PART 148)."^^xsd:string ;
    rdfs:subClassOf epa-frs:HazardousWastePrograms .

epa-frs:UndergroundStorageTankProgram a owl:Class ;
    rdfs:label "UNDERGROUND STORAGE TANK PROGRAM"^^xsd:string ;
    dcterms:description "AN ENVIRONMENTAL PROGRAM DESIGNED TO REDUCE THE CHANCE OF RELEASES FROM UNDERGROUND STORAGE TANKS (USTS), DETECT LEAKS AND SPILLS WHEN THEY DO OCCUR, AND SECURE PROMPT CLEANUP.  AN UST IS A TANK SYSTEM, INCLUDING PIPING CONNECTED TO THE TANK, THAT HAS AT LEAST 10 PERCENT OF ITS VOLUME UNDERGROUND."^^xsd:string ;
    rdfs:subClassOf epa-frs:UndergroundStorageTankPrograms .

epa-frs:UnspecifiedUniverse a owl:Class ;
    rdfs:label "UNSPECIFIED UNIVERSE"^^xsd:string ;
    dcterms:description "THE HANDLER IS NOT CURRENTLY CLASSIFIED IN ANY HAZARDOUS WASTE UNIVERSE."^^xsd:string ;
    rdfs:subClassOf epa-frs:HazardousWastePrograms .

epa-frs:UsedOilProgram a owl:Class ;
    rdfs:label "USED OIL PROGRAM"^^xsd:string ;
    dcterms:description "AN ENVIRONMENTAL PROGRAM THAT PROMOTES THE PROPER MANAGEMENT OF USED OIL, INCLUDING STANDARDS AND REGULATIONS THAT APPLY TO IDENTIFYING, STORING, RECYCLING, TRANSPORTING, AND BURNING USED OIL."^^xsd:string ;
    rdfs:subClassOf epa-frs:HazardousWastePrograms .

epa-frs:VSQG a owl:Class ;
    rdfs:label "VSQG"^^xsd:string ;
    dcterms:description "VERY SMALL QUANTITY GENERATORS (VSQGS) GENERATE 100 KILOGRAMS OR LESS PER MONTH OF HAZARDOUS WASTE OR ONE KILOGRAM OR LESS PER MONTH OF ACUTELY HAZARDOUS WASTE. VSQGS MAY NOT ACCUMULATE MORE THAN 1,000 KILOGRAMS OF HAZARDOUS WASTE AT ANY TIME."^^xsd:string ;
    rdfs:subClassOf epa-frs:HazardousWastePrograms .

epa-frs:VoluntaryCleanUpProgram a owl:Class ;
    rdfs:label "VOLUNTARY CLEAN UP PROGRAM"^^xsd:string ;
    dcterms:description "AN ENVIRONMENTAL PROGRAM TO ENCOURAGE THE VOLUNTARY CLEANUP OF SITES WHERE THERE HAS BEEN A CONTAMINANT RELEASE THREATENING PUBLIC HEALTH AND THE ENVIRONMENT, THEREBY REMOVING THE STIGMA ATTACHED TO THESE SITES WHICH BLOCKS ECONOMIC REDEVELOPMENT."^^xsd:string ;
    rdfs:subClassOf epa-frs:RemediationAndRedevelopmentPrograms .

epa-frs:WasteDischargeRequirements a owl:Class ;
    rdfs:label "WASTE DISCHARGE REQUIREMENTS"^^xsd:string ;
    dcterms:description "SITES THAT DISCHARGE WASTEWATER TO LAND OR NON-FEDERAL WATERS WHICH ARE EXEMPT FROM TITLE 27 REGULATIONS AND NPDES REGULATIONS. CONTAINS PRIMARILY GROUNDWATER SITES ISSUED UNDER STATE AUTHORITY, THOUGH IT ALSO INCLUDES NON-FEDERAL SURFACE WATERS."^^xsd:string ;
    rdfs:subClassOf epa-frs:WasteWaterPrograms .

epa-frs:WastewaterFacility a owl:Class ;
    rdfs:label "WASTEWATER FACILITY"^^xsd:string ;
    dcterms:description "AN ENVIRONMENTAL PROGRAM CONCERNED WITH THE DESIGN, OPERATION, AND MAINTENANCE OF WASTEWATER TREATMENT FACILITIES.  A WASTEWATER TREATMENT FACILITY RECEIVES WASTE WATERS ( AND SOMETIMES RUNOFF) FROM DOMESTIC AND/OR INDUSTRIAL SOURCES, AND BY A COMBINATION OF PHYSICAL, CHEMICAL, AND BIOLOGICAL PROCESSES REDUCES (TREATS) THE WASTE WATERS TO LESS HARMFUL BYPRODUCTS."^^xsd:string ;
    rdfs:subClassOf epa-frs:WasteWaterPrograms .

epa-frs:WastewaterProgram a owl:Class ;
    rdfs:label "WASTEWATER PROGRAM"^^xsd:string ;
    dcterms:description "AN ENVIRONMENTAL PROGRAM THAT REGULATES DISCHARGES OF POLLUTANTS TO WATERS OF THE UNITED STATES, AS REQUIRED BY THE CLEAN WATER ACT."^^xsd:string ;
    rdfs:subClassOf epa-frs:WasteWaterPrograms .

epa-frs:WaterQualityProgram a owl:Class ;
    rdfs:label "WATER QUALITY PROGRAM"^^xsd:string ;
    dcterms:description "PROGRAMS AND PROJECTS DESIGNED TO REDUCE SOURCE WATER POLLUTION SUCH AS STORMWATER MANAGEMENT, STORMWATER PERMITTING, LAND USE REGULATION, WATER QUALITY MANAGEMENT PLANNING, WATER CONSERVATION, WATER SUPPLY ADMINISTRATION AND OTHER STATE AND LOCAL PROGRAMS. "^^xsd:string ;
    rdfs:subClassOf epa-frs:WasteWaterPrograms .

epa-frs:WaterTreatmentPlant a owl:Class ;
    rdfs:label "WATER TREATMENT PLANT"^^xsd:string ;
    dcterms:description "A WATER TREATMENT FACILITY WHICH IS PART OF A PUBLIC DRINKING WATER SYSTEM."^^xsd:string ;
    rdfs:subClassOf epa-frs:DrinkingWaterPrograms .

epa-frs:WoodWasteRecycling a owl:Class ;
    rdfs:label "WOOD WASTE RECYCLING"^^xsd:string ;
    dcterms:description "AN ENVIRONMENTAL PROGRAM WHICH ASSURES THE PROPER MANAGEMENT AND RECYCLING OF NATURAL WOOD WASTES SUCH AS TREE LIMBS, BRUSH, TREE STUMPS, ROOT MATS, LOGS, LEAVES, GRASS CLIPPINGS AND OTHER NATURAL MATERIALS THAT ARE GENERATED WHEN LAND IS CLEARED FOR CONSTRUCTION PURPOSES.  NATURAL WOOD WASTE RECYCLING FACILITIES MAY PRODUCE A VARIETY OF PRODUCTS INCLUDING COMPOST AND MULCH WHICH MAY BE SOLD TO CONSUMERS."^^xsd:string ;
    rdfs:subClassOf epa-frs:SolidWastePrograms .

epa-frs:X-RayEquipment a owl:Class ;
    rdfs:label "X-RAY EQUIPMENT"^^xsd:string ;
    dcterms:description "AN ENVIRONMENTAL PROGRAM REQUIRING REGULAR REGISTRATION AND INSPECTION OF X-RAY UNITS AND LICENSING OF OPERATORS. "^^xsd:string ;
    rdfs:subClassOf epa-frs:RadiationProtectionPrograms .

epa-frs:controlledVocab a owl:Ontology .

epa-frs:hasIdentifier.ACES a owl:DatatypeProperty ;
    rdfs:label "has ACES identifier" ;
    dcterms:description "connects a facility to the identifier in AGENCY COMPLIANCE AND ENFORCEMENT SYSTEMS" ;
    rdfs:domain epa-frs:ACES-Facility ;
    rdfs:subPropertyOf dcterms:identifier .

epa-frs:hasIdentifier.ACRES a owl:DatatypeProperty ;
    rdfs:label "has ACRES identifier" ;
    dcterms:description "connects a facility to the identifier in ASSESSMENT, CLEANUP AND REDEVELOPMENT EXCHANGE SYSTEM" ;
    rdfs:domain epa-frs:ACRES-Facility ;
    rdfs:subPropertyOf dcterms:identifier .

epa-frs:hasIdentifier.AIR a owl:DatatypeProperty ;
    rdfs:label "has AIR identifier" ;
    dcterms:description "connects a facility to the identifier in ICIS-AIR (AIR)" ;
    rdfs:domain epa-frs:AIR-Facility ;
    rdfs:subPropertyOf dcterms:identifier .

epa-frs:hasIdentifier.AIRS-AFS a owl:DatatypeProperty ;
    rdfs:label "has AIRS/AFS identifier" ;
    dcterms:description "connects a facility to the identifier in AIR FACILITY SYSTEM" ;
    rdfs:domain epa-frs:AIRS-AFS-Facility ;
    rdfs:subPropertyOf dcterms:identifier .

epa-frs:hasIdentifier.AIRS-AQS a owl:DatatypeProperty ;
    rdfs:label "has AIRS/AQS identifier" ;
    dcterms:description "connects a facility to the identifier in AIR QUALITY SYSTEM" ;
    rdfs:domain epa-frs:AIRS-AQS-Facility ;
    rdfs:subPropertyOf dcterms:identifier .

epa-frs:hasIdentifier.AZURITE a owl:DatatypeProperty ;
    rdfs:label "has AZURITE identifier" ;
    dcterms:description "connects a facility to the identifier in ARIZONA UNIFIED REPOSITORY FOR INFORMATIONAL TRACKING OF THE ENVIRONMENT" ;
    rdfs:domain epa-frs:AZURITE-Facility ;
    rdfs:subPropertyOf dcterms:identifier .

epa-frs:hasIdentifier.BIA-INDIAN-SCHOOL a owl:DatatypeProperty ;
    rdfs:label "has BIA INDIAN SCHOOL identifier" ;
    dcterms:description "connects a facility to the identifier in BUREAU OF INDIAN AFFAIRS INDIAN SCHOOL" ;
    rdfs:domain epa-frs:BIA-INDIAN-SCHOOL-Facility ;
    rdfs:subPropertyOf dcterms:identifier .

epa-frs:hasIdentifier.BR a owl:DatatypeProperty ;
    rdfs:label "has BR identifier" ;
    dcterms:description "connects a facility to the identifier in BIENNIAL REPORTERS" ;
    rdfs:domain epa-frs:BR-Facility ;
    rdfs:subPropertyOf dcterms:identifier .

epa-frs:hasIdentifier.BRAC a owl:DatatypeProperty ;
    rdfs:label "has BRAC identifier" ;
    dcterms:description "connects a facility to the identifier in BASE REALIGNMENT AND CLOSURE" ;
    rdfs:domain epa-frs:BRAC-Facility ;
    rdfs:subPropertyOf dcterms:identifier .

epa-frs:hasIdentifier.CA-CERS a owl:DatatypeProperty ;
    rdfs:label "has CA-CERS identifier" ;
    dcterms:description "connects a facility to the identifier in CA-CALIFORNIA ENVIRONMENTAL REPORTING SYSTEM" ;
    rdfs:domain epa-frs:CA-CERS-Facility ;
    rdfs:subPropertyOf dcterms:identifier .

epa-frs:hasIdentifier.CA-ENVIROVIEW a owl:DatatypeProperty ;
    rdfs:label "has CA-ENVIROVIEW identifier" ;
    dcterms:description "connects a facility to the identifier in CALIFORNIA - ENVIROVIEW" ;
    rdfs:domain epa-frs:CA-ENVIROVIEW-Facility ;
    rdfs:subPropertyOf dcterms:identifier .

epa-frs:hasIdentifier.CAMDBS a owl:DatatypeProperty ;
    rdfs:label "has CAMDBS identifier" ;
    dcterms:description "connects a facility to the identifier in CLEAN AIR MARKETS DIVISION (CAMD) BUSINESS SYSTEMS" ;
    rdfs:domain epa-frs:CAMDBS-Facility ;
    rdfs:subPropertyOf dcterms:identifier .

epa-frs:hasIdentifier.CASWIS a owl:DatatypeProperty ;
    rdfs:label "has CASWIS identifier" ;
    dcterms:description "connects a facility to the identifier in CALIFORNIA SOLID WASTE INFORMATION SYSTEM" ;
    rdfs:domain epa-frs:CASWIS-Facility ;
    rdfs:subPropertyOf dcterms:identifier .

epa-frs:hasIdentifier.CDAFLP a owl:DatatypeProperty ;
    rdfs:label "has CDAFLP identifier" ;
    dcterms:description "connects a facility to the identifier in COEUR D'ALENE FACILITY LOCATION PROGRAM" ;
    rdfs:domain epa-frs:CDAFLP-Facility ;
    rdfs:subPropertyOf dcterms:identifier .

epa-frs:hasIdentifier.CEDRI a owl:DatatypeProperty ;
    rdfs:label "has CEDRI identifier" ;
    dcterms:description "connects a facility to the identifier in COMPLIANCE AND EMISSIONS DATA REPORTING INTERFACE" ;
    rdfs:domain epa-frs:CEDRI-Facility ;
    rdfs:subPropertyOf dcterms:identifier .

epa-frs:hasIdentifier.CEDS a owl:DatatypeProperty ;
    rdfs:label "has CEDS identifier" ;
    dcterms:description "connects a facility to the identifier in VIRGINIA - COMPREHENSIVE ENVIRONMENTAL DATA SYSTEM" ;
    rdfs:domain epa-frs:CEDS-Facility ;
    rdfs:subPropertyOf dcterms:identifier .

epa-frs:hasIdentifier.CERCLIS a owl:DatatypeProperty ;
    rdfs:label "has CERCLIS identifier" ;
    dcterms:description "connects a facility to the identifier in COMPREHENSIVE ENVIRONMENTAL RESPONSE, COMPENSATION, AND LIABILITY INFORMATION SYSTEM" ;
    rdfs:domain epa-frs:CERCLIS-Facility ;
    rdfs:subPropertyOf dcterms:identifier .

epa-frs:hasIdentifier.CIM a owl:DatatypeProperty ;
    rdfs:label "has CIM identifier" ;
    dcterms:description "connects a facility to the identifier in UTAH - COMMON IDENTIFIER MECHANISM" ;
    rdfs:domain epa-frs:CIM-Facility ;
    rdfs:subPropertyOf dcterms:identifier .

epa-frs:hasIdentifier.CNFRS a owl:DatatypeProperty ;
    rdfs:label "has CNFRS identifier" ;
    dcterms:description "connects a facility to the identifier in CHEROKEE NATION FACILITY REGISTRY SYSTEM" ;
    rdfs:domain epa-frs:CNFRS-Facility ;
    rdfs:subPropertyOf dcterms:identifier .

epa-frs:hasIdentifier.CWNS a owl:DatatypeProperty ;
    rdfs:label "has CWNS identifier" ;
    dcterms:description "connects a facility to the identifier in CLEAN WATERSHEDS NEEDS SURVEY" ;
    rdfs:domain epa-frs:CWNS-Facility ;
    rdfs:subPropertyOf dcterms:identifier .

epa-frs:hasIdentifier.DEN a owl:DatatypeProperty ;
    rdfs:label "has DEN identifier" ;
    dcterms:description "connects a facility to the identifier in DELAWARE ENVIRONMENTAL NAVIGATOR" ;
    rdfs:domain epa-frs:DEN-Facility ;
    rdfs:subPropertyOf dcterms:identifier .

epa-frs:hasIdentifier.DTSC-ENVIROSTOR a owl:DatatypeProperty ;
    rdfs:label "has DTSC-ENVIROSTOR identifier" ;
    dcterms:description "connects a facility to the identifier in CALIFORNIA - DEPARTMENT OF TOXIC SUBSTANCES CONTROL - ENVIROSTOR SYSTEM" ;
    rdfs:domain epa-frs:DTSC-ENVIROSTOR-Facility ;
    rdfs:subPropertyOf dcterms:identifier .

epa-frs:hasIdentifier.E-GGRT a owl:DatatypeProperty ;
    rdfs:label "has E-GGRT identifier" ;
    dcterms:description "connects a facility to the identifier in ELECTRONIC GREENHOUSE GAS REPORTING TOOL (E-GGRT)" ;
    rdfs:domain epa-frs:E-GGRT-Facility ;
    rdfs:subPropertyOf dcterms:identifier .

epa-frs:hasIdentifier.ECRM a owl:DatatypeProperty ;
    rdfs:label "has ECRM identifier" ;
    dcterms:description "connects a facility to the identifier in ENFORCEMENT CRIMINAL RECORDS MANAGEMENT" ;
    rdfs:domain epa-frs:ECRM-Facility ;
    rdfs:subPropertyOf dcterms:identifier .

epa-frs:hasIdentifier.EGRID a owl:DatatypeProperty ;
    rdfs:label "has EGRID identifier" ;
    dcterms:description "connects a facility to the identifier in EMISSIONS & GENERATION RESOURCE INTEGRATED DATABASE" ;
    rdfs:domain epa-frs:EGRID-Facility ;
    rdfs:subPropertyOf dcterms:identifier .

epa-frs:hasIdentifier.EIA-860 a owl:DatatypeProperty ;
    rdfs:label "has EIA-860 identifier" ;
    dcterms:description "connects a facility to the identifier in ENERGY INFORMATION ADMINISTRATION-860 (EIA-860) DATABASE" ;
    rdfs:domain epa-frs:EIA-860-Facility ;
    rdfs:subPropertyOf dcterms:identifier .

epa-frs:hasIdentifier.EIS a owl:DatatypeProperty ;
    rdfs:label "has EIS identifier" ;
    dcterms:description "connects a facility to the identifier in EMISSION INVENTORY SYSTEM (EIS)" ;
    rdfs:domain epa-frs:EIS-Facility ;
    rdfs:subPropertyOf dcterms:identifier .

epa-frs:hasIdentifier.EPS a owl:DatatypeProperty ;
    rdfs:label "has EPS identifier" ;
    dcterms:description "connects a facility to the identifier in ELECTRONIC PERMIT SYSTEM" ;
    rdfs:domain epa-frs:EPS-Facility ;
    rdfs:subPropertyOf dcterms:identifier .

epa-frs:hasIdentifier.FARR a owl:DatatypeProperty ;
    rdfs:label "has FARR identifier" ;
    dcterms:description "connects a facility to the identifier in FEDERAL AIR RULES FOR RESERVATIONS (FARR) REGISTRATION PROGRAM" ;
    rdfs:domain epa-frs:FARR-Facility ;
    rdfs:subPropertyOf dcterms:identifier .

epa-frs:hasIdentifier.FDM a owl:DatatypeProperty ;
    rdfs:label "has FDM identifier" ;
    dcterms:description "connects a facility to the identifier in FLORIDA - FIESTA DATA MAINTENANCE" ;
    rdfs:domain epa-frs:FDM-Facility ;
    rdfs:subPropertyOf dcterms:identifier .

epa-frs:hasIdentifier.FFDOCKET a owl:DatatypeProperty ;
    rdfs:label "has FFDOCKET identifier" ;
    dcterms:description "connects a facility to the identifier in FEDERAL FACILITY HAZARDOUS WASTE COMPLIANCE DOCKET" ;
    rdfs:domain epa-frs:FFDOCKET-Facility ;
    rdfs:subPropertyOf dcterms:identifier .

epa-frs:hasIdentifier.FFEP a owl:DatatypeProperty ;
    rdfs:label "has FFEP identifier" ;
    dcterms:description "connects a facility to the identifier in FEDERAL FACILITIES RECOVERY AND REUSE OFFICE" ;
    rdfs:domain epa-frs:FFEP-Facility ;
    rdfs:subPropertyOf dcterms:identifier .

epa-frs:hasIdentifier.FIS a owl:DatatypeProperty ;
    rdfs:label "has FIS identifier" ;
    dcterms:description "connects a facility to the identifier in NEW YORK - FACILITY INFORMATION SYSTEM" ;
    rdfs:domain epa-frs:FIS-Facility ;
    rdfs:subPropertyOf dcterms:identifier .

epa-frs:hasIdentifier.GEIMS a owl:DatatypeProperty ;
    rdfs:label "has GEIMS identifier" ;
    dcterms:description "connects a facility to the identifier in GEORGIA - GEOGRAPHIC ENVIRONMENTAL INFORMATION MANAGEMENT SYSTEM" ;
    rdfs:domain epa-frs:GEIMS-Facility ;
    rdfs:subPropertyOf dcterms:identifier .

epa-frs:hasIdentifier.HI-EHW a owl:DatatypeProperty ;
    rdfs:label "has HI-EHW identifier" ;
    dcterms:description "connects a facility to the identifier in HAWAII ENVIRONMENTAL HEALTH WAREHOUSE" ;
    rdfs:domain epa-frs:HI-EHW-Facility ;
    rdfs:subPropertyOf dcterms:identifier .

epa-frs:hasIdentifier.HWTS-DATAMART a owl:DatatypeProperty ;
    rdfs:label "has HWTS-DATAMART identifier" ;
    dcterms:description "connects a facility to the identifier in HAZARDOUS WASTE TRACKING SYSTEM - DATAMART" ;
    rdfs:domain epa-frs:HWTS-DATAMART-Facility ;
    rdfs:subPropertyOf dcterms:identifier .

epa-frs:hasIdentifier.ICIS a owl:DatatypeProperty ;
    rdfs:label "has ICIS identifier" ;
    dcterms:description "connects a facility to the identifier in INTEGRATED COMPLIANCE INFORMATION SYSTEM" ;
    rdfs:domain epa-frs:ICIS-Facility ;
    rdfs:subPropertyOf dcterms:identifier .

epa-frs:hasIdentifier.IDDEQ a owl:DatatypeProperty ;
    rdfs:label "has IDDEQ identifier" ;
    dcterms:description "connects a facility to the identifier in IDAHO DEPARTMENT OF ENVIRONMENTAL QUALITY" ;
    rdfs:domain epa-frs:IDDEQ-Facility ;
    rdfs:subPropertyOf dcterms:identifier .

epa-frs:hasIdentifier.IDNR_EFD a owl:DatatypeProperty ;
    rdfs:label "has IDNR_EFD identifier" ;
    dcterms:description "connects a facility to the identifier in IOWA DEPARTMENT OF NATURAL RESOURCES - ENVIRONMENTAL FACILITIES DATABASE" ;
    rdfs:domain epa-frs:IDNR_EFD-Facility ;
    rdfs:subPropertyOf dcterms:identifier .

epa-frs:hasIdentifier.IN-FRS a owl:DatatypeProperty ;
    rdfs:label "has IN-FRS identifier" ;
    dcterms:description "connects a facility to the identifier in INDIANA - FACILITY REGISTRY SYSTEM" ;
    rdfs:domain epa-frs:IN-FRS-Facility ;
    rdfs:subPropertyOf dcterms:identifier .

epa-frs:hasIdentifier.IN-TEMPO a owl:DatatypeProperty ;
    rdfs:label "has IN-TEMPO identifier" ;
    dcterms:description "connects a facility to the identifier in INDIANA-TOOLS FOR ENVIRONMENTAL MANAGEMENT AND PROTECTION ORGANIZATIONS" ;
    rdfs:domain epa-frs:IN-TEMPO-Facility ;
    rdfs:subPropertyOf dcterms:identifier .

epa-frs:hasIdentifier.ISD a owl:DatatypeProperty ;
    rdfs:label "has ISD identifier" ;
    dcterms:description "connects a facility to the identifier in WYOMING - INDUSTRIAL SITING DIVISION" ;
    rdfs:domain epa-frs:ISD-Facility ;
    rdfs:subPropertyOf dcterms:identifier .

epa-frs:hasIdentifier.KS-FP a owl:DatatypeProperty ;
    rdfs:label "has KS-FP identifier" ;
    dcterms:description "connects a facility to the identifier in KANSAS - FACILITY PROFILE" ;
    rdfs:domain epa-frs:KS-FP-Facility ;
    rdfs:subPropertyOf dcterms:identifier .

epa-frs:hasIdentifier.KY-TEMPO a owl:DatatypeProperty ;
    rdfs:label "has KY-TEMPO identifier" ;
    dcterms:description "connects a facility to the identifier in KENTUCKY - TOOLS FOR ENVIRONMENTAL MANAGEMENT AND PROTECTION ORGANIZATIONS" ;
    rdfs:domain epa-frs:KY-TEMPO-Facility ;
    rdfs:subPropertyOf dcterms:identifier .

epa-frs:hasIdentifier.LA-TEMPO a owl:DatatypeProperty ;
    rdfs:label "has LA-TEMPO identifier" ;
    dcterms:description "connects a facility to the identifier in LOUISIANA - TOOLS FOR ENVIRONMENTAL MANAGEMENT AND PROTECTION ORGANIZATIONS" ;
    rdfs:domain epa-frs:LA-TEMPO-Facility ;
    rdfs:subPropertyOf dcterms:identifier .

epa-frs:hasIdentifier.LMOP a owl:DatatypeProperty ;
    rdfs:label "has LMOP identifier" ;
    dcterms:description "connects a facility to the identifier in LANDFILL METHANE OUTREACH PROGRAM" ;
    rdfs:domain epa-frs:LMOP-Facility ;
    rdfs:subPropertyOf dcterms:identifier .

epa-frs:hasIdentifier.LUST-ARRA a owl:DatatypeProperty ;
    rdfs:label "has LUST-ARRA identifier" ;
    dcterms:description "connects a facility to the identifier in LEAKING UNDERGROUND STORAGE TANK (LUST) ¿ AMERICAN RECOVERY AND REINVESTMENT ACT (ARRA)" ;
    rdfs:domain epa-frs:LUST-ARRA-Facility ;
    rdfs:subPropertyOf dcterms:identifier .

epa-frs:hasIdentifier.MA-EPICS a owl:DatatypeProperty ;
    rdfs:label "has MA-EPICS identifier" ;
    dcterms:description "connects a facility to the identifier in MASSACHUSETTS - ENVIRONMENTAL PROTECTION INTEGRATED COMPUTER SYSTEM" ;
    rdfs:domain epa-frs:MA-EPICS-Facility ;
    rdfs:subPropertyOf dcterms:identifier .

epa-frs:hasIdentifier.MD-EPSC a owl:DatatypeProperty ;
    rdfs:label "has MD-EPSC identifier" ;
    dcterms:description "connects a facility to the identifier in MARYLAND - ENVIRONMENTAL PERMIT SERVICE CENTER" ;
    rdfs:domain epa-frs:MD-EPSC-Facility ;
    rdfs:subPropertyOf dcterms:identifier .

epa-frs:hasIdentifier.MD-PEMIS a owl:DatatypeProperty ;
    rdfs:label "has MD-PEMIS identifier" ;
    dcterms:description "connects a facility to the identifier in MARYLAND - PERMANENT (AIR) EMISSION" ;
    rdfs:domain epa-frs:MD-PEMIS-Facility ;
    rdfs:subPropertyOf dcterms:identifier .

epa-frs:hasIdentifier.MD-RCRA a owl:DatatypeProperty ;
    rdfs:label "has MD-RCRA identifier" ;
    dcterms:description "connects a facility to the identifier in MARYLAND-RESOURCE CONVERSATION AND RECOVERY ACT DATABASE" ;
    rdfs:domain epa-frs:MD-RCRA-Facility ;
    rdfs:subPropertyOf dcterms:identifier .

epa-frs:hasIdentifier.MD-TEMPO a owl:DatatypeProperty ;
    rdfs:label "has MD-TEMPO identifier" ;
    dcterms:description "connects a facility to the identifier in MARYLAND - TOOLS FOR ENVIRONMENTAL MANAGEMENT AND PROTECTION ORGANIZATIONS (TEMPO)" ;
    rdfs:domain epa-frs:MD-TEMPO-Facility ;
    rdfs:subPropertyOf dcterms:identifier .

epa-frs:hasIdentifier.ME-EFIS a owl:DatatypeProperty ;
    rdfs:label "has ME-EFIS identifier" ;
    dcterms:description "connects a facility to the identifier in MAINE - ENVIRONMENTAL FACILITY INFORMATION SYSTEM" ;
    rdfs:domain epa-frs:ME-EFIS-Facility ;
    rdfs:subPropertyOf dcterms:identifier .

epa-frs:hasIdentifier.MERI-FIS a owl:DatatypeProperty ;
    rdfs:label "has MERI-FIS identifier" ;
    dcterms:description "connects a facility to the identifier in MEADOWLANDS ENVIRONMENTAL RESEARCH INSTITUTE – FACILITY INFORMATION SYSTEM" ;
    rdfs:domain epa-frs:MERI-FIS-Facility ;
    rdfs:subPropertyOf dcterms:identifier .

epa-frs:hasIdentifier.MN-TEMPO a owl:DatatypeProperty ;
    rdfs:label "has MN-TEMPO identifier" ;
    dcterms:description "connects a facility to the identifier in MINNESOTA - PERMITTING, COMPLIANCE, AND ENFORCEMENT INFORMATION MANAGEMENT SYSTEM" ;
    rdfs:domain epa-frs:MN-TEMPO-Facility ;
    rdfs:subPropertyOf dcterms:identifier .

epa-frs:hasIdentifier.MO-DNR a owl:DatatypeProperty ;
    rdfs:label "has MO-DNR identifier" ;
    dcterms:description "connects a facility to the identifier in MISSOURI DEPARTMENT OF NATURAL RESOURCES" ;
    rdfs:domain epa-frs:MO-DNR-Facility ;
    rdfs:subPropertyOf dcterms:identifier .

epa-frs:hasIdentifier.MS-ENSITE a owl:DatatypeProperty ;
    rdfs:label "has MS-ENSITE identifier" ;
    dcterms:description "connects a facility to the identifier in MISSISSIPPI - TOOLS FOR ENVIRONMENTAL MANAGEMENT AND PROTECTION ORGANIZATIONS" ;
    rdfs:domain epa-frs:MS-ENSITE-Facility ;
    rdfs:subPropertyOf dcterms:identifier .

epa-frs:hasIdentifier.MT-CEDARS a owl:DatatypeProperty ;
    rdfs:label "has MT-CEDARS identifier" ;
    dcterms:description "connects a facility to the identifier in MONTANA - CONSOLIDATED ENVIRONMENTAL DATA ACQUISITION AND RETRIEVAL SYSTEM" ;
    rdfs:domain epa-frs:MT-CEDARS-Facility ;
    rdfs:subPropertyOf dcterms:identifier .

epa-frs:hasIdentifier.NC-FITS a owl:DatatypeProperty ;
    rdfs:label "has NC-FITS identifier" ;
    dcterms:description "connects a facility to the identifier in NORTH CAROLINA - FACILITY IDENTIFICATION TEMPLATE FOR STATES" ;
    rdfs:domain epa-frs:NC-FITS-Facility ;
    rdfs:subPropertyOf dcterms:identifier .

epa-frs:hasIdentifier.NCDB a owl:DatatypeProperty ;
    rdfs:label "has NCDB identifier" ;
    dcterms:description "connects a facility to the identifier in NATIONAL COMPLIANCE DATABASE" ;
    rdfs:domain epa-frs:NCDB-Facility ;
    rdfs:subPropertyOf dcterms:identifier .

epa-frs:hasIdentifier.ND-FP a owl:DatatypeProperty ;
    rdfs:label "has ND-FP identifier" ;
    dcterms:description "connects a facility to the identifier in NORTH DAKOTA - FACILITY PROFILE" ;
    rdfs:domain epa-frs:ND-FP-Facility ;
    rdfs:subPropertyOf dcterms:identifier .

epa-frs:hasIdentifier.NDEQ a owl:DatatypeProperty ;
    rdfs:label "has NDEQ identifier" ;
    dcterms:description "connects a facility to the identifier in NEBRASKA DEPARTMENT OF ENVIRONMENTAL QUALITY" ;
    rdfs:domain epa-frs:NDEQ-Facility ;
    rdfs:subPropertyOf dcterms:identifier .

epa-frs:hasIdentifier.NEI a owl:DatatypeProperty ;
    rdfs:label "has NEI identifier" ;
    dcterms:description "connects a facility to the identifier in NATIONAL EMISSIONS INVENTORY" ;
    rdfs:domain epa-frs:NEI-Facility ;
    rdfs:subPropertyOf dcterms:identifier .

epa-frs:hasIdentifier.NH-DES a owl:DatatypeProperty ;
    rdfs:label "has NH-DES identifier" ;
    dcterms:description "connects a facility to the identifier in NEW HAMPSHIRE - DEPARTMENT OF ENVIRONMENTAL SERVICES" ;
    rdfs:domain epa-frs:NH-DES-Facility ;
    rdfs:subPropertyOf dcterms:identifier .

epa-frs:hasIdentifier.NJ-NJEMS a owl:DatatypeProperty ;
    rdfs:label "has NJ-NJEMS identifier" ;
    dcterms:description "connects a facility to the identifier in NEW JERSEY - NEW JERSEY ENVIRONMENTAL MANAGEMENT SYSTEM" ;
    rdfs:domain epa-frs:NJ-NJEMS-Facility ;
    rdfs:subPropertyOf dcterms:identifier .

epa-frs:hasIdentifier.NM-TEMPO a owl:DatatypeProperty ;
    rdfs:label "has NM-TEMPO identifier" ;
    dcterms:description "connects a facility to the identifier in NEW MEXICO-TOOLS FOR ENVIRONMENTAL MANAGEMENT AND PROTECTION ORGANIZATIONS" ;
    rdfs:domain epa-frs:NM-TEMPO-Facility ;
    rdfs:subPropertyOf dcterms:identifier .

epa-frs:hasIdentifier.NNEMS a owl:DatatypeProperty ;
    rdfs:label "has NNEMS identifier" ;
    dcterms:description "connects a facility to the identifier in NAVAJO NATION ENVIRONMENTAL MANAGEMENT SYSTEM" ;
    rdfs:domain epa-frs:NNEMS-Facility ;
    rdfs:subPropertyOf dcterms:identifier .

epa-frs:hasIdentifier.NPDES a owl:DatatypeProperty ;
    rdfs:label "has NPDES identifier" ;
    dcterms:description "connects a facility to the identifier in NATIONAL POLLUTANT DISCHARGE ELIMINATION SYSTEM (ICIS-NPDES)" ;
    rdfs:domain epa-frs:NPDES-Facility ;
    rdfs:subPropertyOf dcterms:identifier .

epa-frs:hasIdentifier.NV-FP a owl:DatatypeProperty ;
    rdfs:label "has NV-FP identifier" ;
    dcterms:description "connects a facility to the identifier in NEVADA - FACILITY PROFILE" ;
    rdfs:domain epa-frs:NV-FP-Facility ;
    rdfs:subPropertyOf dcterms:identifier .

epa-frs:hasIdentifier.OH-CORE a owl:DatatypeProperty ;
    rdfs:label "has OH-CORE identifier" ;
    dcterms:description "connects a facility to the identifier in OHIO - CORE FACILITY INFORMATION" ;
    rdfs:domain epa-frs:OH-CORE-Facility ;
    rdfs:subPropertyOf dcterms:identifier .

epa-frs:hasIdentifier.OR-DEQ a owl:DatatypeProperty ;
    rdfs:label "has OR-DEQ identifier" ;
    dcterms:description "connects a facility to the identifier in OREGON - DEPARTMENT OF ENVIRONMENTAL QUALITY" ;
    rdfs:domain epa-frs:OR-DEQ-Facility ;
    rdfs:subPropertyOf dcterms:identifier .

epa-frs:hasIdentifier.OSHA-OIS a owl:DatatypeProperty ;
    rdfs:label "has OSHA-OIS identifier" ;
    dcterms:description "connects a facility to the identifier in OCCUPATIONAL SAFETY AND HEALTH ADMINISTRATION INFORMATION SYSTEM" ;
    rdfs:domain epa-frs:OSHA-OIS-Facility ;
    rdfs:subPropertyOf dcterms:identifier .

epa-frs:hasIdentifier.OTAQREG a owl:DatatypeProperty ;
    rdfs:label "has OTAQREG identifier" ;
    dcterms:description "connects a facility to the identifier in OFFICE OF TRANSPORTATION AND AIR QUALITY FUELS REGISTRATION" ;
    rdfs:domain epa-frs:OTAQREG-Facility ;
    rdfs:subPropertyOf dcterms:identifier .

epa-frs:hasIdentifier.PA-EFACTS a owl:DatatypeProperty ;
    rdfs:label "has PA-EFACTS identifier" ;
    dcterms:description "connects a facility to the identifier in PENNSYLVANIA - ENVIRONMENTAL FACILITY APPLICATION COMPLIANCE TRACKING SYSTEM" ;
    rdfs:domain epa-frs:PA-EFACTS-Facility ;
    rdfs:subPropertyOf dcterms:identifier .

epa-frs:hasIdentifier.PDS a owl:DatatypeProperty ;
    rdfs:label "has PDS identifier" ;
    dcterms:description "connects a facility to the identifier in PERMIT DATA SYSTEM" ;
    rdfs:domain epa-frs:PDS-Facility ;
    rdfs:subPropertyOf dcterms:identifier .

epa-frs:hasIdentifier.PERMIT-TRACKING a owl:DatatypeProperty ;
    rdfs:label "has PERMIT TRACKING identifier" ;
    dcterms:description "connects a facility to the identifier in ALBAMA - PERMIT TRACKING" ;
    rdfs:domain epa-frs:PERMIT-TRACKING-Facility ;
    rdfs:subPropertyOf dcterms:identifier .

epa-frs:hasIdentifier.RADINFO a owl:DatatypeProperty ;
    rdfs:label "has RADINFO identifier" ;
    dcterms:description "connects a facility to the identifier in RADIATION INFORMATION SYSTEM" ;
    rdfs:domain epa-frs:RADINFO-Facility ;
    rdfs:subPropertyOf dcterms:identifier .

epa-frs:hasIdentifier.RBLC a owl:DatatypeProperty ;
    rdfs:label "has RBLC identifier" ;
    dcterms:description "connects a facility to the identifier in RACT/BACT/LAER CLEARINGHOUSE" ;
    rdfs:domain epa-frs:RBLC-Facility ;
    rdfs:subPropertyOf dcterms:identifier .

epa-frs:hasIdentifier.RCRAINFO a owl:DatatypeProperty ;
    rdfs:label "has RCRAINFO identifier" ;
    dcterms:description "connects a facility to the identifier in RESOURCE CONSERVATION AND RECOVERY ACT INFORMATION SYSTEM" ;
    rdfs:domain epa-frs:RCRAINFO-Facility ;
    rdfs:subPropertyOf dcterms:identifier .

epa-frs:hasIdentifier.REGION a owl:DatatypeProperty ;
    rdfs:label "has REGION identifier" ;
    dcterms:description "connects a facility to the identifier in REGION" ;
    rdfs:domain epa-frs:REGION-Facility ;
    rdfs:subPropertyOf dcterms:identifier .

epa-frs:hasIdentifier.RFS a owl:DatatypeProperty ;
    rdfs:label "has RFS identifier" ;
    dcterms:description "connects a facility to the identifier in RENEWABLE FUEL STANDARD" ;
    rdfs:domain epa-frs:RFS-Facility ;
    rdfs:subPropertyOf dcterms:identifier .

epa-frs:hasIdentifier.RI-PLOVER a owl:DatatypeProperty ;
    rdfs:label "has RI-PLOVER identifier" ;
    dcterms:description "connects a facility to the identifier in RHODE ISLAND - PERMITS, LICENSES AND OTHER VITAL ENVIRONMENTAL RECORDS" ;
    rdfs:domain epa-frs:RI-PLOVER-Facility ;
    rdfs:subPropertyOf dcterms:identifier .

epa-frs:hasIdentifier.RMP a owl:DatatypeProperty ;
    rdfs:label "has RMP identifier" ;
    dcterms:description "connects a facility to the identifier in RISK MANAGEMENT PLAN" ;
    rdfs:domain epa-frs:RMP-Facility ;
    rdfs:subPropertyOf dcterms:identifier .

epa-frs:hasIdentifier.SC-EFIS a owl:DatatypeProperty ;
    rdfs:label "has SC-EFIS identifier" ;
    dcterms:description "connects a facility to the identifier in SOUTH CAROLINA - ENVIRONMENTAL FACILITY INFORMATION SYSTEM" ;
    rdfs:domain epa-frs:SC-EFIS-Facility ;
    rdfs:subPropertyOf dcterms:identifier .

epa-frs:hasIdentifier.SEMS a owl:DatatypeProperty ;
    rdfs:label "has SEMS identifier" ;
    dcterms:description "connects a facility to the identifier in SUPERFUND ENTERPRISE MANAGEMENT SYSTEM" ;
    rdfs:domain epa-frs:SEMS-Facility ;
    rdfs:subPropertyOf dcterms:identifier .

epa-frs:hasIdentifier.SFDW a owl:DatatypeProperty ;
    rdfs:label "has SFDW identifier" ;
    dcterms:description "connects a facility to the identifier in SAFE DRINKING WATER INFORMATION SYSTEM" ;
    rdfs:domain epa-frs:SFDW-Facility ;
    rdfs:subPropertyOf dcterms:identifier .

epa-frs:hasIdentifier.SIMS a owl:DatatypeProperty ;
    rdfs:label "has SIMS identifier" ;
    dcterms:description "connects a facility to the identifier in CT - SITE INFORMATION MANAGEMENT SYSTEM" ;
    rdfs:domain epa-frs:SIMS-Facility ;
    rdfs:subPropertyOf dcterms:identifier .

epa-frs:hasIdentifier.SRPMICEMS a owl:DatatypeProperty ;
    rdfs:label "has SRPMICEMS identifier" ;
    dcterms:description "connects a facility to the identifier in SALT RIVER PIMA-MARICOPA INDIAN COMMUNITY ENVIRONMENTAL MANAGEMENT SYSTEM" ;
    rdfs:domain epa-frs:SRPMICEMS-Facility ;
    rdfs:subPropertyOf dcterms:identifier .

epa-frs:hasIdentifier.SSTS a owl:DatatypeProperty ;
    rdfs:label "has SSTS identifier" ;
    dcterms:description "connects a facility to the identifier in SECTION SEVEN TRACKING SYSTEM" ;
    rdfs:domain epa-frs:SSTS-Facility ;
    rdfs:subPropertyOf dcterms:identifier .

epa-frs:hasIdentifier.STATE a owl:DatatypeProperty ;
    rdfs:label "has STATE identifier" ;
    dcterms:description "connects a facility to the identifier in STATE SYSTEMS" ;
    rdfs:domain epa-frs:STATE-Facility ;
    rdfs:subPropertyOf dcterms:identifier .

epa-frs:hasIdentifier.SWIPR a owl:DatatypeProperty ;
    rdfs:label "has SWIPR identifier" ;
    dcterms:description "connects a facility to the identifier in SUBPART W IMPOUNDMENT PHOTOGRAPHIC REPORTING" ;
    rdfs:domain epa-frs:SWIPR-Facility ;
    rdfs:subPropertyOf dcterms:identifier .

epa-frs:hasIdentifier.TEST a owl:DatatypeProperty ;
    rdfs:label "has TEST identifier" ;
    dcterms:description "connects a facility to the identifier in TEST PROGRAM FOR CDX" ;
    rdfs:domain epa-frs:TEST-Facility ;
    rdfs:subPropertyOf dcterms:identifier .

epa-frs:hasIdentifier.TRIS a owl:DatatypeProperty ;
    rdfs:label "has TRIS identifier" ;
    dcterms:description "connects a facility to the identifier in TOXICS RELEASE INVENTORY SYSTEM" ;
    rdfs:domain epa-frs:TRIS-Facility ;
    rdfs:subPropertyOf dcterms:identifier .

epa-frs:hasIdentifier.TSCA a owl:DatatypeProperty ;
    rdfs:label "has TSCA identifier" ;
    dcterms:description "connects a facility to the identifier in TOXIC SUBSTANCES CONTROL ACT" ;
    rdfs:domain epa-frs:TSCA-Facility ;
    rdfs:subPropertyOf dcterms:identifier .

epa-frs:hasIdentifier.TX-TCEQ-ACR a owl:DatatypeProperty ;
    rdfs:label "has TX-TCEQ ACR identifier" ;
    dcterms:description "connects a facility to the identifier in TEXAS COMMISSION ON ENVIRONMENTAL QUALITY - AGENCY CENTRAL REGISTRY" ;
    rdfs:domain epa-frs:TX-TCEQ-ACR-Facility ;
    rdfs:subPropertyOf dcterms:identifier .

epa-frs:hasIdentifier.UORS a owl:DatatypeProperty ;
    rdfs:label "has UORS identifier" ;
    dcterms:description "connects a facility to the identifier in CALIFORNIA - USED OIL RECYCLING SYSTEM" ;
    rdfs:domain epa-frs:UORS-Facility ;
    rdfs:subPropertyOf dcterms:identifier .

epa-frs:hasIdentifier.UST a owl:DatatypeProperty ;
    rdfs:label "has UST identifier" ;
    dcterms:description "connects a facility to the identifier in UNDERGROUND STORAGE TANK" ;
    rdfs:domain epa-frs:UST-Facility ;
    rdfs:subPropertyOf dcterms:identifier .

epa-frs:hasIdentifier.WA-FSIS a owl:DatatypeProperty ;
    rdfs:label "has WA-FSIS identifier" ;
    dcterms:description "connects a facility to the identifier in WASHINGTON - FACILITY / SITE IDENTIFICATION SYSTEM" ;
    rdfs:domain epa-frs:WA-FSIS-Facility ;
    rdfs:subPropertyOf dcterms:identifier .

epa-frs:hasIdentifier.WI-ESR a owl:DatatypeProperty ;
    rdfs:label "has WI-ESR identifier" ;
    dcterms:description "connects a facility to the identifier in WISCONSIN - ENVIRONMENTAL SYSTEM REGISTRY" ;
    rdfs:domain epa-frs:WI-ESR-Facility ;
    rdfs:subPropertyOf dcterms:identifier .

epa-frs:ofIndustry.ACES a owl:ObjectProperty ;
    rdfs:label "of Industry in ACES" ;
    dcterms:description "connects a facility to an industry in AGENCY COMPLIANCE AND ENFORCEMENT SYSTEMS" ;
    rdfs:domain epa-frs:ACES-Facility ;
    rdfs:subPropertyOf fio:ofIndustry .

epa-frs:ofIndustry.ACRES a owl:ObjectProperty ;
    rdfs:label "of Industry in ACRES" ;
    dcterms:description "connects a facility to an industry in ASSESSMENT, CLEANUP AND REDEVELOPMENT EXCHANGE SYSTEM" ;
    rdfs:domain epa-frs:ACRES-Facility ;
    rdfs:subPropertyOf fio:ofIndustry .

epa-frs:ofIndustry.AIR a owl:ObjectProperty ;
    rdfs:label "of Industry in AIR" ;
    dcterms:description "connects a facility to an industry in ICIS-AIR (AIR)" ;
    rdfs:domain epa-frs:AIR-Facility ;
    rdfs:subPropertyOf fio:ofIndustry .

epa-frs:ofIndustry.AIRS-AFS a owl:ObjectProperty ;
    rdfs:label "of Industry in AIRS/AFS" ;
    dcterms:description "connects a facility to an industry in AIR FACILITY SYSTEM" ;
    rdfs:domain epa-frs:AIRS-AFS-Facility ;
    rdfs:subPropertyOf fio:ofIndustry .

epa-frs:ofIndustry.AIRS-AQS a owl:ObjectProperty ;
    rdfs:label "of Industry in AIRS/AQS" ;
    dcterms:description "connects a facility to an industry in AIR QUALITY SYSTEM" ;
    rdfs:domain epa-frs:AIRS-AQS-Facility ;
    rdfs:subPropertyOf fio:ofIndustry .

epa-frs:ofIndustry.AZURITE a owl:ObjectProperty ;
    rdfs:label "of Industry in AZURITE" ;
    dcterms:description "connects a facility to an industry in ARIZONA UNIFIED REPOSITORY FOR INFORMATIONAL TRACKING OF THE ENVIRONMENT" ;
    rdfs:domain epa-frs:AZURITE-Facility ;
    rdfs:subPropertyOf fio:ofIndustry .

epa-frs:ofIndustry.BIA-INDIAN-SCHOOL a owl:ObjectProperty ;
    rdfs:label "of Industry in BIA INDIAN SCHOOL" ;
    dcterms:description "connects a facility to an industry in BUREAU OF INDIAN AFFAIRS INDIAN SCHOOL" ;
    rdfs:domain epa-frs:BIA-INDIAN-SCHOOL-Facility ;
    rdfs:subPropertyOf fio:ofIndustry .

epa-frs:ofIndustry.BR a owl:ObjectProperty ;
    rdfs:label "of Industry in BR" ;
    dcterms:description "connects a facility to an industry in BIENNIAL REPORTERS" ;
    rdfs:domain epa-frs:BR-Facility ;
    rdfs:subPropertyOf fio:ofIndustry .

epa-frs:ofIndustry.BRAC a owl:ObjectProperty ;
    rdfs:label "of Industry in BRAC" ;
    dcterms:description "connects a facility to an industry in BASE REALIGNMENT AND CLOSURE" ;
    rdfs:domain epa-frs:BRAC-Facility ;
    rdfs:subPropertyOf fio:ofIndustry .

epa-frs:ofIndustry.CA-CERS a owl:ObjectProperty ;
    rdfs:label "of Industry in CA-CERS" ;
    dcterms:description "connects a facility to an industry in CA-CALIFORNIA ENVIRONMENTAL REPORTING SYSTEM" ;
    rdfs:domain epa-frs:CA-CERS-Facility ;
    rdfs:subPropertyOf fio:ofIndustry .

epa-frs:ofIndustry.CA-ENVIROVIEW a owl:ObjectProperty ;
    rdfs:label "of Industry in CA-ENVIROVIEW" ;
    dcterms:description "connects a facility to an industry in CALIFORNIA - ENVIROVIEW" ;
    rdfs:domain epa-frs:CA-ENVIROVIEW-Facility ;
    rdfs:subPropertyOf fio:ofIndustry .

epa-frs:ofIndustry.CAMDBS a owl:ObjectProperty ;
    rdfs:label "of Industry in CAMDBS" ;
    dcterms:description "connects a facility to an industry in CLEAN AIR MARKETS DIVISION (CAMD) BUSINESS SYSTEMS" ;
    rdfs:domain epa-frs:CAMDBS-Facility ;
    rdfs:subPropertyOf fio:ofIndustry .

epa-frs:ofIndustry.CASWIS a owl:ObjectProperty ;
    rdfs:label "of Industry in CASWIS" ;
    dcterms:description "connects a facility to an industry in CALIFORNIA SOLID WASTE INFORMATION SYSTEM" ;
    rdfs:domain epa-frs:CASWIS-Facility ;
    rdfs:subPropertyOf fio:ofIndustry .

epa-frs:ofIndustry.CDAFLP a owl:ObjectProperty ;
    rdfs:label "of Industry in CDAFLP" ;
    dcterms:description "connects a facility to an industry in COEUR D'ALENE FACILITY LOCATION PROGRAM" ;
    rdfs:domain epa-frs:CDAFLP-Facility ;
    rdfs:subPropertyOf fio:ofIndustry .

epa-frs:ofIndustry.CEDRI a owl:ObjectProperty ;
    rdfs:label "of Industry in CEDRI" ;
    dcterms:description "connects a facility to an industry in COMPLIANCE AND EMISSIONS DATA REPORTING INTERFACE" ;
    rdfs:domain epa-frs:CEDRI-Facility ;
    rdfs:subPropertyOf fio:ofIndustry .

epa-frs:ofIndustry.CEDS a owl:ObjectProperty ;
    rdfs:label "of Industry in CEDS" ;
    dcterms:description "connects a facility to an industry in VIRGINIA - COMPREHENSIVE ENVIRONMENTAL DATA SYSTEM" ;
    rdfs:domain epa-frs:CEDS-Facility ;
    rdfs:subPropertyOf fio:ofIndustry .

epa-frs:ofIndustry.CERCLIS a owl:ObjectProperty ;
    rdfs:label "of Industry in CERCLIS" ;
    dcterms:description "connects a facility to an industry in COMPREHENSIVE ENVIRONMENTAL RESPONSE, COMPENSATION, AND LIABILITY INFORMATION SYSTEM" ;
    rdfs:domain epa-frs:CERCLIS-Facility ;
    rdfs:subPropertyOf fio:ofIndustry .

epa-frs:ofIndustry.CIM a owl:ObjectProperty ;
    rdfs:label "of Industry in CIM" ;
    dcterms:description "connects a facility to an industry in UTAH - COMMON IDENTIFIER MECHANISM" ;
    rdfs:domain epa-frs:CIM-Facility ;
    rdfs:subPropertyOf fio:ofIndustry .

epa-frs:ofIndustry.CNFRS a owl:ObjectProperty ;
    rdfs:label "of Industry in CNFRS" ;
    dcterms:description "connects a facility to an industry in CHEROKEE NATION FACILITY REGISTRY SYSTEM" ;
    rdfs:domain epa-frs:CNFRS-Facility ;
    rdfs:subPropertyOf fio:ofIndustry .

epa-frs:ofIndustry.CWNS a owl:ObjectProperty ;
    rdfs:label "of Industry in CWNS" ;
    dcterms:description "connects a facility to an industry in CLEAN WATERSHEDS NEEDS SURVEY" ;
    rdfs:domain epa-frs:CWNS-Facility ;
    rdfs:subPropertyOf fio:ofIndustry .

epa-frs:ofIndustry.DEN a owl:ObjectProperty ;
    rdfs:label "of Industry in DEN" ;
    dcterms:description "connects a facility to an industry in DELAWARE ENVIRONMENTAL NAVIGATOR" ;
    rdfs:domain epa-frs:DEN-Facility ;
    rdfs:subPropertyOf fio:ofIndustry .

epa-frs:ofIndustry.DTSC-ENVIROSTOR a owl:ObjectProperty ;
    rdfs:label "of Industry in DTSC-ENVIROSTOR" ;
    dcterms:description "connects a facility to an industry in CALIFORNIA - DEPARTMENT OF TOXIC SUBSTANCES CONTROL - ENVIROSTOR SYSTEM" ;
    rdfs:domain epa-frs:DTSC-ENVIROSTOR-Facility ;
    rdfs:subPropertyOf fio:ofIndustry .

epa-frs:ofIndustry.E-GGRT a owl:ObjectProperty ;
    rdfs:label "of Industry in E-GGRT" ;
    dcterms:description "connects a facility to an industry in ELECTRONIC GREENHOUSE GAS REPORTING TOOL (E-GGRT)" ;
    rdfs:domain epa-frs:E-GGRT-Facility ;
    rdfs:subPropertyOf fio:ofIndustry .

epa-frs:ofIndustry.ECRM a owl:ObjectProperty ;
    rdfs:label "of Industry in ECRM" ;
    dcterms:description "connects a facility to an industry in ENFORCEMENT CRIMINAL RECORDS MANAGEMENT" ;
    rdfs:domain epa-frs:ECRM-Facility ;
    rdfs:subPropertyOf fio:ofIndustry .

epa-frs:ofIndustry.EGRID a owl:ObjectProperty ;
    rdfs:label "of Industry in EGRID" ;
    dcterms:description "connects a facility to an industry in EMISSIONS & GENERATION RESOURCE INTEGRATED DATABASE" ;
    rdfs:domain epa-frs:EGRID-Facility ;
    rdfs:subPropertyOf fio:ofIndustry .

epa-frs:ofIndustry.EIA-860 a owl:ObjectProperty ;
    rdfs:label "of Industry in EIA-860" ;
    dcterms:description "connects a facility to an industry in ENERGY INFORMATION ADMINISTRATION-860 (EIA-860) DATABASE" ;
    rdfs:domain epa-frs:EIA-860-Facility ;
    rdfs:subPropertyOf fio:ofIndustry .

epa-frs:ofIndustry.EIS a owl:ObjectProperty ;
    rdfs:label "of Industry in EIS" ;
    dcterms:description "connects a facility to an industry in EMISSION INVENTORY SYSTEM (EIS)" ;
    rdfs:domain epa-frs:EIS-Facility ;
    rdfs:subPropertyOf fio:ofIndustry .

epa-frs:ofIndustry.EPS a owl:ObjectProperty ;
    rdfs:label "of Industry in EPS" ;
    dcterms:description "connects a facility to an industry in ELECTRONIC PERMIT SYSTEM" ;
    rdfs:domain epa-frs:EPS-Facility ;
    rdfs:subPropertyOf fio:ofIndustry .

epa-frs:ofIndustry.FARR a owl:ObjectProperty ;
    rdfs:label "of Industry in FARR" ;
    dcterms:description "connects a facility to an industry in FEDERAL AIR RULES FOR RESERVATIONS (FARR) REGISTRATION PROGRAM" ;
    rdfs:domain epa-frs:FARR-Facility ;
    rdfs:subPropertyOf fio:ofIndustry .

epa-frs:ofIndustry.FDM a owl:ObjectProperty ;
    rdfs:label "of Industry in FDM" ;
    dcterms:description "connects a facility to an industry in FLORIDA - FIESTA DATA MAINTENANCE" ;
    rdfs:domain epa-frs:FDM-Facility ;
    rdfs:subPropertyOf fio:ofIndustry .

epa-frs:ofIndustry.FFDOCKET a owl:ObjectProperty ;
    rdfs:label "of Industry in FFDOCKET" ;
    dcterms:description "connects a facility to an industry in FEDERAL FACILITY HAZARDOUS WASTE COMPLIANCE DOCKET" ;
    rdfs:domain epa-frs:FFDOCKET-Facility ;
    rdfs:subPropertyOf fio:ofIndustry .

epa-frs:ofIndustry.FFEP a owl:ObjectProperty ;
    rdfs:label "of Industry in FFEP" ;
    dcterms:description "connects a facility to an industry in FEDERAL FACILITIES RECOVERY AND REUSE OFFICE" ;
    rdfs:domain epa-frs:FFEP-Facility ;
    rdfs:subPropertyOf fio:ofIndustry .

epa-frs:ofIndustry.FIS a owl:ObjectProperty ;
    rdfs:label "of Industry in FIS" ;
    dcterms:description "connects a facility to an industry in NEW YORK - FACILITY INFORMATION SYSTEM" ;
    rdfs:domain epa-frs:FIS-Facility ;
    rdfs:subPropertyOf fio:ofIndustry .

epa-frs:ofIndustry.GEIMS a owl:ObjectProperty ;
    rdfs:label "of Industry in GEIMS" ;
    dcterms:description "connects a facility to an industry in GEORGIA - GEOGRAPHIC ENVIRONMENTAL INFORMATION MANAGEMENT SYSTEM" ;
    rdfs:domain epa-frs:GEIMS-Facility ;
    rdfs:subPropertyOf fio:ofIndustry .

epa-frs:ofIndustry.HI-EHW a owl:ObjectProperty ;
    rdfs:label "of Industry in HI-EHW" ;
    dcterms:description "connects a facility to an industry in HAWAII ENVIRONMENTAL HEALTH WAREHOUSE" ;
    rdfs:domain epa-frs:HI-EHW-Facility ;
    rdfs:subPropertyOf fio:ofIndustry .

epa-frs:ofIndustry.HWTS-DATAMART a owl:ObjectProperty ;
    rdfs:label "of Industry in HWTS-DATAMART" ;
    dcterms:description "connects a facility to an industry in HAZARDOUS WASTE TRACKING SYSTEM - DATAMART" ;
    rdfs:domain epa-frs:HWTS-DATAMART-Facility ;
    rdfs:subPropertyOf fio:ofIndustry .

epa-frs:ofIndustry.ICIS a owl:ObjectProperty ;
    rdfs:label "of Industry in ICIS" ;
    dcterms:description "connects a facility to an industry in INTEGRATED COMPLIANCE INFORMATION SYSTEM" ;
    rdfs:domain epa-frs:ICIS-Facility ;
    rdfs:subPropertyOf fio:ofIndustry .

epa-frs:ofIndustry.IDDEQ a owl:ObjectProperty ;
    rdfs:label "of Industry in IDDEQ" ;
    dcterms:description "connects a facility to an industry in IDAHO DEPARTMENT OF ENVIRONMENTAL QUALITY" ;
    rdfs:domain epa-frs:IDDEQ-Facility ;
    rdfs:subPropertyOf fio:ofIndustry .

epa-frs:ofIndustry.IDNR_EFD a owl:ObjectProperty ;
    rdfs:label "of Industry in IDNR_EFD" ;
    dcterms:description "connects a facility to an industry in IOWA DEPARTMENT OF NATURAL RESOURCES - ENVIRONMENTAL FACILITIES DATABASE" ;
    rdfs:domain epa-frs:IDNR_EFD-Facility ;
    rdfs:subPropertyOf fio:ofIndustry .

epa-frs:ofIndustry.IN-FRS a owl:ObjectProperty ;
    rdfs:label "of Industry in IN-FRS" ;
    dcterms:description "connects a facility to an industry in INDIANA - FACILITY REGISTRY SYSTEM" ;
    rdfs:domain epa-frs:IN-FRS-Facility ;
    rdfs:subPropertyOf fio:ofIndustry .

epa-frs:ofIndustry.IN-TEMPO a owl:ObjectProperty ;
    rdfs:label "of Industry in IN-TEMPO" ;
    dcterms:description "connects a facility to an industry in INDIANA-TOOLS FOR ENVIRONMENTAL MANAGEMENT AND PROTECTION ORGANIZATIONS" ;
    rdfs:domain epa-frs:IN-TEMPO-Facility ;
    rdfs:subPropertyOf fio:ofIndustry .

epa-frs:ofIndustry.ISD a owl:ObjectProperty ;
    rdfs:label "of Industry in ISD" ;
    dcterms:description "connects a facility to an industry in WYOMING - INDUSTRIAL SITING DIVISION" ;
    rdfs:domain epa-frs:ISD-Facility ;
    rdfs:subPropertyOf fio:ofIndustry .

epa-frs:ofIndustry.KS-FP a owl:ObjectProperty ;
    rdfs:label "of Industry in KS-FP" ;
    dcterms:description "connects a facility to an industry in KANSAS - FACILITY PROFILE" ;
    rdfs:domain epa-frs:KS-FP-Facility ;
    rdfs:subPropertyOf fio:ofIndustry .

epa-frs:ofIndustry.KY-TEMPO a owl:ObjectProperty ;
    rdfs:label "of Industry in KY-TEMPO" ;
    dcterms:description "connects a facility to an industry in KENTUCKY - TOOLS FOR ENVIRONMENTAL MANAGEMENT AND PROTECTION ORGANIZATIONS" ;
    rdfs:domain epa-frs:KY-TEMPO-Facility ;
    rdfs:subPropertyOf fio:ofIndustry .

epa-frs:ofIndustry.LA-TEMPO a owl:ObjectProperty ;
    rdfs:label "of Industry in LA-TEMPO" ;
    dcterms:description "connects a facility to an industry in LOUISIANA - TOOLS FOR ENVIRONMENTAL MANAGEMENT AND PROTECTION ORGANIZATIONS" ;
    rdfs:domain epa-frs:LA-TEMPO-Facility ;
    rdfs:subPropertyOf fio:ofIndustry .

epa-frs:ofIndustry.LMOP a owl:ObjectProperty ;
    rdfs:label "of Industry in LMOP" ;
    dcterms:description "connects a facility to an industry in LANDFILL METHANE OUTREACH PROGRAM" ;
    rdfs:domain epa-frs:LMOP-Facility ;
    rdfs:subPropertyOf fio:ofIndustry .

epa-frs:ofIndustry.LUST-ARRA a owl:ObjectProperty ;
    rdfs:label "of Industry in LUST-ARRA" ;
    dcterms:description "connects a facility to an industry in LEAKING UNDERGROUND STORAGE TANK (LUST) ¿ AMERICAN RECOVERY AND REINVESTMENT ACT (ARRA)" ;
    rdfs:domain epa-frs:LUST-ARRA-Facility ;
    rdfs:subPropertyOf fio:ofIndustry .

epa-frs:ofIndustry.MA-EPICS a owl:ObjectProperty ;
    rdfs:label "of Industry in MA-EPICS" ;
    dcterms:description "connects a facility to an industry in MASSACHUSETTS - ENVIRONMENTAL PROTECTION INTEGRATED COMPUTER SYSTEM" ;
    rdfs:domain epa-frs:MA-EPICS-Facility ;
    rdfs:subPropertyOf fio:ofIndustry .

epa-frs:ofIndustry.MD-EPSC a owl:ObjectProperty ;
    rdfs:label "of Industry in MD-EPSC" ;
    dcterms:description "connects a facility to an industry in MARYLAND - ENVIRONMENTAL PERMIT SERVICE CENTER" ;
    rdfs:domain epa-frs:MD-EPSC-Facility ;
    rdfs:subPropertyOf fio:ofIndustry .

epa-frs:ofIndustry.MD-PEMIS a owl:ObjectProperty ;
    rdfs:label "of Industry in MD-PEMIS" ;
    dcterms:description "connects a facility to an industry in MARYLAND - PERMANENT (AIR) EMISSION" ;
    rdfs:domain epa-frs:MD-PEMIS-Facility ;
    rdfs:subPropertyOf fio:ofIndustry .

epa-frs:ofIndustry.MD-RCRA a owl:ObjectProperty ;
    rdfs:label "of Industry in MD-RCRA" ;
    dcterms:description "connects a facility to an industry in MARYLAND-RESOURCE CONVERSATION AND RECOVERY ACT DATABASE" ;
    rdfs:domain epa-frs:MD-RCRA-Facility ;
    rdfs:subPropertyOf fio:ofIndustry .

epa-frs:ofIndustry.MD-TEMPO a owl:ObjectProperty ;
    rdfs:label "of Industry in MD-TEMPO" ;
    dcterms:description "connects a facility to an industry in MARYLAND - TOOLS FOR ENVIRONMENTAL MANAGEMENT AND PROTECTION ORGANIZATIONS (TEMPO)" ;
    rdfs:domain epa-frs:MD-TEMPO-Facility ;
    rdfs:subPropertyOf fio:ofIndustry .

epa-frs:ofIndustry.ME-EFIS a owl:ObjectProperty ;
    rdfs:label "of Industry in ME-EFIS" ;
    dcterms:description "connects a facility to an industry in MAINE - ENVIRONMENTAL FACILITY INFORMATION SYSTEM" ;
    rdfs:domain epa-frs:ME-EFIS-Facility ;
    rdfs:subPropertyOf fio:ofIndustry .

epa-frs:ofIndustry.MERI-FIS a owl:ObjectProperty ;
    rdfs:label "of Industry in MERI-FIS" ;
    dcterms:description "connects a facility to an industry in MEADOWLANDS ENVIRONMENTAL RESEARCH INSTITUTE – FACILITY INFORMATION SYSTEM" ;
    rdfs:domain epa-frs:MERI-FIS-Facility ;
    rdfs:subPropertyOf fio:ofIndustry .

epa-frs:ofIndustry.MN-TEMPO a owl:ObjectProperty ;
    rdfs:label "of Industry in MN-TEMPO" ;
    dcterms:description "connects a facility to an industry in MINNESOTA - PERMITTING, COMPLIANCE, AND ENFORCEMENT INFORMATION MANAGEMENT SYSTEM" ;
    rdfs:domain epa-frs:MN-TEMPO-Facility ;
    rdfs:subPropertyOf fio:ofIndustry .

epa-frs:ofIndustry.MO-DNR a owl:ObjectProperty ;
    rdfs:label "of Industry in MO-DNR" ;
    dcterms:description "connects a facility to an industry in MISSOURI DEPARTMENT OF NATURAL RESOURCES" ;
    rdfs:domain epa-frs:MO-DNR-Facility ;
    rdfs:subPropertyOf fio:ofIndustry .

epa-frs:ofIndustry.MS-ENSITE a owl:ObjectProperty ;
    rdfs:label "of Industry in MS-ENSITE" ;
    dcterms:description "connects a facility to an industry in MISSISSIPPI - TOOLS FOR ENVIRONMENTAL MANAGEMENT AND PROTECTION ORGANIZATIONS" ;
    rdfs:domain epa-frs:MS-ENSITE-Facility ;
    rdfs:subPropertyOf fio:ofIndustry .

epa-frs:ofIndustry.MT-CEDARS a owl:ObjectProperty ;
    rdfs:label "of Industry in MT-CEDARS" ;
    dcterms:description "connects a facility to an industry in MONTANA - CONSOLIDATED ENVIRONMENTAL DATA ACQUISITION AND RETRIEVAL SYSTEM" ;
    rdfs:domain epa-frs:MT-CEDARS-Facility ;
    rdfs:subPropertyOf fio:ofIndustry .

epa-frs:ofIndustry.NC-FITS a owl:ObjectProperty ;
    rdfs:label "of Industry in NC-FITS" ;
    dcterms:description "connects a facility to an industry in NORTH CAROLINA - FACILITY IDENTIFICATION TEMPLATE FOR STATES" ;
    rdfs:domain epa-frs:NC-FITS-Facility ;
    rdfs:subPropertyOf fio:ofIndustry .

epa-frs:ofIndustry.NCDB a owl:ObjectProperty ;
    rdfs:label "of Industry in NCDB" ;
    dcterms:description "connects a facility to an industry in NATIONAL COMPLIANCE DATABASE" ;
    rdfs:domain epa-frs:NCDB-Facility ;
    rdfs:subPropertyOf fio:ofIndustry .

epa-frs:ofIndustry.ND-FP a owl:ObjectProperty ;
    rdfs:label "of Industry in ND-FP" ;
    dcterms:description "connects a facility to an industry in NORTH DAKOTA - FACILITY PROFILE" ;
    rdfs:domain epa-frs:ND-FP-Facility ;
    rdfs:subPropertyOf fio:ofIndustry .

epa-frs:ofIndustry.NDEQ a owl:ObjectProperty ;
    rdfs:label "of Industry in NDEQ" ;
    dcterms:description "connects a facility to an industry in NEBRASKA DEPARTMENT OF ENVIRONMENTAL QUALITY" ;
    rdfs:domain epa-frs:NDEQ-Facility ;
    rdfs:subPropertyOf fio:ofIndustry .

epa-frs:ofIndustry.NEI a owl:ObjectProperty ;
    rdfs:label "of Industry in NEI" ;
    dcterms:description "connects a facility to an industry in NATIONAL EMISSIONS INVENTORY" ;
    rdfs:domain epa-frs:NEI-Facility ;
    rdfs:subPropertyOf fio:ofIndustry .

epa-frs:ofIndustry.NH-DES a owl:ObjectProperty ;
    rdfs:label "of Industry in NH-DES" ;
    dcterms:description "connects a facility to an industry in NEW HAMPSHIRE - DEPARTMENT OF ENVIRONMENTAL SERVICES" ;
    rdfs:domain epa-frs:NH-DES-Facility ;
    rdfs:subPropertyOf fio:ofIndustry .

epa-frs:ofIndustry.NJ-NJEMS a owl:ObjectProperty ;
    rdfs:label "of Industry in NJ-NJEMS" ;
    dcterms:description "connects a facility to an industry in NEW JERSEY - NEW JERSEY ENVIRONMENTAL MANAGEMENT SYSTEM" ;
    rdfs:domain epa-frs:NJ-NJEMS-Facility ;
    rdfs:subPropertyOf fio:ofIndustry .

epa-frs:ofIndustry.NM-TEMPO a owl:ObjectProperty ;
    rdfs:label "of Industry in NM-TEMPO" ;
    dcterms:description "connects a facility to an industry in NEW MEXICO-TOOLS FOR ENVIRONMENTAL MANAGEMENT AND PROTECTION ORGANIZATIONS" ;
    rdfs:domain epa-frs:NM-TEMPO-Facility ;
    rdfs:subPropertyOf fio:ofIndustry .

epa-frs:ofIndustry.NNEMS a owl:ObjectProperty ;
    rdfs:label "of Industry in NNEMS" ;
    dcterms:description "connects a facility to an industry in NAVAJO NATION ENVIRONMENTAL MANAGEMENT SYSTEM" ;
    rdfs:domain epa-frs:NNEMS-Facility ;
    rdfs:subPropertyOf fio:ofIndustry .

epa-frs:ofIndustry.NPDES a owl:ObjectProperty ;
    rdfs:label "of Industry in NPDES" ;
    dcterms:description "connects a facility to an industry in NATIONAL POLLUTANT DISCHARGE ELIMINATION SYSTEM (ICIS-NPDES)" ;
    rdfs:domain epa-frs:NPDES-Facility ;
    rdfs:subPropertyOf fio:ofIndustry .

epa-frs:ofIndustry.NV-FP a owl:ObjectProperty ;
    rdfs:label "of Industry in NV-FP" ;
    dcterms:description "connects a facility to an industry in NEVADA - FACILITY PROFILE" ;
    rdfs:domain epa-frs:NV-FP-Facility ;
    rdfs:subPropertyOf fio:ofIndustry .

epa-frs:ofIndustry.OH-CORE a owl:ObjectProperty ;
    rdfs:label "of Industry in OH-CORE" ;
    dcterms:description "connects a facility to an industry in OHIO - CORE FACILITY INFORMATION" ;
    rdfs:domain epa-frs:OH-CORE-Facility ;
    rdfs:subPropertyOf fio:ofIndustry .

epa-frs:ofIndustry.OR-DEQ a owl:ObjectProperty ;
    rdfs:label "of Industry in OR-DEQ" ;
    dcterms:description "connects a facility to an industry in OREGON - DEPARTMENT OF ENVIRONMENTAL QUALITY" ;
    rdfs:domain epa-frs:OR-DEQ-Facility ;
    rdfs:subPropertyOf fio:ofIndustry .

epa-frs:ofIndustry.OSHA-OIS a owl:ObjectProperty ;
    rdfs:label "of Industry in OSHA-OIS" ;
    dcterms:description "connects a facility to an industry in OCCUPATIONAL SAFETY AND HEALTH ADMINISTRATION INFORMATION SYSTEM" ;
    rdfs:domain epa-frs:OSHA-OIS-Facility ;
    rdfs:subPropertyOf fio:ofIndustry .

epa-frs:ofIndustry.OTAQREG a owl:ObjectProperty ;
    rdfs:label "of Industry in OTAQREG" ;
    dcterms:description "connects a facility to an industry in OFFICE OF TRANSPORTATION AND AIR QUALITY FUELS REGISTRATION" ;
    rdfs:domain epa-frs:OTAQREG-Facility ;
    rdfs:subPropertyOf fio:ofIndustry .

epa-frs:ofIndustry.PA-EFACTS a owl:ObjectProperty ;
    rdfs:label "of Industry in PA-EFACTS" ;
    dcterms:description "connects a facility to an industry in PENNSYLVANIA - ENVIRONMENTAL FACILITY APPLICATION COMPLIANCE TRACKING SYSTEM" ;
    rdfs:domain epa-frs:PA-EFACTS-Facility ;
    rdfs:subPropertyOf fio:ofIndustry .

epa-frs:ofIndustry.PDS a owl:ObjectProperty ;
    rdfs:label "of Industry in PDS" ;
    dcterms:description "connects a facility to an industry in PERMIT DATA SYSTEM" ;
    rdfs:domain epa-frs:PDS-Facility ;
    rdfs:subPropertyOf fio:ofIndustry .

epa-frs:ofIndustry.PERMIT-TRACKING a owl:ObjectProperty ;
    rdfs:label "of Industry in PERMIT TRACKING" ;
    dcterms:description "connects a facility to an industry in ALBAMA - PERMIT TRACKING" ;
    rdfs:domain epa-frs:PERMIT-TRACKING-Facility ;
    rdfs:subPropertyOf fio:ofIndustry .

epa-frs:ofIndustry.RADINFO a owl:ObjectProperty ;
    rdfs:label "of Industry in RADINFO" ;
    dcterms:description "connects a facility to an industry in RADIATION INFORMATION SYSTEM" ;
    rdfs:domain epa-frs:RADINFO-Facility ;
    rdfs:subPropertyOf fio:ofIndustry .

epa-frs:ofIndustry.RBLC a owl:ObjectProperty ;
    rdfs:label "of Industry in RBLC" ;
    dcterms:description "connects a facility to an industry in RACT/BACT/LAER CLEARINGHOUSE" ;
    rdfs:domain epa-frs:RBLC-Facility ;
    rdfs:subPropertyOf fio:ofIndustry .

epa-frs:ofIndustry.RCRAINFO a owl:ObjectProperty ;
    rdfs:label "of Industry in RCRAINFO" ;
    dcterms:description "connects a facility to an industry in RESOURCE CONSERVATION AND RECOVERY ACT INFORMATION SYSTEM" ;
    rdfs:domain epa-frs:RCRAINFO-Facility ;
    rdfs:subPropertyOf fio:ofIndustry .

epa-frs:ofIndustry.REGION a owl:ObjectProperty ;
    rdfs:label "of Industry in REGION" ;
    dcterms:description "connects a facility to an industry in REGION" ;
    rdfs:domain epa-frs:REGION-Facility ;
    rdfs:subPropertyOf fio:ofIndustry .

epa-frs:ofIndustry.RFS a owl:ObjectProperty ;
    rdfs:label "of Industry in RFS" ;
    dcterms:description "connects a facility to an industry in RENEWABLE FUEL STANDARD" ;
    rdfs:domain epa-frs:RFS-Facility ;
    rdfs:subPropertyOf fio:ofIndustry .

epa-frs:ofIndustry.RI-PLOVER a owl:ObjectProperty ;
    rdfs:label "of Industry in RI-PLOVER" ;
    dcterms:description "connects a facility to an industry in RHODE ISLAND - PERMITS, LICENSES AND OTHER VITAL ENVIRONMENTAL RECORDS" ;
    rdfs:domain epa-frs:RI-PLOVER-Facility ;
    rdfs:subPropertyOf fio:ofIndustry .

epa-frs:ofIndustry.RMP a owl:ObjectProperty ;
    rdfs:label "of Industry in RMP" ;
    dcterms:description "connects a facility to an industry in RISK MANAGEMENT PLAN" ;
    rdfs:domain epa-frs:RMP-Facility ;
    rdfs:subPropertyOf fio:ofIndustry .

epa-frs:ofIndustry.SC-EFIS a owl:ObjectProperty ;
    rdfs:label "of Industry in SC-EFIS" ;
    dcterms:description "connects a facility to an industry in SOUTH CAROLINA - ENVIRONMENTAL FACILITY INFORMATION SYSTEM" ;
    rdfs:domain epa-frs:SC-EFIS-Facility ;
    rdfs:subPropertyOf fio:ofIndustry .

epa-frs:ofIndustry.SEMS a owl:ObjectProperty ;
    rdfs:label "of Industry in SEMS" ;
    dcterms:description "connects a facility to an industry in SUPERFUND ENTERPRISE MANAGEMENT SYSTEM" ;
    rdfs:domain epa-frs:SEMS-Facility ;
    rdfs:subPropertyOf fio:ofIndustry .

epa-frs:ofIndustry.SFDW a owl:ObjectProperty ;
    rdfs:label "of Industry in SFDW" ;
    dcterms:description "connects a facility to an industry in SAFE DRINKING WATER INFORMATION SYSTEM" ;
    rdfs:domain epa-frs:SFDW-Facility ;
    rdfs:subPropertyOf fio:ofIndustry .

epa-frs:ofIndustry.SIMS a owl:ObjectProperty ;
    rdfs:label "of Industry in SIMS" ;
    dcterms:description "connects a facility to an industry in CT - SITE INFORMATION MANAGEMENT SYSTEM" ;
    rdfs:domain epa-frs:SIMS-Facility ;
    rdfs:subPropertyOf fio:ofIndustry .

epa-frs:ofIndustry.SRPMICEMS a owl:ObjectProperty ;
    rdfs:label "of Industry in SRPMICEMS" ;
    dcterms:description "connects a facility to an industry in SALT RIVER PIMA-MARICOPA INDIAN COMMUNITY ENVIRONMENTAL MANAGEMENT SYSTEM" ;
    rdfs:domain epa-frs:SRPMICEMS-Facility ;
    rdfs:subPropertyOf fio:ofIndustry .

epa-frs:ofIndustry.SSTS a owl:ObjectProperty ;
    rdfs:label "of Industry in SSTS" ;
    dcterms:description "connects a facility to an industry in SECTION SEVEN TRACKING SYSTEM" ;
    rdfs:domain epa-frs:SSTS-Facility ;
    rdfs:subPropertyOf fio:ofIndustry .

epa-frs:ofIndustry.STATE a owl:ObjectProperty ;
    rdfs:label "of Industry in STATE" ;
    dcterms:description "connects a facility to an industry in STATE SYSTEMS" ;
    rdfs:domain epa-frs:STATE-Facility ;
    rdfs:subPropertyOf fio:ofIndustry .

epa-frs:ofIndustry.SWIPR a owl:ObjectProperty ;
    rdfs:label "of Industry in SWIPR" ;
    dcterms:description "connects a facility to an industry in SUBPART W IMPOUNDMENT PHOTOGRAPHIC REPORTING" ;
    rdfs:domain epa-frs:SWIPR-Facility ;
    rdfs:subPropertyOf fio:ofIndustry .

epa-frs:ofIndustry.TEST a owl:ObjectProperty ;
    rdfs:label "of Industry in TEST" ;
    dcterms:description "connects a facility to an industry in TEST PROGRAM FOR CDX" ;
    rdfs:domain epa-frs:TEST-Facility ;
    rdfs:subPropertyOf fio:ofIndustry .

epa-frs:ofIndustry.TRIS a owl:ObjectProperty ;
    rdfs:label "of Industry in TRIS" ;
    dcterms:description "connects a facility to an industry in TOXICS RELEASE INVENTORY SYSTEM" ;
    rdfs:domain epa-frs:TRIS-Facility ;
    rdfs:subPropertyOf fio:ofIndustry .

epa-frs:ofIndustry.TSCA a owl:ObjectProperty ;
    rdfs:label "of Industry in TSCA" ;
    dcterms:description "connects a facility to an industry in TOXIC SUBSTANCES CONTROL ACT" ;
    rdfs:domain epa-frs:TSCA-Facility ;
    rdfs:subPropertyOf fio:ofIndustry .

epa-frs:ofIndustry.TX-TCEQ-ACR a owl:ObjectProperty ;
    rdfs:label "of Industry in TX-TCEQ ACR" ;
    dcterms:description "connects a facility to an industry in TEXAS COMMISSION ON ENVIRONMENTAL QUALITY - AGENCY CENTRAL REGISTRY" ;
    rdfs:domain epa-frs:TX-TCEQ-ACR-Facility ;
    rdfs:subPropertyOf fio:ofIndustry .

epa-frs:ofIndustry.UORS a owl:ObjectProperty ;
    rdfs:label "of Industry in UORS" ;
    dcterms:description "connects a facility to an industry in CALIFORNIA - USED OIL RECYCLING SYSTEM" ;
    rdfs:domain epa-frs:UORS-Facility ;
    rdfs:subPropertyOf fio:ofIndustry .

epa-frs:ofIndustry.UST a owl:ObjectProperty ;
    rdfs:label "of Industry in UST" ;
    dcterms:description "connects a facility to an industry in UNDERGROUND STORAGE TANK" ;
    rdfs:domain epa-frs:UST-Facility ;
    rdfs:subPropertyOf fio:ofIndustry .

epa-frs:ofIndustry.WA-FSIS a owl:ObjectProperty ;
    rdfs:label "of Industry in WA-FSIS" ;
    dcterms:description "connects a facility to an industry in WASHINGTON - FACILITY / SITE IDENTIFICATION SYSTEM" ;
    rdfs:domain epa-frs:WA-FSIS-Facility ;
    rdfs:subPropertyOf fio:ofIndustry .

epa-frs:ofIndustry.WI-ESR a owl:ObjectProperty ;
    rdfs:label "of Industry in WI-ESR" ;
    dcterms:description "connects a facility to an industry in WISCONSIN - ENVIRONMENTAL SYSTEM REGISTRY" ;
    rdfs:domain epa-frs:WI-ESR-Facility ;
    rdfs:subPropertyOf fio:ofIndustry .

epa-frs-data:d.Agency.C0067 a epa-frs:Agency.State,
        owl:NamedIndividual ;
    rdfs:label "United States Mission to the United Nations" .

epa-frs-data:d.Agency.C0078 a epa-frs:Agency,
        owl:NamedIndividual ;
    rdfs:label "Federal Reserve System" .

epa-frs-data:d.Agency.C0400 a epa-frs:Agency,
        owl:NamedIndividual ;
    rdfs:label "Government Publishing Office" .

epa-frs-data:d.Agency.C1016 a epa-frs:Agency.Agriculture,
        owl:NamedIndividual ;
    rdfs:label "Agricultural Marketing Service" .

epa-frs-data:d.Agency.C1017 a epa-frs:Agency.Agriculture,
        owl:NamedIndividual ;
    rdfs:label "Agricultural Research Service" .

epa-frs-data:d.Agency.C1018 a epa-frs:Agency.Agriculture,
        owl:NamedIndividual ;
    rdfs:label "Animal and Plant Health Inspection Service" .

epa-frs-data:d.Agency.C1019 a epa-frs:Agency.Agriculture,
        owl:NamedIndividual ;
    rdfs:label "Farm Service Agency" .

epa-frs-data:d.Agency.C1020 a epa-frs:Agency.Agriculture,
        owl:NamedIndividual ;
    rdfs:label "Food Safety and Inspection Service" .

epa-frs-data:d.Agency.C1021 a epa-frs:Agency.Agriculture,
        owl:NamedIndividual ;
    rdfs:label "Natural Institute of Food and Agriculture" .

epa-frs-data:d.Agency.C1022 a epa-frs:Agency.Agriculture,
        owl:NamedIndividual ;
    rdfs:label "Natural Resources Conservation Service" .

epa-frs-data:d.Agency.C1023 a epa-frs:Agency.Agriculture,
        owl:NamedIndividual ;
    rdfs:label "Rural Development" .

epa-frs-data:d.Agency.C1024 a epa-frs:Agency,
        owl:NamedIndividual ;
    rdfs:label "Amtrak" .

epa-frs-data:d.Agency.C1026 a epa-frs:Agency.Commerce,
        owl:NamedIndividual ;
    rdfs:label "Census Bureau" .

epa-frs-data:d.Agency.C1027 a epa-frs:Agency.Commerce,
        owl:NamedIndividual ;
    rdfs:label "Patent and Trademark Office" .

epa-frs-data:d.Agency.C1028 a epa-frs:Agency.Commerce,
        owl:NamedIndividual ;
    rdfs:label "National Institute of Standards and Technology (NIST)" .

epa-frs-data:d.Agency.C1029 a epa-frs:Agency.Commerce,
        owl:NamedIndividual ;
    rdfs:label "National Technical Information Service" .

epa-frs-data:d.Agency.C1030 a epa-frs:Agency.Commerce,
        owl:NamedIndividual ;
    rdfs:label "National Telecommunications and Information Administration" .

epa-frs-data:d.Agency.C1031 a epa-frs:Agency,
        owl:NamedIndividual ;
    rdfs:label "Corporation for National and Community Service" .

epa-frs-data:d.Agency.C1043 a epa-frs:Agency,
        owl:NamedIndividual ;
    rdfs:label "Denali Commission" .

epa-frs-data:d.Agency.C1065 a epa-frs:Agency.HealthandHumanServices,
        owl:NamedIndividual ;
    rdfs:label "Administration for Children & Families" .

epa-frs-data:d.Agency.C1066 a epa-frs:Agency.HealthandHumanServices,
        owl:NamedIndividual ;
    rdfs:label "Center for Disease Control and Prevention" .

epa-frs-data:d.Agency.C1067 a epa-frs:Agency.HealthandHumanServices,
        owl:NamedIndividual ;
    rdfs:label "Food and Drug Administration" .

epa-frs-data:d.Agency.C1068 a epa-frs:Agency.HealthandHumanServices,
        owl:NamedIndividual ;
    rdfs:label "Indian Health Services" .

epa-frs-data:d.Agency.C1069 a epa-frs:Agency.HealthandHumanServices,
        owl:NamedIndividual ;
    rdfs:label "National Institutes of Health" .

epa-frs-data:d.Agency.C1070 a epa-frs:Agency.HealthandHumanServices,
        owl:NamedIndividual ;
    rdfs:label "Substance Abuse and Mental Health Services Administration" .

epa-frs-data:d.Agency.C1071 a epa-frs:Agency.HomelandSecurity,
        owl:NamedIndividual ;
    rdfs:label "Citizenship and Immigration Services" .

epa-frs-data:d.Agency.C1072 a epa-frs:Agency.HomelandSecurity,
        owl:NamedIndividual ;
    rdfs:label "Federal Law Enforcement Training Centers" .

epa-frs-data:d.Agency.C1073 a epa-frs:Agency.HomelandSecurity,
        owl:NamedIndividual ;
    rdfs:label "Federal Protective Service" .

epa-frs-data:d.Agency.C1074 a epa-frs:Agency.HousingandUrbanDevelopment,
        owl:NamedIndividual ;
    rdfs:label "Office of Housing" .

epa-frs-data:d.Agency.C1075 a epa-frs:Agency.HousingandUrbanDevelopment,
        owl:NamedIndividual ;
    rdfs:label "Office of Public and Indian Housing" .

epa-frs-data:d.Agency.C1076 a epa-frs:Agency.Interior,
        owl:NamedIndividual ;
    rdfs:label "Bureau of Safety and Environmental Enforcement" .

epa-frs-data:d.Agency.C1077 a epa-frs:Agency.Interior,
        owl:NamedIndividual ;
    rdfs:label "Bureau of Ocean Energy Management" .

epa-frs-data:d.Agency.C1078 a epa-frs:Agency.Interior,
        owl:NamedIndividual ;
    rdfs:label "Office of Surface Mining, Reclamation and Enforcement" .

epa-frs-data:d.Agency.C1080 a epa-frs:Agency.Justice,
        owl:NamedIndividual ;
    rdfs:label "Federal Bureau of Investigations" .

epa-frs-data:d.Agency.C1081 a epa-frs:Agency.Justice,
        owl:NamedIndividual ;
    rdfs:label "Drug Enforcement Administration" .

epa-frs-data:d.Agency.C1082 a epa-frs:Agency.Justice,
        owl:NamedIndividual ;
    rdfs:label "Marshals Service" .

epa-frs-data:d.Agency.C1083 a epa-frs:Agency.Justice,
        owl:NamedIndividual ;
    rdfs:label "National Institute of Corrections" .

epa-frs-data:d.Agency.C1084 a epa-frs:Agency.Justice,
        owl:NamedIndividual ;
    rdfs:label "National Institute of Justice" .

epa-frs-data:d.Agency.C1085 a epa-frs:Agency.Labor,
        owl:NamedIndividual ;
    rdfs:label "Employment and Training Administration" .

epa-frs-data:d.Agency.C1086 a epa-frs:Agency.Labor,
        owl:NamedIndividual ;
    rdfs:label "Mine Safety and Health Administration" .

epa-frs-data:d.Agency.C1087 a epa-frs:Agency.Labor,
        owl:NamedIndividual ;
    rdfs:label "Occupational Safety and Health Administration" .

epa-frs-data:d.Agency.C1088 a epa-frs:Agency.Labor,
        owl:NamedIndividual ;
    rdfs:label "Veterans Employment and Training Service" .

epa-frs-data:d.Agency.C1089 a epa-frs:Agency,
        owl:NamedIndividual ;
    rdfs:label "Nuclear Regulatory Commission" .

epa-frs-data:d.Agency.C1090 a epa-frs:Agency,
        owl:NamedIndividual ;
    rdfs:label "Office of Management and Budget" .

epa-frs-data:d.Agency.C1091 a epa-frs:Agency,
        owl:NamedIndividual ;
    rdfs:label "Office of Personnel Management" .

epa-frs-data:d.Agency.C1092 a epa-frs:Agency,
        owl:NamedIndividual ;
    rdfs:label "Peace Corps" .

epa-frs-data:d.Agency.C1093 a epa-frs:Agency.State,
        owl:NamedIndividual ;
    rdfs:label "Bureau of Consular Affairs" .

epa-frs-data:d.Agency.C1094 a epa-frs:Agency.State,
        owl:NamedIndividual ;
    rdfs:label "Foreign Service Institute" .

epa-frs-data:d.Agency.C1096 a epa-frs:Agency.Transportation,
        owl:NamedIndividual ;
    rdfs:label "Federal Highway Administration" .

epa-frs-data:d.Agency.C1097 a epa-frs:Agency.Transportation,
        owl:NamedIndividual ;
    rdfs:label "Federal Motor Carrier Safety Administration" .

epa-frs-data:d.Agency.C1098 a epa-frs:Agency.Transportation,
        owl:NamedIndividual ;
    rdfs:label "Federal Railroad Administration" .

epa-frs-data:d.Agency.C1099 a epa-frs:Agency.Transportation,
        owl:NamedIndividual ;
    rdfs:label "Federal Transit Administration" .

epa-frs-data:d.Agency.C1100 a epa-frs:Agency.Transportation,
        owl:NamedIndividual ;
    rdfs:label "Maritime Administration" .

epa-frs-data:d.Agency.C1101 a epa-frs:Agency.Transportation,
        owl:NamedIndividual ;
    rdfs:label "National Highway Traffic Safety Administration" .

epa-frs-data:d.Agency.C1102 a epa-frs:Agency.Transportation,
        owl:NamedIndividual ;
    rdfs:label "Pipeline and Hazardous Materials Safety Administration" .

epa-frs-data:d.Agency.C1103 a epa-frs:Agency.Transportation,
        owl:NamedIndividual ;
    rdfs:label " St. Lawrence Seaway Development Corporation" .

epa-frs-data:d.Agency.C1104 a epa-frs:Agency.Transportation,
        owl:NamedIndividual ;
    rdfs:label "Volpe Center" .

epa-frs-data:d.Agency.C1105 a epa-frs:Agency.Treasury,
        owl:NamedIndividual ;
    rdfs:label "Mint" .

epa-frs-data:d.Agency.C1106 a epa-frs:Agency.Treasury,
        owl:NamedIndividual ;
    rdfs:label "Alcohol and Tobacco Tax and Trade Bureau" .

epa-frs-data:d.Agency.C1107 a epa-frs:Agency.Treasury,
        owl:NamedIndividual ;
    rdfs:label "Bureau of Engraving and Printing" .

epa-frs-data:d.Agency.C1108 a epa-frs:Agency.Treasury,
        owl:NamedIndividual ;
    rdfs:label "Internal Revenue Service" .

epa-frs-data:d.Agency.C1109 a epa-frs:Agency,
        owl:NamedIndividual ;
    rdfs:label "Trade and Development Agency" .

epa-frs-data:d.Agency.C1110 a epa-frs:Agency,
        owl:NamedIndividual ;
    rdfs:label "Agency for International Development" .

epa-frs-data:d.Agency.C1111 a epa-frs:Agency,
        owl:NamedIndividual ;
    rdfs:label "Agency for Global Media" .

epa-frs-data:d.Agency.C1113 a epa-frs:Agency,
        owl:NamedIndividual ;
    rdfs:label "International Trade Commission" .

epa-frs-data:d.Agency.C1114 a epa-frs:Agency.VeteransAffairs,
        owl:NamedIndividual ;
    rdfs:label "Veterans Health Administratioin" .

epa-frs-data:d.Agency.C1115 a epa-frs:Agency.VeteransAffairs,
        owl:NamedIndividual ;
    rdfs:label "National Cemetery Administration" .

epa-frs-data:d.Agency.C1116 a epa-frs:Agency.VeteransAffairs,
        owl:NamedIndividual ;
    rdfs:label "Office of Acquisition, Logistics and Construction" .

epa-frs-data:d.Agency.C1117 a epa-frs:Agency.HomelandSecurity,
        owl:NamedIndividual ;
    rdfs:label "Immigration and Customs Enforcement" .

epa-frs-data:d.Agency.C1118 a epa-frs:Agency.HomelandSecurity,
        owl:NamedIndividual ;
    rdfs:label "Transportation Security Administration" .

epa-frs-data:d.Agency.C1200 a epa-frs:Agency,
        owl:NamedIndividual ;
    rdfs:label "Agriculture" .

epa-frs-data:d.Agency.C1223 a epa-frs:Agency.Agriculture,
        owl:NamedIndividual ;
    rdfs:label "Forest Service" .

epa-frs-data:d.Agency.C1224 a epa-frs:Agency.Agriculture,
        owl:NamedIndividual ;
    rdfs:label "Office of Operations" .

epa-frs-data:d.Agency.C1300 a epa-frs:Agency,
        owl:NamedIndividual ;
    rdfs:label "Commerce" .

epa-frs-data:d.Agency.C1314 a epa-frs:Agency.Commerce,
        owl:NamedIndividual ;
    rdfs:label "National Oceanic & Atmospheric Administration" .

epa-frs-data:d.Agency.C1400 a epa-frs:Agency,
        owl:NamedIndividual ;
    rdfs:label "Interior" .

epa-frs-data:d.Agency.C1407 a epa-frs:Agency.Interior,
        owl:NamedIndividual ;
    rdfs:label "Geological Survey" .

epa-frs-data:d.Agency.C1409 a epa-frs:Agency.Interior,
        owl:NamedIndividual ;
    rdfs:label "Bureau of Indian Affairs" .

epa-frs-data:d.Agency.C1410 a epa-frs:Agency.Interior,
        owl:NamedIndividual ;
    rdfs:label "Bureau of Indian Education" .

epa-frs-data:d.Agency.C1411 a epa-frs:Agency.Interior,
        owl:NamedIndividual ;
    rdfs:label "Bureau of Land Management" .

epa-frs-data:d.Agency.C1417 a epa-frs:Agency.Interior,
        owl:NamedIndividual ;
    rdfs:label "National Park Service" .

epa-frs-data:d.Agency.C1423 a epa-frs:Agency.Interior,
        owl:NamedIndividual ;
    rdfs:label "Bureau of Reclamation" .

epa-frs-data:d.Agency.C1436 a epa-frs:Agency.Interior,
        owl:NamedIndividual ;
    rdfs:label "Fish and Wildlife Service" .

epa-frs-data:d.Agency.C1500 a epa-frs:Agency,
        owl:NamedIndividual ;
    rdfs:label "Justice" .

epa-frs-data:d.Agency.C1519 a epa-frs:Agency.Justice,
        owl:NamedIndividual ;
    rdfs:label "Bureau of Prisons" .

epa-frs-data:d.Agency.C1600 a epa-frs:Agency,
        owl:NamedIndividual ;
    rdfs:label "Labor" .

epa-frs-data:d.Agency.C1800 a epa-frs:Agency,
        owl:NamedIndividual ;
    rdfs:label "Postal Service" .

epa-frs-data:d.Agency.C1900 a epa-frs:Agency,
        owl:NamedIndividual ;
    rdfs:label "State" .

epa-frs-data:d.Agency.C2000 a epa-frs:Agency,
        owl:NamedIndividual ;
    rdfs:label "Treasury" .

epa-frs-data:d.Agency.C2700 a epa-frs:Agency,
        owl:NamedIndividual ;
    rdfs:label "Federal Communications Commission" .

epa-frs-data:d.Agency.C2800 a epa-frs:Agency,
        owl:NamedIndividual ;
    rdfs:label "Social Security Administration" .

epa-frs-data:d.Agency.C3600 a epa-frs:Agency,
        owl:NamedIndividual ;
    rdfs:label "Veterans Affairs" .

epa-frs-data:d.Agency.C4700 a epa-frs:Agency,
        owl:NamedIndividual ;
    rdfs:label "General Services Administration" .

epa-frs-data:d.Agency.C4900 a epa-frs:Agency,
        owl:NamedIndividual ;
    rdfs:label "National Science Foundation" .

epa-frs-data:d.Agency.C5100 a epa-frs:Agency,
        owl:NamedIndividual ;
    rdfs:label "Federal Depository Insurance Corporation" .

epa-frs-data:d.Agency.C5600 a epa-frs:Agency,
        owl:NamedIndividual ;
    rdfs:label "Central Intelligence Agency" .

epa-frs-data:d.Agency.C6100 a epa-frs:Agency,
        owl:NamedIndividual ;
    rdfs:label "Consumer Product Safety Commission" .

epa-frs-data:d.Agency.C6800 a epa-frs:Agency,
        owl:NamedIndividual ;
    rdfs:label "Environmental Protection Agency" .

epa-frs-data:d.Agency.C6900 a epa-frs:Agency,
        owl:NamedIndividual ;
    rdfs:label "Transportation -- not otherwise classified;" .

epa-frs-data:d.Agency.C6905 a epa-frs:Agency.Transportation,
        owl:NamedIndividual ;
    rdfs:label "Federal Aviation Administration" .

epa-frs-data:d.Agency.C7000 a epa-frs:Agency,
        owl:NamedIndividual ;
    rdfs:label "Homeland Security" .

epa-frs-data:d.Agency.C7010 a epa-frs:Agency.HomelandSecurity,
        owl:NamedIndividual ;
    rdfs:label "Customs and Border Protection" .

epa-frs-data:d.Agency.C7030 a epa-frs:Agency.HomelandSecurity,
        owl:NamedIndividual ;
    rdfs:label "Science and Technology Directorate" .

epa-frs-data:d.Agency.C7040 a epa-frs:Agency.HomelandSecurity,
        owl:NamedIndividual ;
    rdfs:label "Cybersecurity and Infrastructure Security Agency" .

epa-frs-data:d.Agency.C7041 a epa-frs:Agency.HomelandSecurity,
        owl:NamedIndividual ;
    rdfs:label "Federal Emergency Management Agency" .

epa-frs-data:d.Agency.C7050 a epa-frs:Agency.HomelandSecurity,
        owl:NamedIndividual ;
    rdfs:label "Secret Service" .

epa-frs-data:d.Agency.C7060 a epa-frs:Agency.HomelandSecurity,
        owl:NamedIndividual ;
    rdfs:label "Coast Guard" .

epa-frs-data:d.Agency.C7300 a epa-frs:Agency,
        owl:NamedIndividual ;
    rdfs:label "Small Business Administration" .

epa-frs-data:d.Agency.C7500 a epa-frs:Agency,
        owl:NamedIndividual ;
    rdfs:label "Health and Human Services" .

epa-frs-data:d.Agency.C7800 a epa-frs:Agency,
        owl:NamedIndividual ;
    rdfs:label "Farm Credit Administration" .

epa-frs-data:d.Agency.C8000 a epa-frs:Agency,
        owl:NamedIndividual ;
    rdfs:label "National Aeronautics and Space Administration" .

epa-frs-data:d.Agency.C8600 a epa-frs:Agency,
        owl:NamedIndividual ;
    rdfs:label "Housing and Urban Development" .

epa-frs-data:d.Agency.C8800 a epa-frs:Agency,
        owl:NamedIndividual ;
    rdfs:label "National Archives and Records Administration" .

epa-frs-data:d.Agency.C9100 a epa-frs:Agency,
        owl:NamedIndividual ;
    rdfs:label "Education" .

epa-frs-data:d.Agency.C9200 a epa-frs:Agency,
        owl:NamedIndividual ;
    rdfs:label "International Boundary and Water Commission" .

epa-frs-data:d.Agency.C9300 a epa-frs:Agency,
        owl:NamedIndividual ;
    rdfs:label "National Weather Service" .

epa-frs-data:d.Agency.D1032 a epa-frs:Agency.Defense,
        owl:NamedIndividual ;
    rdfs:label "Air Force Reserve" .

epa-frs-data:d.Agency.D1033 a epa-frs:Agency.Defense,
        owl:NamedIndividual ;
    rdfs:label "Air National Guard" .

epa-frs-data:d.Agency.D1034 a epa-frs:Agency.Defense,
        owl:NamedIndividual ;
    rdfs:label "Army Reserves" .

epa-frs-data:d.Agency.D1035 a epa-frs:Agency.Defense,
        owl:NamedIndividual ;
    rdfs:label "Army National Guard" .

epa-frs-data:d.Agency.D1036 a epa-frs:Agency.Defense,
        owl:NamedIndividual ;
    rdfs:label "Defense Intelligence Agency" .

epa-frs-data:d.Agency.D1037 a epa-frs:Agency.Defense,
        owl:NamedIndividual ;
    rdfs:label "Department of Defense Education Activity" .

epa-frs-data:d.Agency.D1038 a epa-frs:Agency.Defense,
        owl:NamedIndividual ;
    rdfs:label "Marine Corps Reserves" .

epa-frs-data:d.Agency.D1039 a epa-frs:Agency.Defense,
        owl:NamedIndividual ;
    rdfs:label "Missile Defense Agency" .

epa-frs-data:d.Agency.D1040 a epa-frs:Agency.Defense,
        owl:NamedIndividual ;
    rdfs:label "National Guard" .

epa-frs-data:d.Agency.D1041 a epa-frs:Agency.Defense,
        owl:NamedIndividual ;
    rdfs:label "Navy Reserves" .

epa-frs-data:d.Agency.D1042 a epa-frs:Agency.Defense,
        owl:NamedIndividual ;
    rdfs:label "United States Military Academy" .

epa-frs-data:d.Agency.D1700 a epa-frs:Agency.Defense,
        owl:NamedIndividual ;
    rdfs:label "Navy" .

epa-frs-data:d.Agency.D1737 a epa-frs:Agency.Defense,
        owl:NamedIndividual ;
    rdfs:label "Marine Corps" .

epa-frs-data:d.Agency.D2100 a epa-frs:Agency.Defense,
        owl:NamedIndividual ;
    rdfs:label "Army" .

epa-frs-data:d.Agency.D5700 a epa-frs:Agency.Defense,
        owl:NamedIndividual ;
    rdfs:label "Air Force" .

epa-frs-data:d.Agency.D8400 a epa-frs:Agency.Defense,
        owl:NamedIndividual ;
    rdfs:label "Armed Forces Retirement Home" .

epa-frs-data:d.Agency.D9600 a epa-frs:Agency.Defense,
        owl:NamedIndividual ;
    rdfs:label "Army Corps of Engineers" .

epa-frs-data:d.Agency.D9700 a epa-frs:Agency,
        owl:NamedIndividual ;
    rdfs:label "Defense" .

epa-frs-data:d.Agency.D9705 a epa-frs:Agency.Defense,
        owl:NamedIndividual ;
    rdfs:label "National Security Agency" .

epa-frs-data:d.Agency.D9715 a epa-frs:Agency.Defense,
        owl:NamedIndividual ;
    rdfs:label "Defense Logistics Agency" .

epa-frs-data:d.Agency.E1044 a epa-frs:Agency.Energy,
        owl:NamedIndividual ;
    rdfs:label "Ames National Laboratory" .

epa-frs-data:d.Agency.E1045 a epa-frs:Agency.Energy,
        owl:NamedIndividual ;
    rdfs:label "Argonne National Laboratory" .

epa-frs-data:d.Agency.E1046 a epa-frs:Agency.Energy,
        owl:NamedIndividual ;
    rdfs:label "Brookhaven National Laboratory" .

epa-frs-data:d.Agency.E1047 a epa-frs:Agency.Energy,
        owl:NamedIndividual ;
    rdfs:label "Energy Information Administration" .

epa-frs-data:d.Agency.E1048 a epa-frs:Agency.Energy,
        owl:NamedIndividual ;
    rdfs:label "Federal  Energy Regulatory Commission" .

epa-frs-data:d.Agency.E1049 a epa-frs:Agency.Energy,
        owl:NamedIndividual ;
    rdfs:label "Fermi National Accelerator Laboratory" .

epa-frs-data:d.Agency.E1050 a epa-frs:Agency.Energy,
        owl:NamedIndividual ;
    rdfs:label "Idaho National Laboratory" .

epa-frs-data:d.Agency.E1051 a epa-frs:Agency.Energy,
        owl:NamedIndividual ;
    rdfs:label "Lawrence Berkeley National Laboratory" .

epa-frs-data:d.Agency.E1052 a epa-frs:Agency.Energy,
        owl:NamedIndividual ;
    rdfs:label "Lawrence Livermore National Laboratory" .

epa-frs-data:d.Agency.E1053 a epa-frs:Agency.Energy,
        owl:NamedIndividual ;
    rdfs:label "Los Alamos National Laboratory" .

epa-frs-data:d.Agency.E1054 a epa-frs:Agency.Energy,
        owl:NamedIndividual ;
    rdfs:label "National Energy Technology Laboratory" .

epa-frs-data:d.Agency.E1055 a epa-frs:Agency.Energy,
        owl:NamedIndividual ;
    rdfs:label "National Renewable Energy Laboratory" .

epa-frs-data:d.Agency.E1056 a epa-frs:Agency.Energy,
        owl:NamedIndividual ;
    rdfs:label "Oak Ridge National Laboratory" .

epa-frs-data:d.Agency.E1057 a epa-frs:Agency.Energy,
        owl:NamedIndividual ;
    rdfs:label "Office of Environmental Management" .

epa-frs-data:d.Agency.E1058 a epa-frs:Agency.Energy,
        owl:NamedIndividual ;
    rdfs:label "Office of Science" .

epa-frs-data:d.Agency.E1059 a epa-frs:Agency.Energy,
        owl:NamedIndividual ;
    rdfs:label "Pacific Northwest National Laboratory" .

epa-frs-data:d.Agency.E1060 a epa-frs:Agency.Energy,
        owl:NamedIndividual ;
    rdfs:label "Princeton Plasma Physics Laboratory" .

epa-frs-data:d.Agency.E1061 a epa-frs:Agency.Energy,
        owl:NamedIndividual ;
    rdfs:label "Sandia National Laboratory" .

epa-frs-data:d.Agency.E1062 a epa-frs:Agency.Energy,
        owl:NamedIndividual ;
    rdfs:label "Savannah River National Laboratory" .

epa-frs-data:d.Agency.E1063 a epa-frs:Agency.Energy,
        owl:NamedIndividual ;
    rdfs:label "SLAC National Accelerator Laboratory" .

epa-frs-data:d.Agency.E1064 a epa-frs:Agency.Energy,
        owl:NamedIndividual ;
    rdfs:label "Thomas Jefferson National Accelerator Laboratory" .

epa-frs-data:d.Agency.E1119 a epa-frs:Agency.Energy,
        owl:NamedIndividual ;
    rdfs:label "Bonneville Power Administration" .

epa-frs-data:d.Agency.E1120 a epa-frs:Agency.Energy,
        owl:NamedIndividual ;
    rdfs:label "Southwestern Power Administration" .

epa-frs-data:d.Agency.E1121 a epa-frs:Agency.Energy,
        owl:NamedIndividual ;
    rdfs:label "Western Area Power Administration" .

epa-frs-data:d.Agency.E6400 a epa-frs:Agency.Energy,
        owl:NamedIndividual ;
    rdfs:label "Tennessee Valley Authority" .

epa-frs-data:d.Agency.E8900 a epa-frs:Agency,
        owl:NamedIndividual ;
    rdfs:label "Energy" .

epa-frs-data:d.Agency.E8902 a epa-frs:Agency.Energy,
        owl:NamedIndividual ;
    rdfs:label "National Nuclear Security Administration" .

epa-frs-data:d.Agency.E8903 a epa-frs:Agency.Energy,
        owl:NamedIndividual ;
    rdfs:label "Southeastern Power Administration" .

epa-frs-data:d.Agency.X0100 a epa-frs:Agency.Congress,
        owl:NamedIndividual ;
    rdfs:label "Architect of the Capitol" .

epa-frs-data:d.Agency.X0111 a epa-frs:Agency,
        owl:NamedIndividual ;
    rdfs:label "Library of Congress" .

epa-frs-data:d.Agency.X1000 a epa-frs:Agency,
        owl:NamedIndividual ;
    rdfs:label "Judicial" .

epa-frs-data:d.Agency.X1011 a epa-frs:Agency.Judicial,
        owl:NamedIndividual ;
    rdfs:label "Administrative Office of the U.S. Courts" .

epa-frs-data:d.Agency.X1012 a epa-frs:Agency.Congress,
        owl:NamedIndividual ;
    rdfs:label "Stennis Center for Public Service" .

epa-frs-data:d.Agency.X1013 a epa-frs:Agency.Congress,
        owl:NamedIndividual ;
    rdfs:label "Capital Police" .

epa-frs-data:d.Agency.X1014 a epa-frs:Agency,
        owl:NamedIndividual ;
    rdfs:label "Congress" .

epa-frs-data:d.Agency.X1015 a epa-frs:Agency,
        owl:NamedIndividual ;
    rdfs:label "Advisory Council on History Preservation" .

epa-frs-data:d.Agency.X1025 a epa-frs:Agency,
        owl:NamedIndividual ;
    rdfs:label "Chemical Safety Board" .

epa-frs-data:d.Agency.X1042 a epa-frs:Agency,
        owl:NamedIndividual ;
    rdfs:label "Delaware River Basin Commission" .

epa-frs-data:d.Agency.X1079 a epa-frs:Agency,
        owl:NamedIndividual ;
    rdfs:label "John F. Kennedy Center for the Performing Arts" .

epa-frs-data:d.Agency.X1095 a epa-frs:Agency,
        owl:NamedIndividual ;
    rdfs:label "Susquehanna River Basin Commission" .

epa-frs-data:d.Agency.X1112 a epa-frs:Agency,
        owl:NamedIndividual ;
    rdfs:label "Artic Research Commission" .

epa-frs-data:d.Agency.X3300 a epa-frs:Agency,
        owl:NamedIndividual ;
    rdfs:label "Smithsonian Institution" .

epa-frs-data:d.Agency.X9999 a epa-frs:Agency,
        owl:NamedIndividual ;
    rdfs:label "Undetermined or Unknown Agency Affiliation" .

epa-frs:Agency.Judicial a owl:Class ;
    rdfs:label "Judicial" ;
    rdfs:subClassOf epa-frs:Agency .

epa-frs:HazardousWasteProgram a owl:Class ;
    rdfs:label "HAZARDOUS WASTE PROGRAM"^^xsd:string ;
    dcterms:description "AN ENVIRONMENTAL PROGRAM THAT REGULATES HAZARDOUS WASTE, INCLUDING THE GENERATION, TRANSPORTATION, TREATMENT, STORAGE, AND DISPOSAL OF HAZARDOUS WASTE, AS REQUIRED BY THE RESOURCE CONSERVATION AND RECOVERY ACT (RCRA)."^^xsd:string,
        "ENVIRONMENTAL PROGRAMS THAT REGULATE HAZARDOUS WASTE, INCLUDING THE GENERATION, TRANSPORTATION, TREATMENT, STORAGE, AND DISPOSAL OF HAZARDOUS WASTE, AS REQUIRED BY THE RESOURCE CONSERVATION AND RECOVERY ACT (RCRA)."^^xsd:string ;
    rdfs:subClassOf epa-frs:HazardousWastePrograms .

epa-frs:HealthAndSafetyPrograms a owl:Class ;
    rdfs:label "HEALTH AND SAFETY PROGRAMS"^^xsd:string ;
    dcterms:description "PROGRAMS DESIGNED TO REDUCE HAZARDS AND PREVENT INJURIES, ILLNESSES AND DEATHS IN THE WORKPLACE."^^xsd:string ;
    rdfs:subClassOf epa-frs:EnvironmentalInterest .

epa-frs:ACES-Facility a owl:Class ;
    rdfs:label "AGENCY COMPLIANCE AND ENFORCEMENT SYSTEMS" ;
    dcterms:description "The Agency Compliance and Enforcement Systems (ACES) application supports the compliance and enforcement activities that exist primarily within the Illinois Bureaus of Air, Water, and Land, the Division of Legal Counsel, and the Office of Chemical Safety. The intent of the system is to track compliance and enforcement processes and to share the information throughout the agency, the public and with other entities." ;
    rdfs:subClassOf epa-frs:FRS-Facility .

epa-frs:ACRES-Facility a owl:Class ;
    rdfs:label "ASSESSMENT, CLEANUP AND REDEVELOPMENT EXCHANGE SYSTEM" ;
    dcterms:description "The Assessment, Cleanup and Redevelopment Exchange System (ACRES) stores information reported by EPA Brownfields grant recipients on Brownfields properties assessed or cleaned up with grant funding, as well as information on Targeted Brownfields Assessments (TBA) performed by EPA Regions." ;
    rdfs:subClassOf epa-frs:FRS-Facility .

epa-frs:AIR-Facility a owl:Class ;
    rdfs:label "ICIS-AIR (AIR)" ;
    dcterms:description "ICIS-Air (AIR) – AIR is the modernization of the Air Facility System (AFS) into the Integrated Compliance Information System (ICIS).  AIR contains enforcement, compliance, and permit data for stationary sources of air pollution regulated by the EPA, State, and Local air pollution agencies." ;
    rdfs:subClassOf epa-frs:FRS-Facility .

epa-frs:AIRS-AFS-Facility a owl:Class ;
    rdfs:label "AIR FACILITY SYSTEM" ;
    dcterms:description "The Air Facility System (AFS) contains compliance and permit data for stationary sources of air pollution regulated by the EPA, state, and local air pollution agencies." ;
    rdfs:subClassOf epa-frs:FRS-Facility .

epa-frs:AIRS-AQS-Facility a owl:Class ;
    rdfs:label "AIR QUALITY SYSTEM" ;
    dcterms:description "The Air Quality System (AQS) contains ambient air pollution data collected by EPA, State, Local, and Tribal air pollution control agencies from thousands of monitoring stations." ;
    rdfs:subClassOf epa-frs:FRS-Facility .

epa-frs:AZURITE-Facility a owl:Class ;
    rdfs:label "ARIZONA UNIFIED REPOSITORY FOR INFORMATIONAL TRACKING OF THE ENVIRONMENT" ;
    dcterms:description "The Arizona Unified Repository for Informational Tracking of the Environment (AZURITE) is a database used by the Arizona Department of Environmental Quality (ADEQ) for environmental enforcement and compliance reporting to the Permit and Compliance System (PCS) and to the Air Facility System Universal Interface (AFS-UI)." ;
    rdfs:subClassOf epa-frs:FRS-Facility .

epa-frs:Agency.HousingandUrbanDevelopment a owl:Class ;
    rdfs:label "Housing and Urban Development" ;
    rdfs:subClassOf epa-frs:Agency .

epa-frs:BIA-INDIAN-SCHOOL-Facility a owl:Class ;
    rdfs:label "BUREAU OF INDIAN AFFAIRS INDIAN SCHOOL" ;
    dcterms:description "The Bureau of Indian Affairs (BIA) school data on Indian land. The BIA is responsible for the administration and management of 55.7 million acres of land held in trust by the United States for American Indians, Indian Tribes, and Alaska natives and provides education services to approximately 48,000 Indian students." ;
    rdfs:subClassOf epa-frs:FRS-Facility .

epa-frs:BR-Facility a owl:Class ;
    rdfs:label "BIENNIAL REPORTERS" ;
    dcterms:description "All generators and treatment, storage, and disposal (TSD) facilities who handle hazardous waste are required to report to the EPA Administrator at least once every two years. The data collected is used to create the National Biennial Resource Conservation and Recovery Act (RCRA) Hazardous Waste Report. This data is processed within the RCRA Information (RCRAInfo) database" ;
    rdfs:subClassOf epa-frs:FRS-Facility .

epa-frs:BRAC-Facility a owl:Class ;
    rdfs:label "BASE REALIGNMENT AND CLOSURE" ;
    dcterms:description "Base Realignment and Closure (BRAC) is a process used to close excess military installations and realign the total asset inventory in order to save money on operations and maintenance." ;
    rdfs:subClassOf epa-frs:FRS-Facility .

epa-frs:CA-CERS-Facility a owl:Class ;
    rdfs:label "CA-CALIFORNIA ENVIRONMENTAL REPORTING SYSTEM" ;
    dcterms:description "The California Environmental Reporting System (CERS) is a statewide web-based user and information exchange system to support over 140,000 regulated businesses and over 130 local agencies in electronically collecting and reporting significant hazardous materials, hazardous waste and compliance and enforcement data as mandated by California law. Under oversight by Cal/EPA, certified local governing agencies (Unified Program Agencies - UPAs) consolidate, coordinate and provide consistent regulatory activities for six state and federal environmental programs." ;
    rdfs:subClassOf epa-frs:FRS-Facility .

epa-frs:CA-ENVIROVIEW-Facility a owl:Class ;
    rdfs:label "CALIFORNIA - ENVIROVIEW" ;
    dcterms:description "The California Environmental Protection Agency (CalEPA) has recently implemented a new data warehouse system (“nSite”). This data warehouse combines and merges facility and site information from five different systems managed within CalEPA.  The five systems are: California Environmental Reporting System (CERS),	EnviroStor, GeoTracker, California Integrated Water Quality System (CIWQS), and	Toxic Release Inventory (TRI)." ;
    rdfs:subClassOf epa-frs:FRS-Facility .

epa-frs:CAMDBS-Facility a owl:Class ;
    rdfs:label "CLEAN AIR MARKETS DIVISION (CAMD) BUSINESS SYSTEMS" ;
    dcterms:description "The Clean Air Markets Division Business System (CAMDBS) supports the implementation of market-based air pollution control programs administered by the EPA Clean Air Markets Division, within the Office of Air and Radiation. Programs include the Acid Rain Program and regional programs designed to reduce the transport of ozone." ;
    rdfs:subClassOf epa-frs:FRS-Facility .

epa-frs:CASWIS-Facility a owl:Class ;
    rdfs:label "CALIFORNIA SOLID WASTE INFORMATION SYSTEM" ;
    dcterms:description "California Solid Waste Integrating System (CaSWIS) is California's solid waste facility list that contains information on solid waste facilities, operations, and open and closed disposal sites throughout the state." ;
    rdfs:subClassOf epa-frs:FRS-Facility .

epa-frs:CDAFLP-Facility a owl:Class ;
    rdfs:label "COEUR D'ALENE FACILITY LOCATION PROGRAM" ;
    dcterms:description "The Coeur d'Alene Tribe was awarded a grant to collect locational information for facilities found within current reservation boundaries and for facilities outside reservation boundaries within the Coeur d'Alene aboriginal territory. Using field maps as a reference guide, each site was visited to acquire accurate lat/long coordinates at the entrance of the facility, using a high precision hand-held GPS unit (sub meter accuracy)." ;
    rdfs:subClassOf epa-frs:FRS-Facility .

epa-frs:CEDRI-Facility a owl:Class ;
    rdfs:label "COMPLIANCE AND EMISSIONS DATA REPORTING INTERFACE" ;
    dcterms:description "CEDRI is a web application used by EPA programs and various stakeholders to manage environmental data transmitted to EPA in order to meet EPA's reporting requirements." ;
    rdfs:subClassOf epa-frs:FRS-Facility .

epa-frs:CEDS-Facility a owl:Class ;
    rdfs:label "VIRGINIA - COMPREHENSIVE ENVIRONMENTAL DATA SYSTEM" ;
    dcterms:description "The Comprehensive Environmental Data System (CEDS) is the Virginia Department of Environmental Quality's (DEQ) electronic data system for maintaining data on sources of pollutants in all media." ;
    rdfs:subClassOf epa-frs:FRS-Facility .

epa-frs:CERCLIS-Facility a owl:Class ;
    rdfs:label "COMPREHENSIVE ENVIRONMENTAL RESPONSE, COMPENSATION, AND LIABILITY INFORMATION SYSTEM" ;
    dcterms:description "CERLIS was EPA's inventory of abandoned, inactive, or uncontrolled hazardouse waste sites regulated under the Comprehsensive Environmental Response, Compensation, and Liability Act (CERCLA) through October, 2013. It recorded infromation about all aspects of hazardous waste sites from initial discovery to listing on the National Priorities list (NPL). CERCLIS has been replaced as a source for Superfund data by the Superfund Enterprise Management System (SEMS)." ;
    rdfs:subClassOf epa-frs:FRS-Facility .

epa-frs:CIM-Facility a owl:Class ;
    rdfs:label "UTAH - COMMON IDENTIFIER MECHANISM" ;
    dcterms:description "The Common Identifier Mechanism (CIM) is the Utah Department of Environmental Quality's (UDEQ) data system for compliance and permitting data." ;
    rdfs:subClassOf epa-frs:FRS-Facility .

epa-frs:CNFRS-Facility a owl:Class ;
    rdfs:label "CHEROKEE NATION FACILITY REGISTRY SYSTEM" ;
    dcterms:description "The Cherokee Nation Facility Registry System (CNFRS) is a data flow system that validates existing FRS data and exchanges data about tribal open dump sites." ;
    rdfs:subClassOf epa-frs:FRS-Facility .

epa-frs:CWNS-Facility a owl:Class ;
    rdfs:label "CLEAN WATERSHEDS NEEDS SURVEY" ;
    dcterms:description "THE CLEAN WATERSHEDS NEEDS SURVEY (CWNS) IS A COMPREHENSIVE ASSESSMENT OF THE CAPITAL NEEDS TO MEET THE WATER QUALITY GOALS SET IN THE CLEAN WATER ACT. EVERY FOUR YEARS, THE STATES AND EPA COLLECT INFORMATION ABOUT PUBLICLY OWNED WASTEWATER COLLECTION AND TREATMENT FACILITIES, STORMWATER AND COMBINED SEWER OVERFLOWS CONTROL FACILITIES, NONPOINT SOURCE (NPS) POLLUTION CONTROL PROJECTS, DECENTRALIZED WASTEWATER MANAGEMENT, AND ESTUARY MANAGEMENT PROJECTS. INFORMATION COLLECTED INCLUDES ESTIMATED NEEDS, INCLUDING COSTS AND TECHNICAL INFORMATION, TO ADDRESS A WATER QUALITY OR WATER-RELATED PUBLIC HEALTH PROBLEM, LOCATION AND CONTACT INFORMATION, POPULATIONS SERVED, FLOW, EFFLUENT, AND UNIT PROCESS INFORMATION, AND NPS BEST MANAGEMENT PRACTICES. THIS INFORMATION IS USED BY EPA TO DOCUMENT NATIONAL NEEDS IN A REPORT TO CONGRESS, WHICH ASSISTS IN BUDGETING EFFORTS. THE DATA ARE ALSO USED TO HELP MEASURE ENVIRONMENTAL PROGRESS, CONTRIBUTE TO ACADEMIC RESEARCH, PROVIDE INFORMATION TO THE PUBLIC, AND HELP LOCAL AND STATE GOVERNMENTS IMPLEMENT WATER QUALITY PROGRAMS." ;
    rdfs:subClassOf epa-frs:FRS-Facility .

epa-frs:CoastalAndOceanPrograms a owl:Class ;
    rdfs:label "COASTAL AND OCEAN PROGRAMS"^^xsd:string ;
    dcterms:description "ENVIRONMENTAL PROGRAMS THAT IMPROVE THE QUALITY OF COASTAL AND MARINE ECOSYSTEMS AND PROTECT BEACHES, COAST, AND OCEAN RESOURCES FROM POLLUTION."^^xsd:string ;
    rdfs:subClassOf epa-frs:EnvironmentalInterest .

epa-frs:DEN-Facility a owl:Class ;
    rdfs:label "DELAWARE ENVIRONMENTAL NAVIGATOR" ;
    dcterms:description "The Delaware Environmental Navigator (DEN) contains almost all of environmental data other than ambient air and water monitoring results.  DEN contains facility, program interest, location, owner, permittee, project officer, permit, inspection, violation and enforcement data." ;
    rdfs:subClassOf epa-frs:FRS-Facility .

epa-frs:DTSC-ENVIROSTOR-Facility a owl:Class ;
    rdfs:label "CALIFORNIA - DEPARTMENT OF TOXIC SUBSTANCES CONTROL - ENVIROSTOR SYSTEM" ;
    dcterms:description "California's Department of Toxic Substances Control's (DTSC's)-EnviroStor database is an online search and Geographic Information System (GIS) tool for identifying sites that have known contamination or sites for which there may be reasons to investigate further. The EnviroStor database includes the following site types: Federal Superfund sites (National Priorities List (NPL)); State Response, including Military Facilities and State Superfund; Voluntary Cleanup; and School sites." ;
    rdfs:subClassOf epa-frs:FRS-Facility .

epa-frs:E-GGRT-Facility a owl:Class ;
    rdfs:label "ELECTRONIC GREENHOUSE GAS REPORTING TOOL (E-GGRT)" ;
    dcterms:description "THE ELECTRONIC GREENHOUSE GAS REPORTING TOOL (E-GGRT) IS ACCESSIBLE THROUGH AN EPA WEB PAGE AND USED TO SUBMIT ANNUAL REPORTS IN SUPPORT OF THE EPA RULE FOR MANDATORY REPORTING OF GREENHOUSE GASES (GHG) FROM LARGE GHG EMISSIONS SOURCES. IMPLEMENTATION OF 40 CFR PART 98 IS REFERRED TO AS THE GREENHOUSE GAS REPORTING PROGRAM (GHGRP). THIS COMPREHENSIVE, NATIONWIDE EMISSIONS DATA WILL PROVIDE A BETTER UNDERSTANDING OF THE SOURCES OF GHGS AND WILL GUIDE DEVELOPMENT OF THE POLICIES AND PROGRAMS TO REDUCE EMISSIONS. THE PUBLICALLY AVAILABLE DATA WILL ALLOW REPORTERS TO TRACK THEIR OWN EMISSIONS, COMPARE THEM TO SIMILAR FACILITIES, AND AID IN IDENTIFYING COST EFFECTIVE OPPORTUNITIES TO REDUCE EMISSIONS IN THE FUTURE." ;
    rdfs:subClassOf epa-frs:FRS-Facility .

epa-frs:ECRM-Facility a owl:Class ;
    rdfs:label "ENFORCEMENT CRIMINAL RECORDS MANAGEMENT" ;
    dcterms:description "The Enforcement Criminal Records Management System, now called the Criminal Case Reporting System (CCRS), is the Criminal Investigation Division's \"official record\" of all criminal investigation activities. The system maintains and tracks case-specific program and investigative information on over 8,200 active and archived criminal cases. CCRS is an EPA-only system and data entry is performed directly by CID employees. The Public is allowed to obtain only select defendant data fields for closed, convicted cases via the Freedom of Information Act." ;
    rdfs:subClassOf epa-frs:FRS-Facility .

epa-frs:EGRID-Facility a owl:Class ;
    rdfs:label "EMISSIONS & GENERATION RESOURCE INTEGRATED DATABASE" ;
    dcterms:description "The Emissions & Generation Resource Integrated Database (EGRID) contains data on emissions and resources mix for virtually every power plant and company that generates electricity in the United States." ;
    rdfs:subClassOf epa-frs:FRS-Facility .

epa-frs:EIA-860-Facility a owl:Class ;
    rdfs:label "ENERGY INFORMATION ADMINISTRATION-860 (EIA-860) DATABASE" ;
    dcterms:description "THE ENERGY INFORMATION ADMINISTRATION (EIA) IS AN INDEPENDENT AGENCY WITHIN THE U.S. DEPARTMENT OF ENERGY THAT DEVELOPS SURVEYS, COLLECTS ENERGY DATA, AND DOES ANALYTICAL AND MODELING ANALYSES OF ENERGY ISSUES. THE EIA-860 DATABASE SUPPORTS THE ANNUAL ELECTRIC GENERATOR REPORT AND CONTAINS ELECTRIC UTILITY AND NON-UTILITY (INCLUDING INDEPENDENT POWER PRODUCERS, COMBINED HEAT AND POWER PRODUCERS, AND OTHER INDUSTRIALS) GENERATOR-SPECIFIC PLANT DATA, INCLUDING COUNTY AND STATE LOCATION AND OWNERSHIP INFORMATION" ;
    rdfs:subClassOf epa-frs:FRS-Facility .

epa-frs:EIS-Facility a owl:Class ;
    rdfs:label "EMISSION INVENTORY SYSTEM (EIS)" ;
    dcterms:description "THE EMISSION INVENTORY SYSTEM (EIS) MAINTAINS AN INVENTORY OF LARGE STATIONARY SOURCES AND VOLUNTARILY-REPORTED SMALLER SOURCES OF AIR POINT POLLUTANT EMITTERS. IT CONTAINS INFORMATION ABOUT FACILITY SITES AND THEIR PHYSICAL LOCATION, EMISSIONS UNITS, EMISSIONS PROCESSES, RELEASE POINTS, CONTROL APPROACHES, AND REGULATIONS. FACILITY INVENTORY DATA ARE KEPT SEPARATE FROM THE EMISSIONS DATA AND HAVE STABLE IDENTIFIERS TO IMPROVE CONTINUITY FROM YEAR TO YEAR AND TO HELP IDENTIFY DUPLICATE OR MISSING FACILITIES" ;
    rdfs:subClassOf epa-frs:FRS-Facility .

epa-frs:EPS-Facility a owl:Class ;
    rdfs:label "ELECTRONIC PERMIT SYSTEM" ;
    dcterms:description "ALLOWS PERMITTING AUTHORITIES TO SUBMIT NEW SOURCE REVIEW (NSR) AND TITLE V PERMIT ACTIONS TO EPA FOR REVIEW." ;
    rdfs:subClassOf epa-frs:FRS-Facility .

epa-frs:EcologyOperations a owl:Class ;
    rdfs:label "ECOLOGY OPERATIONS"^^xsd:string ;
    dcterms:description "PROGRAMS THAT CONCENTRATE ON ECOLOGICAL SYSTEMS SUCH AS FOREST AND TREE EXPERTISE"^^xsd:string ;
    rdfs:subClassOf epa-frs:EnvironmentalInterest .

epa-frs:FARR-Facility a owl:Class ;
    rdfs:label "FEDERAL AIR RULES FOR RESERVATIONS (FARR) REGISTRATION PROGRAM" ;
    dcterms:description "THE FEDERAL AIR RULES FOR RESERVATIONS (FARR) REQUIRES PERSONS WHO OWN OR OPERATE CERTAIN SOURCES OF AIR POLLUTION ON INDIAN RESERVATIONS IN IDAHO, OREGON AND WASHINGTON TO REGISTER THOSE SOURCES WITH EPA AND TO REPORT AIR POLLUTANT EMISSIONS ANNUALLY." ;
    rdfs:subClassOf epa-frs:FRS-Facility .

epa-frs:FDM-Facility a owl:Class ;
    rdfs:label "FLORIDA - FIESTA DATA MAINTENANCE" ;
    dcterms:description "The Florida Integrated Environmental System Today (FIESTA) Data Maintenance (FDM) System maintains entity, environmental interest, and affiliation data." ;
    rdfs:subClassOf epa-frs:FRS-Facility .

epa-frs:FFDOCKET-Facility a owl:Class ;
    rdfs:label "FEDERAL FACILITY HAZARDOUS WASTE COMPLIANCE DOCKET" ;
    dcterms:description "SECTION 120(C) OF COMPREHENSIVE ENVIRONMENTAL RESPONSE, COMPENSATION AND LIABILITY ACT (CERCLA) REQUIRES EPA TO ESTABLISH A LISTING, KNOWN AS THE FEDERAL FACILITY HAZARDOUS WASTE COMPLIANCE DOCKET (DOCKET), OF FEDERAL FACILITIES WHICH ARE MANAGING OR HAVE MANAGED HAZARDOUS WASTE; OR HAVE HAD A RELEASE OF HAZARDOUS WASTE. THUS, THE DOCKET IDENTIFIES ALL FEDERAL FACILITIES THAT MUST BE EVALUATED TO DETERMINE WHETHER THEY POSE A RISK TO HUMAN HEALTH AND THE ENVIRONMENT." ;
    rdfs:subClassOf epa-frs:FRS-Facility .

epa-frs:FFEP-Facility a owl:Class ;
    rdfs:label "FEDERAL FACILITIES RECOVERY AND REUSE OFFICE" ;
    dcterms:description "ALLOWS FEDERAL AGENCIES TO SUBMIT FEDERAL SUPERFUND SITE CLEAN-UP DOCUMENTATION TO EPA FOR REVIEW AND APPROVAL." ;
    rdfs:subClassOf epa-frs:FRS-Facility .

epa-frs:FIS-Facility a owl:Class ;
    rdfs:label "NEW YORK - FACILITY INFORMATION SYSTEM" ;
    dcterms:description "The New York Department of Environmental Conservation Facility Information System (FIS) database houses all information about facilities that are regulated or of environmental interest to the state of New York." ;
    rdfs:subClassOf epa-frs:FRS-Facility .

epa-frs:GEIMS-Facility a owl:Class ;
    rdfs:label "GEORGIA - GEOGRAPHIC ENVIRONMENTAL INFORMATION MANAGEMENT SYSTEM" ;
    dcterms:description "Georgia's Geographic Environmental Information Management System (GEIMS) provides the EPA and the public a single point of access to core data for all facilities and sites regulated or monitored by the EPA and a single system for the reporting of all environmental data." ;
    rdfs:subClassOf epa-frs:FRS-Facility .

epa-frs:HI-EHW-Facility a owl:Class ;
    rdfs:label "HAWAII ENVIRONMENTAL HEALTH WAREHOUSE" ;
    dcterms:description "The Environmental Health Warehouse (EHW) is primarily Hawaii Department of Health Environmental Health Administration's (HDOH-EHA) environmental interest data.  The web-based application allows EHA to inquire about sites in Hawaii that are regulated by the administration due to activities that affect the environment, regardless of the regulation or program that directly monitors those activities.  The system allows users a consolidated view of sites and their environmental interests without disrupting the underlying source systems or the staff involved as they process their day-to-day workload.  The EHW offers geo-spatial and tabular inquiry, mapping, reconciliation/data consolidation and utilizes GIS services to derive additional geo-data for environmental interests." ;
    rdfs:subClassOf epa-frs:FRS-Facility .

epa-frs:HWTS-DATAMART-Facility a owl:Class ;
    rdfs:label "HAZARDOUS WASTE TRACKING SYSTEM - DATAMART" ;
    dcterms:description "California's Hazardous Waste Tracking System Data Mart (HWTS-DATAMART) provides information on hazardous waste shipments for generators, transporters, and treatment, storage, and disposal facilities." ;
    rdfs:subClassOf epa-frs:FRS-Facility .

epa-frs:ICIS-Facility a owl:Class ;
    rdfs:label "INTEGRATED COMPLIANCE INFORMATION SYSTEM" ;
    dcterms:description "The Integrated Compliance Information System (ICIS) provides a database that, when complete, will contain integrated enforcement and compliance information across most of EPA's programs. The vision for ICIS is to replace EPA's independent databases that contain enforcement data with a single repository for that information. Currently, ICIS contains all Federal Administrative and Judicial enforcement actions and a subset of the Permit Compliance System (PCS), which supports the National Pollutant Discharge Elimination System (NPDES). This information is maintained in ICIS by EPA in the Regional offices and it at Headquarters. A future release of ICIS will completely replace PCS and will integrate that information with Federal actions already in the system. ICIS also has the capability to track other activities that support compliance and enforcement programs, including incident tracking, compliance assistance, and compliance monitoring." ;
    rdfs:subClassOf epa-frs:FRS-Facility .

epa-frs:IDDEQ-Facility a owl:Class ;
    rdfs:label "IDAHO DEPARTMENT OF ENVIRONMENTAL QUALITY" ;
    dcterms:description "The Idaho Department of Environmental Quality (DEQ) provides a means to query and display data maintained by the Department of Environmental Quality. The system contains key information for each facility/site that is currently, or has been, of interest to the departments environmental programs." ;
    rdfs:subClassOf epa-frs:FRS-Facility .

epa-frs:IDNR_EFD-Facility a owl:Class ;
    rdfs:label "IOWA DEPARTMENT OF NATURAL RESOURCES - ENVIRONMENTAL FACILITIES DATABASE" ;
    dcterms:description "The IDNR_EFD system is a data warehouse which integrates environmental information based on facilities in Iowa." ;
    rdfs:subClassOf epa-frs:FRS-Facility .

epa-frs:IN-FRS-Facility a owl:Class ;
    rdfs:label "INDIANA - FACILITY REGISTRY SYSTEM" ;
    dcterms:description "The Indiana Department of Environmental Management (IDEM) implemented the Indiana Facility Registry System (I-FRS), which provides an interface and processes to link facility data monitored by multiple state and EPA program systems. In addition, I-FRS enables IDEM to reconcile environmental data and exchange it with EPA FRS using the electronic data exchange over the network node." ;
    rdfs:subClassOf epa-frs:FRS-Facility .

epa-frs:IN-TEMPO-Facility a owl:Class ;
    rdfs:label "INDIANA-TOOLS FOR ENVIRONMENTAL MANAGEMENT AND PROTECTION ORGANIZATIONS" ;
    dcterms:description "Indiana's Tools For Environmental Management and Protection Organizations (IN-TEMPO) is Indiana's integrated environmental management system." ;
    rdfs:subClassOf epa-frs:FRS-Facility .

epa-frs:ISD-Facility a owl:Class ;
    rdfs:label "WYOMING - INDUSTRIAL SITING DIVISION" ;
    dcterms:description "The Industrial Siting Division (ISD) administers the Wyoming Industrial Information and Siting Act, which requires permits for all projects with construction costs of $168 million or more and for certain business types regardless of cost, including waste incineration or disposal facilities capable of receiving greater than 500 short tons per day of household refuse or mixed household and industrial refuse, commercial facilities which incinerate or dispose of regulated quantities of hazardous wastes which are subject to hazardous waste shipping manifest requirements under subtitle C of the Resource Conservation and Recovery Act, and commercial radioactive waste management facilities." ;
    rdfs:subClassOf epa-frs:FRS-Facility .

epa-frs:KS-FP-Facility a owl:Class ;
    rdfs:label "KANSAS - FACILITY PROFILE" ;
    dcterms:description "The Kansas Facility Profiler (KS-FP) is a geographically-based data warehouse that presents information about facilities and locations of interest to the Kansas Department of Health and Environment (KDHE). It has in excess of twenty environmental interests which contain information on closed facilities, completed cleanups, and past operations, as well as data on current operations and activities." ;
    rdfs:subClassOf epa-frs:FRS-Facility .

epa-frs:KY-TEMPO-Facility a owl:Class ;
    rdfs:label "KENTUCKY - TOOLS FOR ENVIRONMENTAL MANAGEMENT AND PROTECTION ORGANIZATIONS" ;
    dcterms:description "KENTUCKY- Tools for Environmental Management and Protection Organizations (KY-TEMPO) is Kentucky's central repository for facility data and includes permits, surveillance, enforcement, and remediation information." ;
    rdfs:subClassOf epa-frs:FRS-Facility .

epa-frs:LA-TEMPO-Facility a owl:Class ;
    rdfs:label "LOUISIANA - TOOLS FOR ENVIRONMENTAL MANAGEMENT AND PROTECTION ORGANIZATIONS" ;
    dcterms:description "The Louisiana - Tools For Environmental Management And Protection Organizations (LA-TEMPO) is Louisiana's central repository for all facility data and includes permits, surveillance, enforcement, and remediation information." ;
    rdfs:subClassOf epa-frs:FRS-Facility .

epa-frs:LMOP-Facility a owl:Class ;
    rdfs:label "LANDFILL METHANE OUTREACH PROGRAM" ;
    dcterms:description "EPA'S LANDFILL METHANE OUTREACH PROGRAM (LMOP) IS A VOLUNTARY ASSISTANCE PROGRAM THAT HELPS TO REDUCE METHANE EMISSIONS FROM LANDFILLS BY ENCOURAGING THE RECOVERY AND USE OF LANDFILL GAS (LFG) AS AN ENERGY RESOURCE. LMOP FORMS PARTNERSHIPS WITH COMMUNITIES, LANDFILL OWNERS, UTILITIES, POWER MARKETERS, STATES, PROJECT DEVELOPERS, TRIBES, AND NONPROFIT ORGANIZATIONS TO OVERCOME BARRIERS TO PROJECT DEVELOPMENT BY HELPING THEM ASSESS PROJECT FEASIBILITY, FIND FINANCING, AND MARKET THE BENEFITS OF PROJECT DEVELOPMENT TO THE COMMUNITY." ;
    rdfs:subClassOf epa-frs:FRS-Facility .

epa-frs:LUST-ARRA-Facility a owl:Class ;
    rdfs:label "LEAKING UNDERGROUND STORAGE TANK (LUST) ¿ AMERICAN RECOVERY AND REINVESTMENT ACT (ARRA)" ;
    dcterms:description "THE LEAKING UNDERGROUND STORAGE TANK (LUST) ¿ AMERICAN RECOVERY AND REINVESTMENT ACT (ARRA) SYSTEM COLLECTS DATA ON LUST RELEASES THAT ARE TRACKED BY ARRA PERFORMANCE MEASURES OR FOR WHICH ARRA FUNDS ARE BEING SPENT. DATA IS COLLECTED FOR EACH RELEASE, INCLUDING IDENTIFICATION, PERFORMANCE MEASURES, REFERENCE INFORMATION, AND LOCATION INFORMATION." ;
    rdfs:subClassOf epa-frs:FRS-Facility .

epa-frs:MA-EPICS-Facility a owl:Class ;
    rdfs:label "MASSACHUSETTS - ENVIRONMENTAL PROTECTION INTEGRATED COMPUTER SYSTEM" ;
    dcterms:description "The Massachusetts - Environmental Protection Integrated Computer System (MA-EPICS) is the central repository for all environmental protection data for the State of Massachusetts." ;
    rdfs:subClassOf epa-frs:FRS-Facility .

epa-frs:MD-EPSC-Facility a owl:Class ;
    rdfs:label "MARYLAND - ENVIRONMENTAL PERMIT SERVICE CENTER" ;
    dcterms:description "The Maryland Department of the Environment (MDE) Environmental Permits Service Center (MD-EPSC) promotes multi-media pollution prevention and provides permit assistance to business and industries." ;
    rdfs:subClassOf epa-frs:FRS-Facility .

epa-frs:MD-PEMIS-Facility a owl:Class ;
    rdfs:label "MARYLAND - PERMANENT (AIR) EMISSION" ;
    dcterms:description "The Maryland Permanent Emission (MD-PEMIS) database houses data related to air emissions." ;
    rdfs:subClassOf epa-frs:FRS-Facility .

epa-frs:MD-RCRA-Facility a owl:Class ;
    rdfs:label "MARYLAND-RESOURCE CONVERSATION AND RECOVERY ACT DATABASE" ;
    dcterms:description "Maryland's Resource Conservation and Recovery Act (RCRA) database houses data related to hazardous waste." ;
    rdfs:subClassOf epa-frs:FRS-Facility .

epa-frs:MD-TEMPO-Facility a owl:Class ;
    rdfs:label "MARYLAND - TOOLS FOR ENVIRONMENTAL MANAGEMENT AND PROTECTION ORGANIZATIONS (TEMPO)" ;
    dcterms:description "MD-TEMPO is Maryland's central repository for all facility data and includes permits, compliance, enforcement activities information needed to ensure the quality of Maryland's air, water, and land resources." ;
    rdfs:subClassOf epa-frs:FRS-Facility .

epa-frs:ME-EFIS-Facility a owl:Class ;
    rdfs:label "MAINE - ENVIRONMENTAL FACILITY INFORMATION SYSTEM" ;
    dcterms:description "The Maine Department of Environmental Protection (DEP) Environmental Facility Information System (ME-EFIS) integrates information on environmental facilities, permits, violations, enforcement actions, and compliance activities needed to support regulatory requirements and target environmental quality improvements for the water, air, solid waste, and hazardous waste program areas." ;
    rdfs:subClassOf epa-frs:FRS-Facility .

epa-frs:MERI-FIS-Facility a owl:Class ;
    rdfs:label "MEADOWLANDS ENVIRONMENTAL RESEARCH INSTITUTE – FACILITY INFORMATION SYSTEM" ;
    dcterms:description "MERI-FIS is the Hackensack Meadowlands District of NJ's central repository for facility registration data and includes Right To Know hazardous substances data stored in the registered facilities." ;
    rdfs:subClassOf epa-frs:FRS-Facility .

epa-frs:MN-TEMPO-Facility a owl:Class ;
    rdfs:label "MINNESOTA - PERMITTING, COMPLIANCE, AND ENFORCEMENT INFORMATION MANAGEMENT SYSTEM" ;
    dcterms:description "MN-TEMPO is the Minnesota Pollution Control Agency's (MPCA) permitting, compliance, and enforcement information management system, which facilitates the issuance of permits and manages compliance." ;
    rdfs:subClassOf epa-frs:FRS-Facility .

epa-frs:MO-DNR-Facility a owl:Class ;
    rdfs:label "MISSOURI DEPARTMENT OF NATURAL RESOURCES" ;
    dcterms:description "The Missouri Department of Natural Resources (MO-DNR) involves a resource assessment and monitoring program, biological criteria development, monitoring of targeted sites to determine compliance with the designated use of aquatic life protection in the standards, monitoring for 303(3) purposes, and the development of a stream classification framework." ;
    rdfs:subClassOf epa-frs:FRS-Facility .

epa-frs:MS-ENSITE-Facility a owl:Class ;
    rdfs:label "MISSISSIPPI - TOOLS FOR ENVIRONMENTAL MANAGEMENT AND PROTECTION ORGANIZATIONS" ;
    dcterms:description "The Mississippi Department of Environmental Quality (MDEQ), Office of Pollution Controls (OPC) maintains ENSITE, the Electronic Environmental Site Information System that regulates compliance assurance, permitting, activity tracking, and maintenance of a single agency interest-link to master file." ;
    rdfs:subClassOf epa-frs:FRS-Facility .

epa-frs:MT-CEDARS-Facility a owl:Class ;
    rdfs:label "MONTANA - CONSOLIDATED ENVIRONMENTAL DATA ACQUISITION AND RETRIEVAL SYSTEM" ;
    dcterms:description "The Montana Department of Environmental Quality (DEQ) Consolidated Environmental Data Acquisition and Retrieval System (MT-CEDARS) allows facilities throughout the state to quickly and easily report daily air and water quality data." ;
    rdfs:subClassOf epa-frs:FRS-Facility .

epa-frs:NC-FITS-Facility a owl:Class ;
    rdfs:label "NORTH CAROLINA - FACILITY IDENTIFICATION TEMPLATE FOR STATES" ;
    dcterms:description "The North Carolina Facility Identification Template for States (NC-FITS) derives FRS data for submittal to EPA via the central data exchange." ;
    rdfs:subClassOf epa-frs:FRS-Facility .

epa-frs:NCDB-Facility a owl:Class ;
    rdfs:label "NATIONAL COMPLIANCE DATABASE" ;
    dcterms:description "The National Compliance Database (NCDB) supports implementation of the Federal Insecticide, Fungicide, and Rodenticide Act (FIFRA) and the Toxic Substances Control Act (TSCA)." ;
    rdfs:subClassOf epa-frs:FRS-Facility .

epa-frs:ND-FP-Facility a owl:Class ;
    rdfs:label "NORTH DAKOTA - FACILITY PROFILE" ;
    dcterms:description "The North Dakota Facility Profile (ND-FP) contains facility based, integrated environmental information for the State of North Dakota." ;
    rdfs:subClassOf epa-frs:FRS-Facility .

epa-frs:NDEQ-Facility a owl:Class ;
    rdfs:label "NEBRASKA DEPARTMENT OF ENVIRONMENTAL QUALITY" ;
    dcterms:description "The Nebraska Department of Environmental Quality (DEQ) maintains the EPA facility files." ;
    rdfs:subClassOf epa-frs:FRS-Facility .

epa-frs:NEI-Facility a owl:Class ;
    rdfs:label "NATIONAL EMISSIONS INVENTORY" ;
    dcterms:description "The National Emissions Inventory contains information about stationary and mobile sources that emit criteria air pollutants and their precursors, as well as hazardous air pollutants (HAPs)." ;
    rdfs:subClassOf epa-frs:FRS-Facility .

epa-frs:NH-DES-Facility a owl:Class ;
    rdfs:label "NEW HAMPSHIRE - DEPARTMENT OF ENVIRONMENTAL SERVICES" ;
    dcterms:description "The New Hampshire Department of Environmental Services (NHDES) ensures high levels of water quality for water supplies, regulates the emissions of air pollutants, and fosters the proper management of municipal and industrial waste." ;
    rdfs:subClassOf epa-frs:FRS-Facility .

epa-frs:NJ-NJEMS-Facility a owl:Class ;
    rdfs:label "NEW JERSEY - NEW JERSEY ENVIRONMENTAL MANAGEMENT SYSTEM" ;
    dcterms:description "The New Jersey Department of Environmental Protection (NJDEP) Environmental Management System (NJEMS) is an integrated system that manages large databases of environmental information." ;
    rdfs:subClassOf epa-frs:FRS-Facility .

epa-frs:NM-TEMPO-Facility a owl:Class ;
    rdfs:label "NEW MEXICO-TOOLS FOR ENVIRONMENTAL MANAGEMENT AND PROTECTION ORGANIZATIONS" ;
    dcterms:description "New Mexico's -Tools For Environmental Management and Protection Organizations (NM-TEMPO) is New Mexico's integrated environmental management system." ;
    rdfs:subClassOf epa-frs:FRS-Facility .

epa-frs:NNEMS-Facility a owl:Class ;
    rdfs:label "NAVAJO NATION ENVIRONMENTAL MANAGEMENT SYSTEM" ;
    dcterms:description "The Navajo Nation Environmental Management System (NNEMS) contains facility information for the Navajo Nation." ;
    rdfs:subClassOf epa-frs:FRS-Facility .

epa-frs:NPDES-Facility a owl:Class ;
    rdfs:label "NATIONAL POLLUTANT DISCHARGE ELIMINATION SYSTEM (ICIS-NPDES)" ;
    dcterms:description "The National Pollutant Discharge Elimination System (NPDES) module of the Integrated Compliance Information System (ICIS). Under NPDES, all facilities that discharge pollutants from any point source into waters of the United States are required to obtain a permit. The permit will likely contain limits on what can be discharged, impose monitoring and reporting requirements, and include other provisions to ensure that the discharge does not adversely affect water quality." ;
    rdfs:subClassOf epa-frs:FRS-Facility .

epa-frs:NV-FP-Facility a owl:Class ;
    rdfs:label "NEVADA - FACILITY PROFILE" ;
    dcterms:description "The Nevada Facility Profile (NV-FP) system contains facility based, integrated environmental information for the State of Nevada." ;
    rdfs:subClassOf epa-frs:FRS-Facility .

epa-frs:OH-CORE-Facility a owl:Class ;
    rdfs:label "OHIO - CORE FACILITY INFORMATION" ;
    dcterms:description "The OH-CORE database contains information commonly shared among the Ohio EPA environmental programs. The information is facility-based, general in nature, and used to support specific programmatic systems while simultaneously maintaining an inventory of common facility-related data. Specific programmatic details are maintained in programmatic databases." ;
    rdfs:subClassOf epa-frs:FRS-Facility .

epa-frs:OR-DEQ-Facility a owl:Class ;
    rdfs:label "OREGON - DEPARTMENT OF ENVIRONMENTAL QUALITY" ;
    dcterms:description "The Oregon Department of Environmental Quality (DEQ) is a regulatory agency tasked with protecting the quality of Oregon's environment. DEQ uses a combination of technical assistance, inspections, and permitting to help public and private facilities and citizens understand and comply with state and federal environmental regulations." ;
    rdfs:subClassOf epa-frs:FRS-Facility .

epa-frs:OSHA-OIS-Facility a owl:Class ;
    rdfs:label "OCCUPATIONAL SAFETY AND HEALTH ADMINISTRATION INFORMATION SYSTEM" ;
    dcterms:description "The Department of Labor, Occupational Safety and Health Administration information system consists of inspection case detail for approximately 100,000 OSHA inspections conducted annually. The FRS dataset includes facilities that had inspections within the last 7 years within the mining, oil and gas, utilities, and manufacturing sectors." ;
    rdfs:subClassOf epa-frs:FRS-Facility .

epa-frs:OTAQREG-Facility a owl:Class ;
    rdfs:label "OFFICE OF TRANSPORTATION AND AIR QUALITY FUELS REGISTRATION" ;
    dcterms:description "IN ACCORDANCE WITH THE FEDERAL CLEAN AIR ACT (CAA) EPA ESTABLISHES FUEL QUALITY STANDARDS TO HELP PROTECT PUBLIC HEALTH AND THE ENVIRONMENT FROM HARMFUL GAS AND PARTICULATE MATTER EMISSIONS FROM MOTOR VEHICLES AND ENGINES. THE OFFICE OF TRANSPORTATION AND AIR QUALITY (OTAQ) HAS DEVELOPED THE REGISTRATION AND DC FUELS ONLINE APPLICATIONS IMPLEMENTED THROUGH EPA S CENTRAL DATA EXCHANGE (CDX) WHICH PROVIDES ONLINE APPLICATIONS TO ASSIST THE FUEL MANUFACTURING COMMUNITY WITH REGISTRATION AND COMPLIANCE WITH REPORTING REQUIREMENTS." ;
    rdfs:subClassOf epa-frs:FRS-Facility .

epa-frs:PA-EFACTS-Facility a owl:Class ;
    rdfs:label "PENNSYLVANIA - ENVIRONMENTAL FACILITY APPLICATION COMPLIANCE TRACKING SYSTEM" ;
    dcterms:description "Pennsylvania's Department of Environmental Protection's (DEP) Environmental, Facility, Application, and Compliance Tracking System (PA-EFACTS) is a department-wide database that provides a holistic view of clients and sites (including facilities) that DEP regulates." ;
    rdfs:subClassOf epa-frs:FRS-Facility .

epa-frs:PDS-Facility a owl:Class ;
    rdfs:label "PERMIT DATA SYSTEM" ;
    dcterms:description "The Arkansas Permit Data System (PDS) is an integrated system maintaining data on air quality, mining, tires, solid waste, tank, water and hazardous waste, as well as inspections, invoicing and complaints." ;
    rdfs:subClassOf epa-frs:FRS-Facility .

epa-frs:PERMIT-TRACKING-Facility a owl:Class ;
    rdfs:label "ALBAMA - PERMIT TRACKING" ;
    dcterms:description "The Alabama Department of Environmental Management (ADEM) Permit Tracking system provides data entry, retrieval, and accounting functions and includes brief general data about facilities, their ADEM permits and fees owed and/or paid." ;
    rdfs:subClassOf epa-frs:FRS-Facility .

epa-frs:RADINFO-Facility a owl:Class ;
    rdfs:label "RADIATION INFORMATION SYSTEM" ;
    dcterms:description "The Radiation Information System (RADINFO) contains information about facilities that are regulated by US EPA for radiation and radioactivity." ;
    rdfs:subClassOf epa-frs:FRS-Facility .

epa-frs:RBLC-Facility a owl:Class ;
    rdfs:label "RACT/BACT/LAER CLEARINGHOUSE" ;
    dcterms:description "The RACT/BACT/LAER Clearinghouse (RBLC) database contains case-specific information on the \"best available\" air pollution technologies that have been required to reduce the emission of air pollutions from stationary sources.  RACT, or Reasonably Available Control Technology, is required on existing sources in areas that are not meeting national ambient air quality standards. BACT, or Best Available Control Technology, is required on major new or modified sources in clean areas. LAER, or Lowest Achievable Emission Rate, is required on major new or modified sources in non-attainment areas." ;
    rdfs:subClassOf epa-frs:FRS-Facility .

epa-frs:RCRAINFO-Facility a owl:Class ;
    rdfs:label "RESOURCE CONSERVATION AND RECOVERY ACT INFORMATION SYSTEM" ;
    dcterms:description "The Resource Conservation and Recovery Act Information System (RCRAInfo) is EPA's comprehensive information system in support of the Resource Conservation and Recovery Act (RCRA) of 1976 and the Hazardous and Solid Waste Amendments (HSWA) of 1984. It tracks many types of information about generators, transporters, treaters, storers, and disposers of hazardous waste." ;
    rdfs:subClassOf epa-frs:FRS-Facility .

epa-frs:REGION-Facility a owl:Class ;
    rdfs:label "REGION" ;
    dcterms:description "A COLLECTION OF INFORMATION ABOUT LIKE FACILITIES EXISTING IN AN EPA REGION FOR SPECIALIZED PURPOSES, ONE OF WHICH MAY BE IMPROVING GEOSPATIAL INFORMATION." ;
    rdfs:subClassOf epa-frs:FRS-Facility .

epa-frs:RFS-Facility a owl:Class ;
    rdfs:label "RENEWABLE FUEL STANDARD" ;
    dcterms:description "The Renewable Fuel Standard (RFS) Program encourages the blending of renewable fuels into our nation's motor vehicle fuel by establishing annual renewable fuel standards, responsibilities of refiners and other fuel producers, a trading system and other compliance mechanisms, and recordkeeping and reporting requirements. In addition to the rule, EPA has published a Regulatory Impact Analysis (RIA), which contains analyses of the economic and environmental impacts of the expanded use of renewable fuels under this program. A renewable fuel is defined as a motor vehicle fuel that is produced from plant or animal products or wastes, as opposed to fossil fuel sources." ;
    rdfs:subClassOf epa-frs:FRS-Facility .

epa-frs:RI-PLOVER-Facility a owl:Class ;
    rdfs:label "RHODE ISLAND - PERMITS, LICENSES AND OTHER VITAL ENVIRONMENTAL RECORDS" ;
    dcterms:description "The Rhode Island - Permits, Licenses and Other Vital Environmental Records (RI-PLOVER) is Rhode Island's Department of Environmental Management's regulatory programs' integrated information management system." ;
    rdfs:subClassOf epa-frs:FRS-Facility .

epa-frs:RMP-Facility a owl:Class ;
    rdfs:label "RISK MANAGEMENT PLAN" ;
    dcterms:description "The Risk Management Plan (RMP) database stores the risk management plans reported by companies that handle, manufacture, use, or store certain flammable or toxic substances, as required under section 112(r) of the Clean Air Act (CAA)." ;
    rdfs:subClassOf epa-frs:FRS-Facility .

epa-frs:SC-EFIS-Facility a owl:Class ;
    rdfs:label "SOUTH CAROLINA - ENVIRONMENTAL FACILITY INFORMATION SYSTEM" ;
    dcterms:description "The South Carolina Department of Health and Environmental Control (DHEC) Environmental Facility Information System (SC-EFIS) integrates information on environmental facilities, permits, violations, enforcement actions, and compliance activities needed to support regulatory requirements and target environmental quality improvements for the water, air, solid waste, and hazardous waste program areas." ;
    rdfs:subClassOf epa-frs:FRS-Facility .

epa-frs:SEMS-Facility a owl:Class ;
    rdfs:label "SUPERFUND ENTERPRISE MANAGEMENT SYSTEM" ;
    dcterms:description "THE SUPERFUND ENTERPRISE MANAGEMENT SYSTEM (SEMS) INTEGRATES MULTIPLE LEGACY SYSTEMS INTO A COMPREHENSIVE TRACKING AND REPORTING TOOL, PROVIDING DATA ON THE INVENTORY OF ACTIVE AND ARCHIVED HAZARDOUS WASTE SITES EVALUATED BY THE SUPERFUND PROGRAM. IT CONTAINS SITES THAT ARE EITHER PROPOSED TO BE OR ARE ON THE NATIONAL PRIORITIES LIST (NPL) AS WELL AS SITES THAT ARE IN THE SCREENING AND ASSESSMENT PHASE FOR POSSIBLE INCLUSION ON THE NPL." ;
    rdfs:subClassOf epa-frs:FRS-Facility .

epa-frs:SFDW-Facility a owl:Class ;
    rdfs:label "SAFE DRINKING WATER INFORMATION SYSTEM" ;
    dcterms:description "The Safe Drinking Water Information System contains information about public water systems and their violations of EPA's drinking water regulations." ;
    rdfs:subClassOf epa-frs:FRS-Facility .

epa-frs:SIMS-Facility a owl:Class ;
    rdfs:label "CT - SITE INFORMATION MANAGEMENT SYSTEM" ;
    dcterms:description "A suite of Web-based applications designed to allow the Connecticut Department of Environmental Protection (DEP) staff to harmonize environmental interest information from disparate systems into a single agency-wide data repository (known as CFI). The Site Information Management System (SIMS) provides tools for identifying and resolving duplicate data, querying data (using both tabular and geospatial methods), and viewing and maintaining documents associated to the data." ;
    rdfs:subClassOf epa-frs:FRS-Facility .

epa-frs:SRPMICEMS-Facility a owl:Class ;
    rdfs:label "SALT RIVER PIMA-MARICOPA INDIAN COMMUNITY ENVIRONMENTAL MANAGEMENT SYSTEM" ;
    dcterms:description "The Salt River Pima-Maricopa Indian Community Environmental Management System (SRPMICEMS) contains facility information for the Salt River Pima-Maricopa Indian Community." ;
    rdfs:subClassOf epa-frs:FRS-Facility .

epa-frs:SSTS-Facility a owl:Class ;
    rdfs:label "SECTION SEVEN TRACKING SYSTEM" ;
    dcterms:description "The Section Seven Tracking System (SSTS) tracks the registration of all pesticide-producing establishments and tracks annually the types and amounts of pesticides, active ingredients, and related devices that are produced, sold, or distributed." ;
    rdfs:subClassOf epa-frs:FRS-Facility .

epa-frs:STATE-Facility a owl:Class ;
    rdfs:label "STATE SYSTEMS" ;
    dcterms:description "The STATE acronym is used for facilities entered manually through the FRS Linkage Application, used primarily by State users for a variety of state programs." ;
    rdfs:subClassOf epa-frs:FRS-Facility .

epa-frs:SWIPR-Facility a owl:Class ;
    rdfs:label "SUBPART W IMPOUNDMENT PHOTOGRAPHIC REPORTING" ;
    dcterms:description "Under section 112 of the Clean Air Act, the EPA regulates toxic air pollutants. These regulations are known as the National Emission Standards for Hazardous Air Pollutants (NESHAPs). The SWIPR program delivers a web-based reporting system, which allows mill owners and operators to comply with NESHAPs regulations." ;
    rdfs:subClassOf epa-frs:FRS-Facility .

epa-frs:TEST-Facility a owl:Class ;
    rdfs:label "TEST PROGRAM FOR CDX" ;
    dcterms:description "TEST PROGRAM FOR CDX" ;
    rdfs:subClassOf epa-frs:FRS-Facility .

epa-frs:TRIS-Facility a owl:Class ;
    rdfs:label "TOXICS RELEASE INVENTORY SYSTEM" ;
    dcterms:description "The Toxic Release Inventory System (TRIS) is a publicly available EPA database reported annually by certain covered industry groups, as well as federal facilities. It contains information about more than 650 toxic chemicals that are being used, manufactured, treated, transported, or released into the environment, and includes information about waste management and pollution prevention activities." ;
    rdfs:subClassOf epa-frs:FRS-Facility .

epa-frs:TSCA-Facility a owl:Class ;
    rdfs:label "TOXIC SUBSTANCES CONTROL ACT" ;
    dcterms:description "The database that supports the Toxic Substances Control Act (TSCA) of 1976, which provides EPA with authority to require reporting, record-keeping and testing requirements, and restrictions relating to chemical substances and/or mixtures. Certain substances are generally excluded from TSCA, including, among others, food, drugs, cosmetics and pesticides. TSCA addresses the production, importation, use, and disposal of specific chemicals including polychlorinated biphenyls (PCBs), asbestos, radon and lead-based paint." ;
    rdfs:subClassOf epa-frs:FRS-Facility .

epa-frs:TX-TCEQ-ACR-Facility a owl:Class ;
    rdfs:label "TEXAS COMMISSION ON ENVIRONMENTAL QUALITY - AGENCY CENTRAL REGISTRY" ;
    dcterms:description "The Texas Commission on Environmental Quality (TCEQ) - Agency Central Registry is a computer application that allows the TCEQ to use a single, centralized area to record common information, such as the company names, addresses, and telephone numbers of those the TCEQ regulates. It also contains additional IDs (permits, registrations, authorizations, etc) and their status." ;
    rdfs:subClassOf epa-frs:FRS-Facility .

epa-frs:UORS-Facility a owl:Class ;
    rdfs:label "CALIFORNIA - USED OIL RECYCLING SYSTEM" ;
    dcterms:description "The Used Oil Recycling System (UORS) is managed by the California Integrated Waste Management Board (CIWMB). The CIWMB helps communities establish and promote convenient collection opportunities for used oil and used oil filters." ;
    rdfs:subClassOf epa-frs:FRS-Facility .

epa-frs:UST-Facility a owl:Class ;
    rdfs:label "UNDERGROUND STORAGE TANK" ;
    dcterms:description "The Underground Storage Tank (UST) system is a State of Tennessee system for managing information on underground storage tanks and any underground piping connected to the tanks that have at least 10 percent of its combined volume underground." ;
    rdfs:subClassOf epa-frs:FRS-Facility .

epa-frs:WA-FSIS-Facility a owl:Class ;
    rdfs:label "WASHINGTON - FACILITY / SITE IDENTIFICATION SYSTEM" ;
    dcterms:description "The Washington Facility / Site Identification System (WA-FSIS) provides a means to query and display data maintained by the Department of Ecology. The system contains key information for each facility/site that is currently, or has been, of interest to the departments air quality, dam safety, hazardous waste, toxic cleanup, and water quality programs." ;
    rdfs:subClassOf epa-frs:FRS-Facility .

epa-frs:WI-ESR-Facility a owl:Class ;
    rdfs:label "WISCONSIN - ENVIRONMENTAL SYSTEM REGISTRY" ;
    dcterms:description "The Wisconsin Environmental Site Register (WI-ESR) is a database that contains core information about facilities, organizations, and people related to the Wisconsin Department of Natural Resources (DNR)." ;
    rdfs:subClassOf epa-frs:FRS-Facility .

epa-frs:Agency.Congress a owl:Class ;
    rdfs:label "Congress" ;
    rdfs:subClassOf epa-frs:Agency .

epa-frs:Agency.State a owl:Class ;
    rdfs:label "State" ;
    rdfs:subClassOf epa-frs:Agency .

epa-frs:Agency.VeteransAffairs a owl:Class ;
    rdfs:label "Veterans Affairs" ;
    rdfs:subClassOf epa-frs:Agency .

epa-frs:ChemicalReleasePrograms a owl:Class ;
    rdfs:label "CHEMICAL RELEASE PROGRAMS"^^xsd:string ;
    dcterms:description "ENVIRONMENTAL PROGRAMS THAT REGULATE OR MONITOR CHEMICALS RELEASED TO THE ENVIRONMENT (E.G., TOXIC RELEASE INVENTORY, RELEASE ASSESSMENTS)."^^xsd:string ;
    rdfs:subClassOf epa-frs:EnvironmentalInterest .

epa-frs:FacilitySiteIdentification a owl:Class ;
    rdfs:label "FACILITY/SITE IDENTIFICATION"^^xsd:string ;
    dcterms:description "INCLUDES SYSTEMS THAT MAINTAIN BASIC IDENTIFICATION INFORMATION ABOUT FACILITIES/SITES AND LINKAGES TO ENVIRONMENTAL PERMITS AND PROGRAMS AT THE STATE, TRIBAL AND NATIONAL LEVEL."^^xsd:string ;
    rdfs:subClassOf epa-frs:EnvironmentalInterest .

epa-frs:UndergroundStorageTankPrograms a owl:Class ;
    rdfs:label "UNDERGROUND STORAGE TANK PROGRAMS"^^xsd:string ;
    dcterms:description "ENVIRONMENTAL PROGRAMS DESIGNED TO REDUCE THE CHANCE OF RELEASES FROM UNDERGROUND STORAGE TANKS (USTS), DETECT LEAKS AND SPILLS WHEN THEY DO OCCUR, AND SECURE PROMPT CLEANUP. "^^xsd:string ;
    rdfs:subClassOf epa-frs:EnvironmentalInterest .

epa-frs:Agency.Labor a owl:Class ;
    rdfs:label "Labor" ;
    rdfs:subClassOf epa-frs:Agency .

epa-frs:Agency.Treasury a owl:Class ;
    rdfs:label "Treasury" ;
    rdfs:subClassOf epa-frs:Agency .

epa-frs:AnimalOperations a owl:Class ;
    rdfs:label "ANIMAL OPERATIONS"^^xsd:string ;
    dcterms:description "ENVIRONMENTAL PROGRAMS RELATED TO ANIMAL OPERATIONS (E.G., LIVESTOCK WASTE CONTROL)."^^xsd:string ;
    rdfs:subClassOf epa-frs:EnvironmentalInterest .

epa-frs:GroundWaterPrograms a owl:Class ;
    rdfs:label "GROUND WATER PROGRAMS"^^xsd:string ;
    dcterms:description "ENVIRONMENTAL PROGRAMS DESIGNED TO PROTECT GROUND WATER (E.G., UNDERGROUND INJECTION CONTROL (UIC),  MINERAL EXPLORATION)."^^xsd:string ;
    rdfs:subClassOf epa-frs:EnvironmentalInterest .

epa-frs:WaterResourcesPrograms a owl:Class ;
    rdfs:label "WATER RESOURCES PROGRAMS"^^xsd:string ;
    dcterms:description "ENVIRONMENTAL PROGRAMS THAT MANAGE WATER RESOURCES TO MEET THE NEEDS OF THE NATURAL ENVIRONMENT AND HUMAN COMMUNITIES, INCLUDING WATERSHED MANAGEMENT, STREAM FLOWS, WATER RIGHTS, WELL DRILLING, USE OF WATER SUPPLIES, AND DAM SAFETY."^^xsd:string ;
    rdfs:subClassOf epa-frs:EnvironmentalInterest .

epa-frs:ChemicalStoragePrograms a owl:Class ;
    rdfs:label "CHEMICAL STORAGE PROGRAMS"^^xsd:string ;
    dcterms:description "ENVIRONMENTAL PROGRAMS THAT REGULATE OR MONITOR THE STORAGE OF CHEMICALS (E.G., RISK MANAGEMENT PROGRAM, SUPERFUND AMENDMENTS AND REAUTHORIZATION ACT (SARA) TITLE III PROGRAM)."^^xsd:string ;
    rdfs:subClassOf epa-frs:EnvironmentalInterest .

epa-frs:DrinkingWaterPrograms a owl:Class ;
    rdfs:label "DRINKING WATER PROGRAMS"^^xsd:string ;
    dcterms:description "ENVIRONMENTAL PROGRAMS THAT PROTECT THE QUALITY OF DRINKING WATER IN THE UNITED STATES, AS REQUIRED BY THE SAFE DRINKING WATER ACT."^^xsd:string ;
    rdfs:subClassOf epa-frs:EnvironmentalInterest .

epa-frs:LegalEnforcementActivities a owl:Class ;
    rdfs:label "LEGAL/ENFORCEMENT ACTIVITIES"^^xsd:string ;
    dcterms:description "LEGAL OR ENFORCEMENT ACTIVITIES IN SUPPORT OF OTHER ENVIRONMENTAL PROGRAMS."^^xsd:string ;
    rdfs:subClassOf epa-frs:EnvironmentalInterest .

epa-frs:PesticidesPrograms a owl:Class ;
    rdfs:label "PESTICIDES PROGRAMS"^^xsd:string ;
    dcterms:description "ENVIRONMENTAL PROGRAMS THAT MONITOR BUSINESSES, GOVERNMENT AGENCIES, AND INDIVIDUALS THAT HANDLE, STORE, SELL, AND/OR APPLY PESITICIDES."^^xsd:string ;
    rdfs:subClassOf epa-frs:EnvironmentalInterest .

epa-frs:Agency.Commerce a owl:Class ;
    rdfs:label "Commerce" ;
    rdfs:subClassOf epa-frs:Agency .

epa-frs:Agency.HealthandHumanServices a owl:Class ;
    rdfs:label "Health and Human Services" ;
    rdfs:subClassOf epa-frs:Agency .

epa-frs:Agency.Justice a owl:Class ;
    rdfs:label "Justice" ;
    rdfs:subClassOf epa-frs:Agency .

epa-frs:AssistanceAndSupportPrograms a owl:Class ;
    rdfs:label "ASSISTANCE AND SUPPORT PROGRAMS"^^xsd:string ;
    dcterms:description "ENVIRONMENTAL PROGRAMS THAT PROVIDE ASSISTANCE TO THE REGULATED COMMUNITY AND THE GENERAL PUBLIC (E.G., ENVIRONMENTAL GRANTS, OUTREACH ACTIVITIES) OR ACTIVITIES THAT PROVIDE SUPPORT ACROSS ENVIRONMENTAL PROGRAMS."^^xsd:string ;
    rdfs:subClassOf epa-frs:EnvironmentalInterest .

epa-frs:RadiationProtectionPrograms a owl:Class ;
    rdfs:label "RADIATION PROTECTION PROGRAMS"^^xsd:string ;
    dcterms:description "ENVIRONMENTAL PROGRAMS DESIGNED TO PROTECT PEOPLE AND THE ENVIRONMENT FROM HARMFUL EXPOSURE TO RADIATION"^^xsd:string ;
    rdfs:subClassOf epa-frs:EnvironmentalInterest .

epa-frs:ElectronicPermitSystem a owl:Class ;
    rdfs:label "ELECTRONIC PERMIT SYSTEM"^^xsd:string ;
    dcterms:description "ELECTRONIC PERMIT SYSTEM"^^xsd:string ;
    rdfs:subClassOf epa-frs:EnvironmentalInterest .

epa-frs:Agency.Agriculture a owl:Class ;
    rdfs:label "Agriculture" ;
    rdfs:subClassOf epa-frs:Agency .

epa-frs:Agency.Interior a owl:Class ;
    rdfs:label "Interior" ;
    rdfs:subClassOf epa-frs:Agency .

epa-frs:Agency.Transportation a owl:Class ;
    rdfs:label "Transportation" ;
    rdfs:subClassOf epa-frs:Agency .

epa-frs:Agency.HomelandSecurity a owl:Class ;
    rdfs:label "Homeland Security" ;
    rdfs:subClassOf epa-frs:Agency .

epa-frs:RemediationAndRedevelopmentPrograms a owl:Class ;
    rdfs:label "REMEDIATION AND REDEVELOPMENT PROGRAMS"^^xsd:string ;
    dcterms:description "ENVIRONMENTAL PROGRAMS AIMED AT CLEANING UP AND/OR REDEVELOPING UNCONTROLLED OR ABANDONED PLACES WHERE HAZARDOUS WASTE MAY BE LOCATED POSSIBLY AFFECTING LOCAL ECOSYSTEMS OR PEOPLE."^^xsd:string ;
    rdfs:subClassOf epa-frs:EnvironmentalInterest .

epa-frs:SolidWastePrograms a owl:Class ;
    rdfs:label "SOLID WASTE PROGRAMS"^^xsd:string ;
    dcterms:description "ENVIRONMENTAL PROGRAMS THAT REGULATE SOLID WASTES (E.G., COMPOST SITES, LANDFILLS, TRANSFER STATIONS)."^^xsd:string ;
    rdfs:subClassOf epa-frs:EnvironmentalInterest .

epa-frs:Agency.Defense a owl:Class ;
    rdfs:label "Defense" ;
    rdfs:subClassOf epa-frs:Agency .

epa-frs:HazardousWastePrograms a owl:Class ;
    rdfs:label "HAZARDOUS WASTE PROGRAMS"^^xsd:string ;
    dcterms:description "ENVIRONMENTAL PROGRAMS THAT REGULATE HAZARDOUS WASTE, INCLUDING THE GENERATION, TRANSPORTATION, TREATMENT, STORAGE, AND DISPOSAL OF HAZARDOUS WASTE, AS REQUIRED BY THE RESOURCE CONSERVATION AND RECOVERY ACT (RCRA)."^^xsd:string ;
    rdfs:subClassOf epa-frs:EnvironmentalInterest .

epa-frs:Agency.Energy a owl:Class ;
    rdfs:label "Energy" ;
    rdfs:subClassOf epa-frs:Agency .

epa-frs:WasteWaterPrograms a owl:Class ;
    rdfs:label "WASTE WATER PROGRAMS"^^xsd:string ;
    dcterms:description "ENVIRONMENTAL PROGRAMS THAT REGULATE DISCHARGES OF POLLUTANTS TO WATERS OF THE UNITED STATES, AS REQUIRED BY THE CLEAN WATER ACT."^^xsd:string ;
    rdfs:subClassOf epa-frs:EnvironmentalInterest .

epa-frs:AirPrograms a owl:Class ;
    rdfs:label "AIR PROGRAMS"^^xsd:string ;
    dcterms:description "ENVIRONMENTAL PROGRAMS THAT REGULATE OR MONITOR AIR EMISSIONS FROM AREA, STATIONARY, AND MOBILE SOURCES, AS REQUIRED BY THE CLEAN AIR ACT."^^xsd:string ;
    rdfs:subClassOf epa-frs:EnvironmentalInterest .

